@prefix : <https://linked.data.gov.au/dataset/gnaf/code/streetClass/> .
@prefix cs: <https://linked.data.gov.au/dataset/gnaf/code/streetClass> .
@prefix dcterms: <http://purl.org/dc/terms/> .
@prefix iso19153: <http://def.isotc211.org/iso19135/-1/2015/CoreModel/code/RE_ItemStatus/> .
@prefix rdfs: <http://www.w3.org/2000/01/rdf-schema#> .
@prefix sdo: <https://schema.org/> .
@prefix skos: <http://www.w3.org/2004/02/skos/core#> .
@prefix status: <http://purl.org/linked-data/registry#> .
@prefix xsd: <http://www.w3.org/2001/XMLSchema#> .

:C a skos:Concept ;
    dcterms:identifier "C"^^xsd:token ;
    status:status iso19153:original ;
    rdfs:isDefinedBy cs: ;
    skos:definition "A Confirmed Street Is Present In The Roads Data Of The Psma Transport And Topography Product For The Same Release."@en ;
    skos:inScheme cs: ;
    skos:prefLabel "Confirmed"@en ;
    skos:topConceptOf cs: .

:U a skos:Concept ;
    dcterms:identifier "U"^^xsd:token ;
    status:status iso19153:original ;
    rdfs:isDefinedBy cs: ;
    skos:definition "An Unconfirmed Street Is Not Present In The Roads Data Of The Psma Transport And Topography Product For The Same Release And Will Not Have A Street Locality Geocode."@en ;
    skos:inScheme cs: ;
    skos:prefLabel "Unconfirmed"@en ;
    skos:topConceptOf cs: .

cs: a skos:ConceptScheme ;
    dcterms:created "2018-02-10"^^xsd:date ;
    dcterms:identifier "streetClass"^^xsd:token ;
    dcterms:modified "2022-05-30"^^xsd:date ;
    dcterms:provenance "Automatically created from the G-NAF codelists"@en ;
    skos:definition "Description of what this street class code represents (e.g. N N - - Gazetted Street, Unconfirmed Street)"@en ;
    skos:hasTopConcept :C,
        :U ;
    skos:prefLabel "Street Class"@en ;
    sdo:creator <https://linked.data.gov.au/org/ga> ;
    sdo:publisher <https://linked.data.gov.au/org/icsm> .

