@prefix : <https://linked.data.gov.au/dataset/gnaf/code/mbMatchType/> .
@prefix cs: <https://linked.data.gov.au/dataset/gnaf/code/mbMatchType> .
@prefix dcterms: <http://purl.org/dc/terms/> .
@prefix iso19153: <http://def.isotc211.org/iso19135/-1/2015/CoreModel/code/RE_ItemStatus/> .
@prefix rdfs: <http://www.w3.org/2000/01/rdf-schema#> .
@prefix sdo: <https://schema.org/> .
@prefix skos: <http://www.w3.org/2004/02/skos/core#> .
@prefix status: <http://purl.org/linked-data/registry#> .
@prefix xsd: <http://www.w3.org/2001/XMLSchema#> .

:1 a skos:Concept ;
    dcterms:identifier "1"^^xsd:token ;
    status:status iso19153:original ;
    rdfs:isDefinedBy cs: ;
    skos:definition "A Parcel Level Geocode For The Address Has Been Applied And Clearly Within The Boundaries Of A Single Mesh Block.  The Mesh Block Id Allocated To The Address In Most Cases Is At A Very High Level Of Confidence."@en ;
    skos:inScheme cs: ;
    skos:prefLabel "Parcel Level Match"@en ;
    skos:topConceptOf cs: .

:2 a skos:Concept ;
    dcterms:identifier "2"^^xsd:token ;
    status:status iso19153:original ;
    rdfs:isDefinedBy cs: ;
    skos:definition "A Gap Geocoded Match For The Address Has Been Applied And Clearly Within The Boundaries Of A Single Mesh Block.  The Mesh Block Id Allocated To The Address In Most Cases Is At A High Level Of Confidence."@en ;
    skos:inScheme cs: ;
    skos:prefLabel "Gap Geocoded Address Level Match"@en ;
    skos:topConceptOf cs: .

:3 a skos:Concept ;
    dcterms:identifier "3"^^xsd:token ;
    status:status iso19153:original ;
    rdfs:isDefinedBy cs: ;
    skos:definition "A Street-Locality Level Geocode For The Address Has Been Applied And Clearly Within The Boundaries Of A Single Mesh Block.  The Mesh Block Id Allocated To The Address In Most Cases Is At A High Level Of Confidence."@en ;
    skos:inScheme cs: ;
    skos:prefLabel "Street Locality Level Single Match"@en ;
    skos:topConceptOf cs: .

:4 a skos:Concept ;
    dcterms:identifier "4"^^xsd:token ;
    status:status iso19153:original ;
    rdfs:isDefinedBy cs: ;
    skos:definition "A Street-Locality Level Geocode For The Address Has Been Applied And Is Within The Boundaries Of A Multiple Mesh Blocks.  The Mesh Block Id Allocated To The Address Is At A Low Level Of Confidence."@en ;
    skos:inScheme cs: ;
    skos:prefLabel "Street Locality Level Multiple Match"@en ;
    skos:topConceptOf cs: .

:5 a skos:Concept ;
    dcterms:identifier "5"^^xsd:token ;
    status:status iso19153:original ;
    rdfs:isDefinedBy cs: ;
    skos:definition "A Locality Level Geocode For The Address Has Been Applied And Is Within The Boundaries Of A Multiple Mesh Blocks.  The Mesh Block Id Allocated To The Address Is At A Very Low Level Of Confidence."@en ;
    skos:inScheme cs: ;
    skos:prefLabel "Locality Level Multiple Match"@en ;
    skos:topConceptOf cs: .

cs: a skos:ConceptScheme ;
    dcterms:created "2018-02-10"^^xsd:date ;
    dcterms:identifier "mbMatchType"^^xsd:token ;
    dcterms:modified "2022-05-30"^^xsd:date ;
    dcterms:provenance "Automatically created from the G-NAF codelists"@en ;
    skos:definition "Description of what the match code means"@en ;
    skos:hasTopConcept :1,
        :2,
        :3,
        :4,
        :5 ;
    skos:prefLabel "Mb Match Code"@en ;
    sdo:creator <https://linked.data.gov.au/org/ga> ;
    sdo:publisher <https://linked.data.gov.au/org/icsm> .

