@prefix : <https://linked.data.gov.au/dataset/gnaf/code/geocodeType/> .
@prefix cs: <https://linked.data.gov.au/dataset/gnaf/code/geocodeType> .
@prefix dcterms: <http://purl.org/dc/terms/> .
@prefix iso19153: <http://def.isotc211.org/iso19135/-1/2015/CoreModel/code/RE_ItemStatus/> .
@prefix rdfs: <http://www.w3.org/2000/01/rdf-schema#> .
@prefix sdo: <https://schema.org/> .
@prefix skos: <http://www.w3.org/2004/02/skos/core#> .
@prefix status: <http://purl.org/linked-data/registry#> .
@prefix xsd: <http://www.w3.org/2001/XMLSchema#> .

:BAP a skos:Concept ;
    dcterms:identifier "BAP"^^xsd:token ;
    status:status iso19153:original ;
    rdfs:isDefinedBy cs: ;
    skos:definition "Point Of Access To The Building."@en ;
    skos:inScheme cs: ;
    skos:prefLabel "Building Access Point"@en ;
    skos:topConceptOf cs: .

:BC a skos:Concept ;
    dcterms:identifier "BC"^^xsd:token ;
    status:status iso19153:original ;
    rdfs:isDefinedBy cs: ;
    skos:definition "Point As Centre Of Building And Lying Within Its Bounds (E.G. For U-Shaped Building)."@en ;
    skos:inScheme cs: ;
    skos:prefLabel "Building Centroid"@en ;
    skos:topConceptOf cs: .

:CDF a skos:Concept ;
    dcterms:identifier "CDF"^^xsd:token ;
    status:status iso19153:original ;
    rdfs:isDefinedBy cs: ;
    skos:definition "A Point On The Road Centre-Line Opposite The Centre Of The Road Frontage Of An Address Site."@en ;
    skos:inScheme cs: ;
    skos:prefLabel "Centre-Line Dropped Frontage"@en ;
    skos:topConceptOf cs: .

:DF a skos:Concept ;
    dcterms:identifier "DF"^^xsd:token ;
    status:status iso19153:original ;
    rdfs:isDefinedBy cs: ;
    skos:definition "Centre Of Driveway On Address Site Frontage."@en ;
    skos:inScheme cs: ;
    skos:prefLabel "Driveway Frontage"@en ;
    skos:topConceptOf cs: .

:EA a skos:Concept ;
    dcterms:identifier "EA"^^xsd:token ;
    status:status iso19153:original ;
    rdfs:isDefinedBy cs: ;
    skos:definition "Specific Building Or Property Access Point For Emergency Services."@en ;
    skos:inScheme cs: ;
    skos:prefLabel "Emergency Access"@en ;
    skos:topConceptOf cs: .

:EAS a skos:Concept ;
    dcterms:identifier "EAS"^^xsd:token ;
    status:status iso19153:original ;
    rdfs:isDefinedBy cs: ;
    skos:definition "Specific Building Or Property Secondary Access Point For Emergency Services."@en ;
    skos:inScheme cs: ;
    skos:prefLabel "Emergency Access Secondary"@en ;
    skos:topConceptOf cs: .

:ECP a skos:Concept ;
    dcterms:identifier "ECP"^^xsd:token ;
    status:status iso19153:original ;
    rdfs:isDefinedBy cs: ;
    skos:definition "Electricity Connection Point (E.G. Box, Or Underground Chamber)."@en ;
    skos:inScheme cs: ;
    skos:prefLabel "Electricity Connection Point"@en ;
    skos:topConceptOf cs: .

:EM a skos:Concept ;
    dcterms:identifier "EM"^^xsd:token ;
    status:status iso19153:original ;
    rdfs:isDefinedBy cs: ;
    skos:definition "Electricity Meter Point (E.G. Box, Or Underground Chamber)."@en ;
    skos:inScheme cs: ;
    skos:prefLabel "Electricity Meter"@en ;
    skos:topConceptOf cs: .

:FC a skos:Concept ;
    dcterms:identifier "FC"^^xsd:token ;
    status:status iso19153:original ;
    rdfs:isDefinedBy cs: ;
    skos:definition "Point On The Centre Of The Address Site Frontage."@en ;
    skos:inScheme cs: ;
    skos:prefLabel "Frontage Centre"@en ;
    skos:topConceptOf cs: .

:FCS a skos:Concept ;
    dcterms:identifier "FCS"^^xsd:token ;
    status:status iso19153:original ;
    rdfs:isDefinedBy cs: ;
    skos:definition "A Point Set Back From The Centre Of The Road Frontage Within An Address Site."@en ;
    skos:inScheme cs: ;
    skos:prefLabel "Frontage Centre Setback"@en ;
    skos:topConceptOf cs: .

:FDA a skos:Concept ;
    dcterms:identifier "FDA"^^xsd:token ;
    status:status iso19153:original ;
    rdfs:isDefinedBy cs: ;
    skos:definition "Front Door Of Building."@en ;
    skos:inScheme cs: ;
    skos:prefLabel "Front Door Access"@en ;
    skos:topConceptOf cs: .

:GCP a skos:Concept ;
    dcterms:identifier "GCP"^^xsd:token ;
    status:status iso19153:original ;
    rdfs:isDefinedBy cs: ;
    skos:definition "Gas Connection Point (E.G. Box, Or Underground Chamber)."@en ;
    skos:inScheme cs: ;
    skos:prefLabel "Gas Connection Point"@en ;
    skos:topConceptOf cs: .

:GG a skos:Concept ;
    dcterms:identifier "GG"^^xsd:token ;
    status:status iso19153:original ;
    rdfs:isDefinedBy cs: ;
    skos:definition "Point Programmatically Allocated During The G-Naf Production Process Proportionally Between Adjacent Address Locations (Based On Number_First)."@en ;
    skos:inScheme cs: ;
    skos:prefLabel "Gap Geocode"@en ;
    skos:topConceptOf cs: .

:GM a skos:Concept ;
    dcterms:identifier "GM"^^xsd:token ;
    status:status iso19153:original ;
    rdfs:isDefinedBy cs: ;
    skos:definition "Gas Meter Point (E.G. Box, Or Underground Chamber)."@en ;
    skos:inScheme cs: ;
    skos:prefLabel "Gas Meter"@en ;
    skos:topConceptOf cs: .

:ICP a skos:Concept ;
    dcterms:identifier "ICP"^^xsd:token ;
    status:status iso19153:original ;
    rdfs:isDefinedBy cs: ;
    skos:definition "Internet Connection Point (E.G. Box, Or Underground Chamber)."@en ;
    skos:inScheme cs: ;
    skos:prefLabel "Internet Connection Point"@en ;
    skos:topConceptOf cs: .

:LB a skos:Concept ;
    dcterms:identifier "LB"^^xsd:token ;
    status:status iso19153:original ;
    rdfs:isDefinedBy cs: ;
    skos:definition "Place Where Mail Is Deposited."@en ;
    skos:inScheme cs: ;
    skos:prefLabel "Letterbox"@en ;
    skos:topConceptOf cs: .

:LOC a skos:Concept ;
    dcterms:identifier "LOC"^^xsd:token ;
    status:status iso19153:original ;
    rdfs:isDefinedBy cs: ;
    skos:definition "Point Representing A Locality"@en ;
    skos:inScheme cs: ;
    skos:prefLabel "Locality"@en ;
    skos:topConceptOf cs: .

:PAP a skos:Concept ;
    dcterms:identifier "PAP"^^xsd:token ;
    status:status iso19153:original ;
    rdfs:isDefinedBy cs: ;
    skos:definition "Access Point (Centre Of) At The Road Frontage Of The Property."@en ;
    skos:inScheme cs: ;
    skos:prefLabel "Property Access Point"@en ;
    skos:topConceptOf cs: .

:PAPS a skos:Concept ;
    dcterms:identifier "PAPS"^^xsd:token ;
    status:status iso19153:original ;
    rdfs:isDefinedBy cs: ;
    skos:definition "A Point Set Back From The (Centre Of The) Access Point At The Road Frontage Of The Property."@en ;
    skos:inScheme cs: ;
    skos:prefLabel "Property Access Point Setback"@en ;
    skos:topConceptOf cs: .

:PC a skos:Concept ;
    dcterms:identifier "PC"^^xsd:token ;
    status:status iso19153:original ;
    rdfs:isDefinedBy cs: ;
    skos:definition "Point Of Centre Of Parcels Making Up A Property And Lying Within Its Boundaries (E.G. For L-Shaped Property)."@en ;
    skos:inScheme cs: ;
    skos:prefLabel "Property Centroid"@en ;
    skos:topConceptOf cs: .

:PCM a skos:Concept ;
    dcterms:identifier "PCM"^^xsd:token ;
    status:status iso19153:original ;
    rdfs:isDefinedBy cs: ;
    skos:definition "Point Manually Placed Approximately At Centre Of Parcels Making Up A Property And Lying Within Its Boundaries (E.G. For L-Shaped Property)."@en ;
    skos:inScheme cs: ;
    skos:prefLabel "Property Centroid Manual"@en ;
    skos:topConceptOf cs: .

:SCP a skos:Concept ;
    dcterms:identifier "SCP"^^xsd:token ;
    status:status iso19153:original ;
    rdfs:isDefinedBy cs: ;
    skos:definition "Sewerage Connection Point (E.G. Box, Or Underground Chamber)."@en ;
    skos:inScheme cs: ;
    skos:prefLabel "Sewerage Connection Point"@en ;
    skos:topConceptOf cs: .

:STL a skos:Concept ;
    dcterms:identifier "STL"^^xsd:token ;
    status:status iso19153:original ;
    rdfs:isDefinedBy cs: ;
    skos:definition "Point Representing The Extent Of A Street Within A Locality"@en ;
    skos:inScheme cs: ;
    skos:prefLabel "Street Locality"@en ;
    skos:topConceptOf cs: .

:TCP a skos:Concept ;
    dcterms:identifier "TCP"^^xsd:token ;
    status:status iso19153:original ;
    rdfs:isDefinedBy cs: ;
    skos:definition "Telephone Connection Point (E.G. Box, Or Underground Chamber)."@en ;
    skos:inScheme cs: ;
    skos:prefLabel "Telephone Connection Point"@en ;
    skos:topConceptOf cs: .

:UC a skos:Concept ;
    dcterms:identifier "UC"^^xsd:token ;
    status:status iso19153:original ;
    rdfs:isDefinedBy cs: ;
    skos:definition "Point At Centre Of Unit And Lying Within Its Bounds (E.G. For U-Shaped Unit)."@en ;
    skos:inScheme cs: ;
    skos:prefLabel "Unit Centroid"@en ;
    skos:topConceptOf cs: .

:UCM a skos:Concept ;
    dcterms:identifier "UCM"^^xsd:token ;
    status:status iso19153:original ;
    rdfs:isDefinedBy cs: ;
    skos:definition "Point Manually Placed Approximately At Centre Of Unit And Lying Within Its Bounds (E.G. For U-Shaped Unit)."@en ;
    skos:inScheme cs: ;
    skos:prefLabel "Unit Centroid Manual"@en ;
    skos:topConceptOf cs: .

:UNK a skos:Concept ;
    dcterms:identifier "UNK"^^xsd:token ;
    status:status iso19153:original ;
    rdfs:isDefinedBy cs: ;
    skos:definition "The Type Of Real World Feature The Point Represents Is Not Known."@en ;
    skos:inScheme cs: ;
    skos:prefLabel "Unknown"@en ;
    skos:topConceptOf cs: .

:WCP a skos:Concept ;
    dcterms:identifier "WCP"^^xsd:token ;
    status:status iso19153:original ;
    rdfs:isDefinedBy cs: ;
    skos:definition "Water Connection Point (E.G. Box, Or Underground Chamber)."@en ;
    skos:inScheme cs: ;
    skos:prefLabel "Water Connection Point"@en ;
    skos:topConceptOf cs: .

:WM a skos:Concept ;
    dcterms:identifier "WM"^^xsd:token ;
    status:status iso19153:original ;
    rdfs:isDefinedBy cs: ;
    skos:definition "Water Meter Point (E.G. Box, Or Underground Chamber)."@en ;
    skos:inScheme cs: ;
    skos:prefLabel "Water Meter"@en ;
    skos:topConceptOf cs: .

cs: a skos:ConceptScheme ;
    dcterms:created "2018-02-10"^^xsd:date ;
    dcterms:identifier "geocodeType"^^xsd:token ;
    dcterms:modified "2022-05-30"^^xsd:date ;
    dcterms:provenance "Automatically created from the G-NAF codelists"@en ;
    skos:definition "Description of geocode type code"@en ;
    skos:hasTopConcept :BAP,
        :BC,
        :CDF,
        :DF,
        :EA,
        :EAS,
        :ECP,
        :EM,
        :FC,
        :FCS,
        :FDA,
        :GCP,
        :GG,
        :GM,
        :ICP,
        :LB,
        :LOC,
        :PAP,
        :PAPS,
        :PC,
        :PCM,
        :SCP,
        :STL,
        :TCP,
        :UC,
        :UCM,
        :UNK,
        :WCP,
        :WM ;
    skos:prefLabel "Geocode Type"@en ;
    sdo:creator <https://linked.data.gov.au/org/ga> ;
    sdo:publisher <https://linked.data.gov.au/org/icsm> .

