@prefix : <https://linked.data.gov.au/dataset/gnaf/code/addressChangeType/> .
@prefix cs: <https://linked.data.gov.au/dataset/gnaf/code/addressChangeType> .
@prefix dcterms: <http://purl.org/dc/terms/> .
@prefix iso19153: <http://def.isotc211.org/iso19135/-1/2015/CoreModel/code/RE_ItemStatus/> .
@prefix rdfs: <http://www.w3.org/2000/01/rdf-schema#> .
@prefix sdo: <https://schema.org/> .
@prefix skos: <http://www.w3.org/2004/02/skos/core#> .
@prefix status: <http://purl.org/linked-data/registry#> .
@prefix xsd: <http://www.w3.org/2001/XMLSchema#> .

:LOC a skos:Concept ;
    dcterms:identifier "LOC"^^xsd:token ;
    status:status iso19153:original ;
    rdfs:isDefinedBy cs: ;
    skos:definition "Change To Locality Name Only"@en ;
    skos:inScheme cs: ;
    skos:prefLabel "Locality"@en ;
    skos:topConceptOf cs: .

:LOC-LOT a skos:Concept ;
    dcterms:identifier "LOC-LOT"^^xsd:token ;
    status:status iso19153:original ;
    rdfs:isDefinedBy cs: ;
    skos:definition "Change To Locality Name And Lot Number"@en ;
    skos:inScheme cs: ;
    skos:prefLabel "Locality-Lotno"@en ;
    skos:topConceptOf cs: .

:LOC-LOT-LVN a skos:Concept ;
    dcterms:identifier "LOC-LOT-LVN"^^xsd:token ;
    status:status iso19153:original ;
    rdfs:isDefinedBy cs: ;
    skos:definition "Change To Locality Name, Lot Number And Level Number"@en ;
    skos:inScheme cs: ;
    skos:prefLabel "Locality-Lotno-Levelno"@en ;
    skos:topConceptOf cs: .

:LOC-LOT-LVN-PPC a skos:Concept ;
    dcterms:identifier "LOC-LOT-LVN-PPC"^^xsd:token ;
    status:status iso19153:original ;
    rdfs:isDefinedBy cs: ;
    skos:definition "Change To Locality Name, Lot Number, Level Number And Primary Postcode"@en ;
    skos:inScheme cs: ;
    skos:prefLabel "Locality-Lotno-Levelno-Postcode"@en ;
    skos:topConceptOf cs: .

:LOC-LOT-PPC a skos:Concept ;
    dcterms:identifier "LOC-LOT-PPC"^^xsd:token ;
    status:status iso19153:original ;
    rdfs:isDefinedBy cs: ;
    skos:definition "Change To Locality Name, Lot Number And Primary Postcode"@en ;
    skos:inScheme cs: ;
    skos:prefLabel "Locality-Lotno-Postcode"@en ;
    skos:topConceptOf cs: .

:LOC-LVN a skos:Concept ;
    dcterms:identifier "LOC-LVN"^^xsd:token ;
    status:status iso19153:original ;
    rdfs:isDefinedBy cs: ;
    skos:definition "Change To Locality Name And Level Number"@en ;
    skos:inScheme cs: ;
    skos:prefLabel "Locality-Levelno"@en ;
    skos:topConceptOf cs: .

:LOC-LVN-PPC a skos:Concept ;
    dcterms:identifier "LOC-LVN-PPC"^^xsd:token ;
    status:status iso19153:original ;
    rdfs:isDefinedBy cs: ;
    skos:definition "Change To Locality Name, Level Number And Primary Postcode"@en ;
    skos:inScheme cs: ;
    skos:prefLabel "Locality-Levelno-Postcode"@en ;
    skos:topConceptOf cs: .

:LOC-NOF a skos:Concept ;
    dcterms:identifier "LOC-NOF"^^xsd:token ;
    status:status iso19153:original ;
    rdfs:isDefinedBy cs: ;
    skos:definition "Change To Locality Name And Number First"@en ;
    skos:inScheme cs: ;
    skos:prefLabel "Locality-Nofirst"@en ;
    skos:topConceptOf cs: .

:LOC-NOF-LOT a skos:Concept ;
    dcterms:identifier "LOC-NOF-LOT"^^xsd:token ;
    status:status iso19153:original ;
    rdfs:isDefinedBy cs: ;
    skos:definition "Change To Locality Name, Number First And Lot Number"@en ;
    skos:inScheme cs: ;
    skos:prefLabel "Locality-Nofirst-Lotno"@en ;
    skos:topConceptOf cs: .

:LOC-NOF-LOT-LVN a skos:Concept ;
    dcterms:identifier "LOC-NOF-LOT-LVN"^^xsd:token ;
    status:status iso19153:original ;
    rdfs:isDefinedBy cs: ;
    skos:definition "Change To Locality Name, Number First, Lot Number And Level Number"@en ;
    skos:inScheme cs: ;
    skos:prefLabel "Locality-Nofirst-Lotno-Levelno"@en ;
    skos:topConceptOf cs: .

:LOC-NOF-LOT-LVN-PPC a skos:Concept ;
    dcterms:identifier "LOC-NOF-LOT-LVN-PPC"^^xsd:token ;
    status:status iso19153:original ;
    rdfs:isDefinedBy cs: ;
    skos:definition "Change To Locality Name, Number First, Lot Number, Level Number And Primary Postcode"@en ;
    skos:inScheme cs: ;
    skos:prefLabel "Locality-Nofirst-Lotno-Levelno-Postcode"@en ;
    skos:topConceptOf cs: .

:LOC-NOF-LOT-PPC a skos:Concept ;
    dcterms:identifier "LOC-NOF-LOT-PPC"^^xsd:token ;
    status:status iso19153:original ;
    rdfs:isDefinedBy cs: ;
    skos:definition "Change To Locality Name, Number First, Lot Number And Primary Postcode"@en ;
    skos:inScheme cs: ;
    skos:prefLabel "Locality-Nofirst-Lotno-Postcode"@en ;
    skos:topConceptOf cs: .

:LOC-NOF-LVN a skos:Concept ;
    dcterms:identifier "LOC-NOF-LVN"^^xsd:token ;
    status:status iso19153:original ;
    rdfs:isDefinedBy cs: ;
    skos:definition "Change To Locality Name, Number First And Level Number"@en ;
    skos:inScheme cs: ;
    skos:prefLabel "Locality-Nofirst-Levelno"@en ;
    skos:topConceptOf cs: .

:LOC-NOF-LVN-PPC a skos:Concept ;
    dcterms:identifier "LOC-NOF-LVN-PPC"^^xsd:token ;
    status:status iso19153:original ;
    rdfs:isDefinedBy cs: ;
    skos:definition "Change To Locality Name, Number First, Level Number And Primary Postcode"@en ;
    skos:inScheme cs: ;
    skos:prefLabel "Locality-Nofirst-Levelno-Postcode"@en ;
    skos:topConceptOf cs: .

:LOC-NOF-NOL a skos:Concept ;
    dcterms:identifier "LOC-NOF-NOL"^^xsd:token ;
    status:status iso19153:original ;
    rdfs:isDefinedBy cs: ;
    skos:definition "Change To Locality Name, Number First And Number Last"@en ;
    skos:inScheme cs: ;
    skos:prefLabel "Locality-Nofirst-Nolast"@en ;
    skos:topConceptOf cs: .

:LOC-NOF-NOL-LOT a skos:Concept ;
    dcterms:identifier "LOC-NOF-NOL-LOT"^^xsd:token ;
    status:status iso19153:original ;
    rdfs:isDefinedBy cs: ;
    skos:definition "Change To Locality Name, Number First, Number Last And Lot Number"@en ;
    skos:inScheme cs: ;
    skos:prefLabel "Locality-Nofirst-Nolast-Lotno"@en ;
    skos:topConceptOf cs: .

:LOC-NOF-NOL-LOT-LVN a skos:Concept ;
    dcterms:identifier "LOC-NOF-NOL-LOT-LVN"^^xsd:token ;
    status:status iso19153:original ;
    rdfs:isDefinedBy cs: ;
    skos:definition "Change To Locality Name, Number First, Number Last, Lot Number And Level Number"@en ;
    skos:inScheme cs: ;
    skos:prefLabel "Locality-Nofirst-Nolast-Lotno-Levelno"@en ;
    skos:topConceptOf cs: .

:LOC-NOF-NOL-LOT-LVN-PPC a skos:Concept ;
    dcterms:identifier "LOC-NOF-NOL-LOT-LVN-PPC"^^xsd:token ;
    status:status iso19153:original ;
    rdfs:isDefinedBy cs: ;
    skos:definition "Change To Locality Name, Number First, Number Last, Lot Number, Level Number And Primary Postcode"@en ;
    skos:inScheme cs: ;
    skos:prefLabel "Locality-Nofirst-Nolast-Lotno-Levelno-Postcode"@en ;
    skos:topConceptOf cs: .

:LOC-NOF-NOL-LOT-PPC a skos:Concept ;
    dcterms:identifier "LOC-NOF-NOL-LOT-PPC"^^xsd:token ;
    status:status iso19153:original ;
    rdfs:isDefinedBy cs: ;
    skos:definition "Change To Locality Name, Number First, Number Last, Lot Number And Primary Postcode"@en ;
    skos:inScheme cs: ;
    skos:prefLabel "Locality-Nofirst-Nolast-Lotno-Postcode"@en ;
    skos:topConceptOf cs: .

:LOC-NOF-NOL-LVN a skos:Concept ;
    dcterms:identifier "LOC-NOF-NOL-LVN"^^xsd:token ;
    status:status iso19153:original ;
    rdfs:isDefinedBy cs: ;
    skos:definition "Change To Locality Name, Number First, Number Last And Level Number"@en ;
    skos:inScheme cs: ;
    skos:prefLabel "Locality-Nofirst-Nolast-Levelno"@en ;
    skos:topConceptOf cs: .

:LOC-NOF-NOL-LVN-PPC a skos:Concept ;
    dcterms:identifier "LOC-NOF-NOL-LVN-PPC"^^xsd:token ;
    status:status iso19153:original ;
    rdfs:isDefinedBy cs: ;
    skos:definition "Change To Locality Name, Number First, Number Last, Level Number And Primary Postcode"@en ;
    skos:inScheme cs: ;
    skos:prefLabel "Locality-Nofirst-Nolast-Levelno-Postcode"@en ;
    skos:topConceptOf cs: .

:LOC-NOF-NOL-PPC a skos:Concept ;
    dcterms:identifier "LOC-NOF-NOL-PPC"^^xsd:token ;
    status:status iso19153:original ;
    rdfs:isDefinedBy cs: ;
    skos:definition "Change To Locality Name, Number First, Number Last And Primary Postcode"@en ;
    skos:inScheme cs: ;
    skos:prefLabel "Locality-Nofirst-Nolast-Postcode"@en ;
    skos:topConceptOf cs: .

:LOC-NOF-PPC a skos:Concept ;
    dcterms:identifier "LOC-NOF-PPC"^^xsd:token ;
    status:status iso19153:original ;
    rdfs:isDefinedBy cs: ;
    skos:definition "Change To Locality Name, Number First And Primary Postcode"@en ;
    skos:inScheme cs: ;
    skos:prefLabel "Locality-Nofirst-Postcode"@en ;
    skos:topConceptOf cs: .

:LOC-NOL a skos:Concept ;
    dcterms:identifier "LOC-NOL"^^xsd:token ;
    status:status iso19153:original ;
    rdfs:isDefinedBy cs: ;
    skos:definition "Change To Locality Name And Number Last"@en ;
    skos:inScheme cs: ;
    skos:prefLabel "Locality-Nolast"@en ;
    skos:topConceptOf cs: .

:LOC-NOL-LOT a skos:Concept ;
    dcterms:identifier "LOC-NOL-LOT"^^xsd:token ;
    status:status iso19153:original ;
    rdfs:isDefinedBy cs: ;
    skos:definition "Change To Locality Name, Number Last And Lot Number"@en ;
    skos:inScheme cs: ;
    skos:prefLabel "Locality-Nolast-Lotno"@en ;
    skos:topConceptOf cs: .

:LOC-NOL-LOT-LVN a skos:Concept ;
    dcterms:identifier "LOC-NOL-LOT-LVN"^^xsd:token ;
    status:status iso19153:original ;
    rdfs:isDefinedBy cs: ;
    skos:definition "Change To Locality Name, Number Last, Lot Number And Level Number"@en ;
    skos:inScheme cs: ;
    skos:prefLabel "Locality-Nolast-Lotno-Levelno"@en ;
    skos:topConceptOf cs: .

:LOC-NOL-LOT-LVN-PPC a skos:Concept ;
    dcterms:identifier "LOC-NOL-LOT-LVN-PPC"^^xsd:token ;
    status:status iso19153:original ;
    rdfs:isDefinedBy cs: ;
    skos:definition "Change To Locality Name, Number Last, Lot Number, Level Number And Primary Postcode"@en ;
    skos:inScheme cs: ;
    skos:prefLabel "Locality-Nolast-Lotno-Levelno-Postcode"@en ;
    skos:topConceptOf cs: .

:LOC-NOL-LOT-PPC a skos:Concept ;
    dcterms:identifier "LOC-NOL-LOT-PPC"^^xsd:token ;
    status:status iso19153:original ;
    rdfs:isDefinedBy cs: ;
    skos:definition "Change To Locality Name, Number Last, Lot Number And Primary Postcode"@en ;
    skos:inScheme cs: ;
    skos:prefLabel "Locality-Nolast-Lotno-Postcode"@en ;
    skos:topConceptOf cs: .

:LOC-NOL-LVN a skos:Concept ;
    dcterms:identifier "LOC-NOL-LVN"^^xsd:token ;
    status:status iso19153:original ;
    rdfs:isDefinedBy cs: ;
    skos:definition "Change To Locality Name, Number Last And Level Number"@en ;
    skos:inScheme cs: ;
    skos:prefLabel "Locality-Nolast-Levelno"@en ;
    skos:topConceptOf cs: .

:LOC-NOL-LVN-PPC a skos:Concept ;
    dcterms:identifier "LOC-NOL-LVN-PPC"^^xsd:token ;
    status:status iso19153:original ;
    rdfs:isDefinedBy cs: ;
    skos:definition "Change To Locality Name, Number Last, Level Number And Primary Postcode"@en ;
    skos:inScheme cs: ;
    skos:prefLabel "Locality-Nolast-Levelno-Postcode"@en ;
    skos:topConceptOf cs: .

:LOC-NOL-PPC a skos:Concept ;
    dcterms:identifier "LOC-NOL-PPC"^^xsd:token ;
    status:status iso19153:original ;
    rdfs:isDefinedBy cs: ;
    skos:definition "Change To Locality Name, Number Last And Primary Postcode"@en ;
    skos:inScheme cs: ;
    skos:prefLabel "Locality-Nolast-Postcode"@en ;
    skos:topConceptOf cs: .

:LOC-PPC a skos:Concept ;
    dcterms:identifier "LOC-PPC"^^xsd:token ;
    status:status iso19153:original ;
    rdfs:isDefinedBy cs: ;
    skos:definition "Change To Locality Name And Primary Postcode"@en ;
    skos:inScheme cs: ;
    skos:prefLabel "Locality-Postcode"@en ;
    skos:topConceptOf cs: .

:LOC-STN a skos:Concept ;
    dcterms:identifier "LOC-STN"^^xsd:token ;
    status:status iso19153:original ;
    rdfs:isDefinedBy cs: ;
    skos:definition "Change To Locality Name And Street Name"@en ;
    skos:inScheme cs: ;
    skos:prefLabel "Locality-Stname"@en ;
    skos:topConceptOf cs: .

:LOC-STN-LOT a skos:Concept ;
    dcterms:identifier "LOC-STN-LOT"^^xsd:token ;
    status:status iso19153:original ;
    rdfs:isDefinedBy cs: ;
    skos:definition "Change To Locality Name, Street Name And Lot Number"@en ;
    skos:inScheme cs: ;
    skos:prefLabel "Locality-Stname-Lotno"@en ;
    skos:topConceptOf cs: .

:LOC-STN-LOT-LVN a skos:Concept ;
    dcterms:identifier "LOC-STN-LOT-LVN"^^xsd:token ;
    status:status iso19153:original ;
    rdfs:isDefinedBy cs: ;
    skos:definition "Change To Locality Name, Street Name, Lot Number And Level Number"@en ;
    skos:inScheme cs: ;
    skos:prefLabel "Locality-Stname-Lotno-Levelno"@en ;
    skos:topConceptOf cs: .

:LOC-STN-LOT-LVN-PPC a skos:Concept ;
    dcterms:identifier "LOC-STN-LOT-LVN-PPC"^^xsd:token ;
    status:status iso19153:original ;
    rdfs:isDefinedBy cs: ;
    skos:definition "Change To Locality Name, Street Name, Lot Number, Level Number And Primary Postcode"@en ;
    skos:inScheme cs: ;
    skos:prefLabel "Locality-Stname-Lotno-Levelno-Postcode"@en ;
    skos:topConceptOf cs: .

:LOC-STN-LOT-PPC a skos:Concept ;
    dcterms:identifier "LOC-STN-LOT-PPC"^^xsd:token ;
    status:status iso19153:original ;
    rdfs:isDefinedBy cs: ;
    skos:definition "Change To Locality Name, Street Name, Lot Number And Primary Postcode"@en ;
    skos:inScheme cs: ;
    skos:prefLabel "Locality-Stname-Lotno-Postcode"@en ;
    skos:topConceptOf cs: .

:LOC-STN-LVN a skos:Concept ;
    dcterms:identifier "LOC-STN-LVN"^^xsd:token ;
    status:status iso19153:original ;
    rdfs:isDefinedBy cs: ;
    skos:definition "Change To Locality Name, Street Name And Level Number"@en ;
    skos:inScheme cs: ;
    skos:prefLabel "Locality-Stname-Levelno"@en ;
    skos:topConceptOf cs: .

:LOC-STN-LVN-PPC a skos:Concept ;
    dcterms:identifier "LOC-STN-LVN-PPC"^^xsd:token ;
    status:status iso19153:original ;
    rdfs:isDefinedBy cs: ;
    skos:definition "Change To Locality Name, Street Name, Level Number And Primary Postcode"@en ;
    skos:inScheme cs: ;
    skos:prefLabel "Locality-Stname-Levelno-Postcode"@en ;
    skos:topConceptOf cs: .

:LOC-STN-NOF a skos:Concept ;
    dcterms:identifier "LOC-STN-NOF"^^xsd:token ;
    status:status iso19153:original ;
    rdfs:isDefinedBy cs: ;
    skos:definition "Change To Locality Name, Street Name And Number First"@en ;
    skos:inScheme cs: ;
    skos:prefLabel "Locality-Stname-Nofirst"@en ;
    skos:topConceptOf cs: .

:LOC-STN-NOF-LOT a skos:Concept ;
    dcterms:identifier "LOC-STN-NOF-LOT"^^xsd:token ;
    status:status iso19153:original ;
    rdfs:isDefinedBy cs: ;
    skos:definition "Change To Locality Name, Street Name, Number First And Lot Number"@en ;
    skos:inScheme cs: ;
    skos:prefLabel "Locality-Stname-Nofirst-Lotno"@en ;
    skos:topConceptOf cs: .

:LOC-STN-NOF-LOT-LVN a skos:Concept ;
    dcterms:identifier "LOC-STN-NOF-LOT-LVN"^^xsd:token ;
    status:status iso19153:original ;
    rdfs:isDefinedBy cs: ;
    skos:definition "Change To Locality Name, Street Name, Number First, Lot Number And Level Number"@en ;
    skos:inScheme cs: ;
    skos:prefLabel "Locality-Stname-Nofirst-Lotno-Levelno"@en ;
    skos:topConceptOf cs: .

:LOC-STN-NOF-LOT-LVN-PPC a skos:Concept ;
    dcterms:identifier "LOC-STN-NOF-LOT-LVN-PPC"^^xsd:token ;
    status:status iso19153:original ;
    rdfs:isDefinedBy cs: ;
    skos:definition "Change To Locality Name, Street Name, Number First, Lot Number, Level Number And Primary Postcode"@en ;
    skos:inScheme cs: ;
    skos:prefLabel "Locality-Stname-Nofirst-Lotno-Levelno-Postcode"@en ;
    skos:topConceptOf cs: .

:LOC-STN-NOF-LOT-PPC a skos:Concept ;
    dcterms:identifier "LOC-STN-NOF-LOT-PPC"^^xsd:token ;
    status:status iso19153:original ;
    rdfs:isDefinedBy cs: ;
    skos:definition "Change To Locality Name, Street Name, Number First, Lot Number And Primary Postcode"@en ;
    skos:inScheme cs: ;
    skos:prefLabel "Locality-Stname-Nofirst-Lotno-Postcode"@en ;
    skos:topConceptOf cs: .

:LOC-STN-NOF-LVN a skos:Concept ;
    dcterms:identifier "LOC-STN-NOF-LVN"^^xsd:token ;
    status:status iso19153:original ;
    rdfs:isDefinedBy cs: ;
    skos:definition "Change To Locality Name, Street Name, Number First And Level Number"@en ;
    skos:inScheme cs: ;
    skos:prefLabel "Locality-Stname-Nofirst-Levelno"@en ;
    skos:topConceptOf cs: .

:LOC-STN-NOF-LVN-PPC a skos:Concept ;
    dcterms:identifier "LOC-STN-NOF-LVN-PPC"^^xsd:token ;
    status:status iso19153:original ;
    rdfs:isDefinedBy cs: ;
    skos:definition "Change To Locality Name, Street Name, Number First, Level Number And Primary Postcode"@en ;
    skos:inScheme cs: ;
    skos:prefLabel "Locality-Stname-Nofirst-Levelno-Postcode"@en ;
    skos:topConceptOf cs: .

:LOC-STN-NOF-NOL a skos:Concept ;
    dcterms:identifier "LOC-STN-NOF-NOL"^^xsd:token ;
    status:status iso19153:original ;
    rdfs:isDefinedBy cs: ;
    skos:definition "Change To Locality Name, Street Name, Number First And Number Last"@en ;
    skos:inScheme cs: ;
    skos:prefLabel "Locality-Stname-Nofirst-Nolast"@en ;
    skos:topConceptOf cs: .

:LOC-STN-NOF-NOL-LOT a skos:Concept ;
    dcterms:identifier "LOC-STN-NOF-NOL-LOT"^^xsd:token ;
    status:status iso19153:original ;
    rdfs:isDefinedBy cs: ;
    skos:definition "Change To Locality Name, Street Name, Number First, Number Last And Lot Number"@en ;
    skos:inScheme cs: ;
    skos:prefLabel "Locality-Stname-Nofirst-Nolast-Lotno"@en ;
    skos:topConceptOf cs: .

:LOC-STN-NOF-NOL-LOT-LVN a skos:Concept ;
    dcterms:identifier "LOC-STN-NOF-NOL-LOT-LVN"^^xsd:token ;
    status:status iso19153:original ;
    rdfs:isDefinedBy cs: ;
    skos:definition "Change To Locality Name, Street Name, Number First, Number Last, Lot Number And Level Number"@en ;
    skos:inScheme cs: ;
    skos:prefLabel "Locality-Stname-Nofirst-Nolast-Lotno-Levelno"@en ;
    skos:topConceptOf cs: .

:LOC-STN-NOF-NOL-LOT-LVN-PPC a skos:Concept ;
    dcterms:identifier "LOC-STN-NOF-NOL-LOT-LVN-PPC"^^xsd:token ;
    status:status iso19153:original ;
    rdfs:isDefinedBy cs: ;
    skos:definition "Change To Locality Name, Street Name, Number First, Number Last, Lot Number, Level Number And Primary Postcode"@en ;
    skos:inScheme cs: ;
    skos:prefLabel "Locality-Stname-Nofirst-Nolast-Lotno-Levelno-Postcode"@en ;
    skos:topConceptOf cs: .

:LOC-STN-NOF-NOL-LOT-PPC a skos:Concept ;
    dcterms:identifier "LOC-STN-NOF-NOL-LOT-PPC"^^xsd:token ;
    status:status iso19153:original ;
    rdfs:isDefinedBy cs: ;
    skos:definition "Change To Locality Name, Street Name, Number First, Number Last, Lot Number And Primary Postcode"@en ;
    skos:inScheme cs: ;
    skos:prefLabel "Locality-Stname-Nofirst-Nolast-Lotno-Postcode"@en ;
    skos:topConceptOf cs: .

:LOC-STN-NOF-NOL-LVN a skos:Concept ;
    dcterms:identifier "LOC-STN-NOF-NOL-LVN"^^xsd:token ;
    status:status iso19153:original ;
    rdfs:isDefinedBy cs: ;
    skos:definition "Change To Locality Name, Street Name, Number First, Number Last And Level Number"@en ;
    skos:inScheme cs: ;
    skos:prefLabel "Locality-Stname-Nofirst-Nolast-Levelno"@en ;
    skos:topConceptOf cs: .

:LOC-STN-NOF-NOL-LVN-PPC a skos:Concept ;
    dcterms:identifier "LOC-STN-NOF-NOL-LVN-PPC"^^xsd:token ;
    status:status iso19153:original ;
    rdfs:isDefinedBy cs: ;
    skos:definition "Change To Locality Name, Street Name, Number First, Number Last, Level Number And Primary Postcode"@en ;
    skos:inScheme cs: ;
    skos:prefLabel "Locality-Stname-Nofirst-Nolast-Levelno-Postcode"@en ;
    skos:topConceptOf cs: .

:LOC-STN-NOF-NOL-PPC a skos:Concept ;
    dcterms:identifier "LOC-STN-NOF-NOL-PPC"^^xsd:token ;
    status:status iso19153:original ;
    rdfs:isDefinedBy cs: ;
    skos:definition "Change To Locality Name, Street Name, Number First, Number Last And Primary Postcode"@en ;
    skos:inScheme cs: ;
    skos:prefLabel "Locality-Stname-Nofirst-Nolast-Postcode"@en ;
    skos:topConceptOf cs: .

:LOC-STN-NOF-PPC a skos:Concept ;
    dcterms:identifier "LOC-STN-NOF-PPC"^^xsd:token ;
    status:status iso19153:original ;
    rdfs:isDefinedBy cs: ;
    skos:definition "Change To Locality Name, Street Name, Number First And Primary Postcode"@en ;
    skos:inScheme cs: ;
    skos:prefLabel "Locality-Stname-Nofirst-Postcode"@en ;
    skos:topConceptOf cs: .

:LOC-STN-NOL a skos:Concept ;
    dcterms:identifier "LOC-STN-NOL"^^xsd:token ;
    status:status iso19153:original ;
    rdfs:isDefinedBy cs: ;
    skos:definition "Change To Locality Name, Street Name And Number Last"@en ;
    skos:inScheme cs: ;
    skos:prefLabel "Locality-Stname-Nolast"@en ;
    skos:topConceptOf cs: .

:LOC-STN-NOL-LOT a skos:Concept ;
    dcterms:identifier "LOC-STN-NOL-LOT"^^xsd:token ;
    status:status iso19153:original ;
    rdfs:isDefinedBy cs: ;
    skos:definition "Change To Locality Name, Street Name, Number Last And Lot Number"@en ;
    skos:inScheme cs: ;
    skos:prefLabel "Locality-Stname-Nolast-Lotno"@en ;
    skos:topConceptOf cs: .

:LOC-STN-NOL-LOT-LVN a skos:Concept ;
    dcterms:identifier "LOC-STN-NOL-LOT-LVN"^^xsd:token ;
    status:status iso19153:original ;
    rdfs:isDefinedBy cs: ;
    skos:definition "Change To Locality Name, Street Name, Number Last, Lot Number And Level Number"@en ;
    skos:inScheme cs: ;
    skos:prefLabel "Locality-Stname-Nolast-Lotno-Levelno"@en ;
    skos:topConceptOf cs: .

:LOC-STN-NOL-LOT-LVN-PPC a skos:Concept ;
    dcterms:identifier "LOC-STN-NOL-LOT-LVN-PPC"^^xsd:token ;
    status:status iso19153:original ;
    rdfs:isDefinedBy cs: ;
    skos:definition "Change To Locality Name, Street Name, Number Last, Lot Number, Level Number And Primary Postcode"@en ;
    skos:inScheme cs: ;
    skos:prefLabel "Locality-Stname-Nolast-Lotno-Levelno-Postcode"@en ;
    skos:topConceptOf cs: .

:LOC-STN-NOL-LOT-PPC a skos:Concept ;
    dcterms:identifier "LOC-STN-NOL-LOT-PPC"^^xsd:token ;
    status:status iso19153:original ;
    rdfs:isDefinedBy cs: ;
    skos:definition "Change To Locality Name, Street Name, Number Last, Lot Number And Primary Postcode"@en ;
    skos:inScheme cs: ;
    skos:prefLabel "Locality-Stname-Nolast-Lotno-Postcode"@en ;
    skos:topConceptOf cs: .

:LOC-STN-NOL-LVN a skos:Concept ;
    dcterms:identifier "LOC-STN-NOL-LVN"^^xsd:token ;
    status:status iso19153:original ;
    rdfs:isDefinedBy cs: ;
    skos:definition "Change To Locality Name, Street Name, Number Last And Level Number"@en ;
    skos:inScheme cs: ;
    skos:prefLabel "Locality-Stname-Nolast-Levelno"@en ;
    skos:topConceptOf cs: .

:LOC-STN-NOL-LVN-PPC a skos:Concept ;
    dcterms:identifier "LOC-STN-NOL-LVN-PPC"^^xsd:token ;
    status:status iso19153:original ;
    rdfs:isDefinedBy cs: ;
    skos:definition "Change To Locality Name, Street Name, Number Last, Level Number And Primary Postcode"@en ;
    skos:inScheme cs: ;
    skos:prefLabel "Locality-Stname-Nolast-Levelno-Postcode"@en ;
    skos:topConceptOf cs: .

:LOC-STN-NOL-PPC a skos:Concept ;
    dcterms:identifier "LOC-STN-NOL-PPC"^^xsd:token ;
    status:status iso19153:original ;
    rdfs:isDefinedBy cs: ;
    skos:definition "Change To Locality Name, Street Name, Number Last And Primary Postcode"@en ;
    skos:inScheme cs: ;
    skos:prefLabel "Locality-Stname-Nolast-Postcode"@en ;
    skos:topConceptOf cs: .

:LOC-STN-PPC a skos:Concept ;
    dcterms:identifier "LOC-STN-PPC"^^xsd:token ;
    status:status iso19153:original ;
    rdfs:isDefinedBy cs: ;
    skos:definition "Change To Locality Name, Street Name And Primary Postcode"@en ;
    skos:inScheme cs: ;
    skos:prefLabel "Locality-Stname-Postcode"@en ;
    skos:topConceptOf cs: .

:LOC-STN-STS a skos:Concept ;
    dcterms:identifier "LOC-STN-STS"^^xsd:token ;
    status:status iso19153:original ;
    rdfs:isDefinedBy cs: ;
    skos:definition "Change To Locality Name, Street Name And Street Suffix"@en ;
    skos:inScheme cs: ;
    skos:prefLabel "Locality-Stname-Stsuffix"@en ;
    skos:topConceptOf cs: .

:LOC-STN-STS-LOT a skos:Concept ;
    dcterms:identifier "LOC-STN-STS-LOT"^^xsd:token ;
    status:status iso19153:original ;
    rdfs:isDefinedBy cs: ;
    skos:definition "Change To Locality Name, Street Name, Street Suffix And Lot Number"@en ;
    skos:inScheme cs: ;
    skos:prefLabel "Locality-Stname-Stsuffix-Lotno"@en ;
    skos:topConceptOf cs: .

:LOC-STN-STS-LOT-LVN a skos:Concept ;
    dcterms:identifier "LOC-STN-STS-LOT-LVN"^^xsd:token ;
    status:status iso19153:original ;
    rdfs:isDefinedBy cs: ;
    skos:definition "Change To Locality Name, Street Name, Street Suffix, Lot Number And Level Number"@en ;
    skos:inScheme cs: ;
    skos:prefLabel "Locality-Stname-Stsuffix-Lotno-Levelno"@en ;
    skos:topConceptOf cs: .

:LOC-STN-STS-LOT-LVN-PPC a skos:Concept ;
    dcterms:identifier "LOC-STN-STS-LOT-LVN-PPC"^^xsd:token ;
    status:status iso19153:original ;
    rdfs:isDefinedBy cs: ;
    skos:definition "Change To Locality Name, Street Name, Street Suffix, Lot Number, Level Number And Primary Postcode"@en ;
    skos:inScheme cs: ;
    skos:prefLabel "Locality-Stname-Stsuffix-Lotno-Levelno-Postcode"@en ;
    skos:topConceptOf cs: .

:LOC-STN-STS-LOT-PPC a skos:Concept ;
    dcterms:identifier "LOC-STN-STS-LOT-PPC"^^xsd:token ;
    status:status iso19153:original ;
    rdfs:isDefinedBy cs: ;
    skos:definition "Change To Locality Name, Street Name, Street Suffix, Lot Number And Primary Postcode"@en ;
    skos:inScheme cs: ;
    skos:prefLabel "Locality-Stname-Stsuffix-Lotno-Postcode"@en ;
    skos:topConceptOf cs: .

:LOC-STN-STS-LVN a skos:Concept ;
    dcterms:identifier "LOC-STN-STS-LVN"^^xsd:token ;
    status:status iso19153:original ;
    rdfs:isDefinedBy cs: ;
    skos:definition "Change To Locality Name, Street Name, Street Suffix And Level Number"@en ;
    skos:inScheme cs: ;
    skos:prefLabel "Locality-Stname-Stsuffix-Levelno"@en ;
    skos:topConceptOf cs: .

:LOC-STN-STS-LVN-PPC a skos:Concept ;
    dcterms:identifier "LOC-STN-STS-LVN-PPC"^^xsd:token ;
    status:status iso19153:original ;
    rdfs:isDefinedBy cs: ;
    skos:definition "Change To Locality Name, Street Name, Street Suffix, Level Number And Primary Postcode"@en ;
    skos:inScheme cs: ;
    skos:prefLabel "Locality-Stname-Stsuffix-Levelno-Postcode"@en ;
    skos:topConceptOf cs: .

:LOC-STN-STS-NOF a skos:Concept ;
    dcterms:identifier "LOC-STN-STS-NOF"^^xsd:token ;
    status:status iso19153:original ;
    rdfs:isDefinedBy cs: ;
    skos:definition "Change To Locality Name, Street Name, Street Suffix And Number First"@en ;
    skos:inScheme cs: ;
    skos:prefLabel "Locality-Stname-Stsuffix-Nofirst"@en ;
    skos:topConceptOf cs: .

:LOC-STN-STS-NOF-LOT a skos:Concept ;
    dcterms:identifier "LOC-STN-STS-NOF-LOT"^^xsd:token ;
    status:status iso19153:original ;
    rdfs:isDefinedBy cs: ;
    skos:definition "Change To Locality Name, Street Name, Street Suffix, Number First And Lot Number"@en ;
    skos:inScheme cs: ;
    skos:prefLabel "Locality-Stname-Stsuffix-Nofirst-Lotno"@en ;
    skos:topConceptOf cs: .

:LOC-STN-STS-NOF-LOT-LVN a skos:Concept ;
    dcterms:identifier "LOC-STN-STS-NOF-LOT-LVN"^^xsd:token ;
    status:status iso19153:original ;
    rdfs:isDefinedBy cs: ;
    skos:definition "Change To Locality Name, Street Name, Street Suffix, Number First, Lot Number And Level Number"@en ;
    skos:inScheme cs: ;
    skos:prefLabel "Locality-Stname-Stsuffix-Nofirst-Lotno-Levelno"@en ;
    skos:topConceptOf cs: .

:LOC-STN-STS-NOF-LOT-LVN-PPC a skos:Concept ;
    dcterms:identifier "LOC-STN-STS-NOF-LOT-LVN-PPC"^^xsd:token ;
    status:status iso19153:original ;
    rdfs:isDefinedBy cs: ;
    skos:definition "Change To Locality Name, Street Name, Street Suffix, Number First, Lot Number, Level Number And Primary Postcode"@en ;
    skos:inScheme cs: ;
    skos:prefLabel "Locality-Stname-Stsuffix-Nofirst-Lotno-Levelno-Postcode"@en ;
    skos:topConceptOf cs: .

:LOC-STN-STS-NOF-LOT-PPC a skos:Concept ;
    dcterms:identifier "LOC-STN-STS-NOF-LOT-PPC"^^xsd:token ;
    status:status iso19153:original ;
    rdfs:isDefinedBy cs: ;
    skos:definition "Change To Locality Name, Street Name, Street Suffix, Number First, Lot Number And Primary Postcode"@en ;
    skos:inScheme cs: ;
    skos:prefLabel "Locality-Stname-Stsuffix-Nofirst-Lotno-Postcode"@en ;
    skos:topConceptOf cs: .

:LOC-STN-STS-NOF-LVN a skos:Concept ;
    dcterms:identifier "LOC-STN-STS-NOF-LVN"^^xsd:token ;
    status:status iso19153:original ;
    rdfs:isDefinedBy cs: ;
    skos:definition "Change To Locality Name, Street Name, Street Suffix, Number First And Level Number"@en ;
    skos:inScheme cs: ;
    skos:prefLabel "Locality-Stname-Stsuffix-Nofirst-Levelno"@en ;
    skos:topConceptOf cs: .

:LOC-STN-STS-NOF-LVN-PPC a skos:Concept ;
    dcterms:identifier "LOC-STN-STS-NOF-LVN-PPC"^^xsd:token ;
    status:status iso19153:original ;
    rdfs:isDefinedBy cs: ;
    skos:definition "Change To Locality Name, Street Name, Street Suffix, Number First, Level Number And Primary Postcode"@en ;
    skos:inScheme cs: ;
    skos:prefLabel "Locality-Stname-Stsuffix-Nofirst-Levelno-Postcode"@en ;
    skos:topConceptOf cs: .

:LOC-STN-STS-NOF-NOL a skos:Concept ;
    dcterms:identifier "LOC-STN-STS-NOF-NOL"^^xsd:token ;
    status:status iso19153:original ;
    rdfs:isDefinedBy cs: ;
    skos:definition "Change To Locality Name, Street Name, Street Suffix, Number First And Number Last"@en ;
    skos:inScheme cs: ;
    skos:prefLabel "Locality-Stname-Stsuffix-Nofirst-Nolast"@en ;
    skos:topConceptOf cs: .

:LOC-STN-STS-NOF-NOL-LOT a skos:Concept ;
    dcterms:identifier "LOC-STN-STS-NOF-NOL-LOT"^^xsd:token ;
    status:status iso19153:original ;
    rdfs:isDefinedBy cs: ;
    skos:definition "Change To Locality Name, Street Name, Street Suffix, Number First, Number Last And Lot Number"@en ;
    skos:inScheme cs: ;
    skos:prefLabel "Locality-Stname-Stsuffix-Nofirst-Nolast-Lotno"@en ;
    skos:topConceptOf cs: .

:LOC-STN-STS-NOF-NOL-LOT-LVN a skos:Concept ;
    dcterms:identifier "LOC-STN-STS-NOF-NOL-LOT-LVN"^^xsd:token ;
    status:status iso19153:original ;
    rdfs:isDefinedBy cs: ;
    skos:definition "Change To Locality Name, Street Name, Street Suffix, Number First, Number Last, Lot Number And Level Number"@en ;
    skos:inScheme cs: ;
    skos:prefLabel "Locality-Stname-Stsuffix-Nofirst-Nolast-Lotno-Levelno"@en ;
    skos:topConceptOf cs: .

:LOC-STN-STS-NOF-NOL-LOT-LVN-PPC a skos:Concept ;
    dcterms:identifier "LOC-STN-STS-NOF-NOL-LOT-LVN-PPC"^^xsd:token ;
    status:status iso19153:original ;
    rdfs:isDefinedBy cs: ;
    skos:definition "Change To Locality Name, Street Name, Street Suffix, Number First, Number Last, Lot Number, Level Number And Primary Postcode"@en ;
    skos:inScheme cs: ;
    skos:prefLabel "Locality-Stname-Stsuffix-Nofirst-Nolast-Lotno-Levelno-Postcode"@en ;
    skos:topConceptOf cs: .

:LOC-STN-STS-NOF-NOL-LOT-PPC a skos:Concept ;
    dcterms:identifier "LOC-STN-STS-NOF-NOL-LOT-PPC"^^xsd:token ;
    status:status iso19153:original ;
    rdfs:isDefinedBy cs: ;
    skos:definition "Change To Locality Name, Street Name, Street Suffix, Number First, Number Last, Lot Number And Primary Postcode"@en ;
    skos:inScheme cs: ;
    skos:prefLabel "Locality-Stname-Stsuffix-Nofirst-Nolast-Lotno-Postcode"@en ;
    skos:topConceptOf cs: .

:LOC-STN-STS-NOF-NOL-LVN a skos:Concept ;
    dcterms:identifier "LOC-STN-STS-NOF-NOL-LVN"^^xsd:token ;
    status:status iso19153:original ;
    rdfs:isDefinedBy cs: ;
    skos:definition "Change To Locality Name, Street Name, Street Suffix, Number First, Number Last And Level Number"@en ;
    skos:inScheme cs: ;
    skos:prefLabel "Locality-Stname-Stsuffix-Nofirst-Nolast-Levelno"@en ;
    skos:topConceptOf cs: .

:LOC-STN-STS-NOF-NOL-LVN-PPC a skos:Concept ;
    dcterms:identifier "LOC-STN-STS-NOF-NOL-LVN-PPC"^^xsd:token ;
    status:status iso19153:original ;
    rdfs:isDefinedBy cs: ;
    skos:definition "Change To Locality Name, Street Name, Street Suffix, Number First, Number Last, Level Number And Primary Postcode"@en ;
    skos:inScheme cs: ;
    skos:prefLabel "Locality-Stname-Stsuffix-Nofirst-Nolast-Levelno-Postcode"@en ;
    skos:topConceptOf cs: .

:LOC-STN-STS-NOF-NOL-PPC a skos:Concept ;
    dcterms:identifier "LOC-STN-STS-NOF-NOL-PPC"^^xsd:token ;
    status:status iso19153:original ;
    rdfs:isDefinedBy cs: ;
    skos:definition "Change To Locality Name, Street Name, Street Suffix, Number First, Number Last And Primary Postcode"@en ;
    skos:inScheme cs: ;
    skos:prefLabel "Locality-Stname-Stsuffix-Nofirst-Nolast-Postcode"@en ;
    skos:topConceptOf cs: .

:LOC-STN-STS-NOF-PPC a skos:Concept ;
    dcterms:identifier "LOC-STN-STS-NOF-PPC"^^xsd:token ;
    status:status iso19153:original ;
    rdfs:isDefinedBy cs: ;
    skos:definition "Change To Locality Name, Street Name, Street Suffix, Number First And Primary Postcode"@en ;
    skos:inScheme cs: ;
    skos:prefLabel "Locality-Stname-Stsuffix-Nofirst-Postcode"@en ;
    skos:topConceptOf cs: .

:LOC-STN-STS-NOL a skos:Concept ;
    dcterms:identifier "LOC-STN-STS-NOL"^^xsd:token ;
    status:status iso19153:original ;
    rdfs:isDefinedBy cs: ;
    skos:definition "Change To Locality Name, Street Name, Street Suffix And Number Last"@en ;
    skos:inScheme cs: ;
    skos:prefLabel "Locality-Stname-Stsuffix-Nolast"@en ;
    skos:topConceptOf cs: .

:LOC-STN-STS-NOL-LOT a skos:Concept ;
    dcterms:identifier "LOC-STN-STS-NOL-LOT"^^xsd:token ;
    status:status iso19153:original ;
    rdfs:isDefinedBy cs: ;
    skos:definition "Change To Locality Name, Street Name, Street Suffix, Number Last And Lot Number"@en ;
    skos:inScheme cs: ;
    skos:prefLabel "Locality-Stname-Stsuffix-Nolast-Lotno"@en ;
    skos:topConceptOf cs: .

:LOC-STN-STS-NOL-LOT-LVN a skos:Concept ;
    dcterms:identifier "LOC-STN-STS-NOL-LOT-LVN"^^xsd:token ;
    status:status iso19153:original ;
    rdfs:isDefinedBy cs: ;
    skos:definition "Change To Locality Name, Street Name, Street Suffix, Number Last, Lot Number And Level Number"@en ;
    skos:inScheme cs: ;
    skos:prefLabel "Locality-Stname-Stsuffix-Nolast-Lotno-Levelno"@en ;
    skos:topConceptOf cs: .

:LOC-STN-STS-NOL-LOT-LVN-PPC a skos:Concept ;
    dcterms:identifier "LOC-STN-STS-NOL-LOT-LVN-PPC"^^xsd:token ;
    status:status iso19153:original ;
    rdfs:isDefinedBy cs: ;
    skos:definition "Change To Locality Name, Street Name, Street Suffix, Number Last, Lot Number, Level Number And Primary Postcode"@en ;
    skos:inScheme cs: ;
    skos:prefLabel "Locality-Stname-Stsuffix-Nolast-Lotno-Levelno-Postcode"@en ;
    skos:topConceptOf cs: .

:LOC-STN-STS-NOL-LOT-PPC a skos:Concept ;
    dcterms:identifier "LOC-STN-STS-NOL-LOT-PPC"^^xsd:token ;
    status:status iso19153:original ;
    rdfs:isDefinedBy cs: ;
    skos:definition "Change To Locality Name, Street Name, Street Suffix, Number Last, Lot Number And Primary Postcode"@en ;
    skos:inScheme cs: ;
    skos:prefLabel "Locality-Stname-Stsuffix-Nolast-Lotno-Postcode"@en ;
    skos:topConceptOf cs: .

:LOC-STN-STS-NOL-LVN a skos:Concept ;
    dcterms:identifier "LOC-STN-STS-NOL-LVN"^^xsd:token ;
    status:status iso19153:original ;
    rdfs:isDefinedBy cs: ;
    skos:definition "Change To Locality Name, Street Name, Street Suffix, Number Last And Level Number"@en ;
    skos:inScheme cs: ;
    skos:prefLabel "Locality-Stname-Stsuffix-Nolast-Levelno"@en ;
    skos:topConceptOf cs: .

:LOC-STN-STS-NOL-LVN-PPC a skos:Concept ;
    dcterms:identifier "LOC-STN-STS-NOL-LVN-PPC"^^xsd:token ;
    status:status iso19153:original ;
    rdfs:isDefinedBy cs: ;
    skos:definition "Change To Locality Name, Street Name, Street Suffix, Number Last, Level Number And Primary Postcode"@en ;
    skos:inScheme cs: ;
    skos:prefLabel "Locality-Stname-Stsuffix-Nolast-Levelno-Postcode"@en ;
    skos:topConceptOf cs: .

:LOC-STN-STS-NOL-PPC a skos:Concept ;
    dcterms:identifier "LOC-STN-STS-NOL-PPC"^^xsd:token ;
    status:status iso19153:original ;
    rdfs:isDefinedBy cs: ;
    skos:definition "Change To Locality Name, Street Name, Street Suffix, Number Last And Primary Postcode"@en ;
    skos:inScheme cs: ;
    skos:prefLabel "Locality-Stname-Stsuffix-Nolast-Postcode"@en ;
    skos:topConceptOf cs: .

:LOC-STN-STS-PPC a skos:Concept ;
    dcterms:identifier "LOC-STN-STS-PPC"^^xsd:token ;
    status:status iso19153:original ;
    rdfs:isDefinedBy cs: ;
    skos:definition "Change To Locality Name, Street Name, Street Suffix And Primary Postcode"@en ;
    skos:inScheme cs: ;
    skos:prefLabel "Locality-Stname-Stsuffix-Postcode"@en ;
    skos:topConceptOf cs: .

:LOC-STN-STT a skos:Concept ;
    dcterms:identifier "LOC-STN-STT"^^xsd:token ;
    status:status iso19153:original ;
    rdfs:isDefinedBy cs: ;
    skos:definition "Change To Locality Name, Street Name And Street Type"@en ;
    skos:inScheme cs: ;
    skos:prefLabel "Locality-Stname-Sttype"@en ;
    skos:topConceptOf cs: .

:LOC-STN-STT-LOT a skos:Concept ;
    dcterms:identifier "LOC-STN-STT-LOT"^^xsd:token ;
    status:status iso19153:original ;
    rdfs:isDefinedBy cs: ;
    skos:definition "Change To Locality Name, Street Name, Street Type And Lot Number"@en ;
    skos:inScheme cs: ;
    skos:prefLabel "Locality-Stname-Sttype-Lotno"@en ;
    skos:topConceptOf cs: .

:LOC-STN-STT-LOT-LVN a skos:Concept ;
    dcterms:identifier "LOC-STN-STT-LOT-LVN"^^xsd:token ;
    status:status iso19153:original ;
    rdfs:isDefinedBy cs: ;
    skos:definition "Change To Locality Name, Street Name, Street Type, Lot Number And Level Number"@en ;
    skos:inScheme cs: ;
    skos:prefLabel "Locality-Stname-Sttype-Lotno-Levelno"@en ;
    skos:topConceptOf cs: .

:LOC-STN-STT-LOT-LVN-PPC a skos:Concept ;
    dcterms:identifier "LOC-STN-STT-LOT-LVN-PPC"^^xsd:token ;
    status:status iso19153:original ;
    rdfs:isDefinedBy cs: ;
    skos:definition "Change To Locality Name, Street Name, Street Type, Lot Number, Level Number And Primary Postcode"@en ;
    skos:inScheme cs: ;
    skos:prefLabel "Locality-Stname-Sttype-Lotno-Levelno-Postcode"@en ;
    skos:topConceptOf cs: .

:LOC-STN-STT-LOT-PPC a skos:Concept ;
    dcterms:identifier "LOC-STN-STT-LOT-PPC"^^xsd:token ;
    status:status iso19153:original ;
    rdfs:isDefinedBy cs: ;
    skos:definition "Change To Locality Name, Street Name, Street Type, Lot Number And Primary Postcode"@en ;
    skos:inScheme cs: ;
    skos:prefLabel "Locality-Stname-Sttype-Lotno-Postcode"@en ;
    skos:topConceptOf cs: .

:LOC-STN-STT-LVN a skos:Concept ;
    dcterms:identifier "LOC-STN-STT-LVN"^^xsd:token ;
    status:status iso19153:original ;
    rdfs:isDefinedBy cs: ;
    skos:definition "Change To Locality Name, Street Name, Street Type And Level Number"@en ;
    skos:inScheme cs: ;
    skos:prefLabel "Locality-Stname-Sttype-Levelno"@en ;
    skos:topConceptOf cs: .

:LOC-STN-STT-LVN-PPC a skos:Concept ;
    dcterms:identifier "LOC-STN-STT-LVN-PPC"^^xsd:token ;
    status:status iso19153:original ;
    rdfs:isDefinedBy cs: ;
    skos:definition "Change To Locality Name, Street Name, Street Type, Level Number And Primary Postcode"@en ;
    skos:inScheme cs: ;
    skos:prefLabel "Locality-Stname-Sttype-Levelno-Postcode"@en ;
    skos:topConceptOf cs: .

:LOC-STN-STT-NOF a skos:Concept ;
    dcterms:identifier "LOC-STN-STT-NOF"^^xsd:token ;
    status:status iso19153:original ;
    rdfs:isDefinedBy cs: ;
    skos:definition "Change To Locality Name, Street Name, Street Type And Number First"@en ;
    skos:inScheme cs: ;
    skos:prefLabel "Locality-Stname-Sttype-Nofirst"@en ;
    skos:topConceptOf cs: .

:LOC-STN-STT-NOF-LOT a skos:Concept ;
    dcterms:identifier "LOC-STN-STT-NOF-LOT"^^xsd:token ;
    status:status iso19153:original ;
    rdfs:isDefinedBy cs: ;
    skos:definition "Change To Locality Name, Street Name, Street Type, Number First And Lot Number"@en ;
    skos:inScheme cs: ;
    skos:prefLabel "Locality-Stname-Sttype-Nofirst-Lotno"@en ;
    skos:topConceptOf cs: .

:LOC-STN-STT-NOF-LOT-LVN a skos:Concept ;
    dcterms:identifier "LOC-STN-STT-NOF-LOT-LVN"^^xsd:token ;
    status:status iso19153:original ;
    rdfs:isDefinedBy cs: ;
    skos:definition "Change To Locality Name, Street Name, Street Type, Number First, Lot Number And Level Number"@en ;
    skos:inScheme cs: ;
    skos:prefLabel "Locality-Stname-Sttype-Nofirst-Lotno-Levelno"@en ;
    skos:topConceptOf cs: .

:LOC-STN-STT-NOF-LOT-LVN-PPC a skos:Concept ;
    dcterms:identifier "LOC-STN-STT-NOF-LOT-LVN-PPC"^^xsd:token ;
    status:status iso19153:original ;
    rdfs:isDefinedBy cs: ;
    skos:definition "Change To Locality Name, Street Name, Street Type, Number First, Lot Number, Level Number And Primary Postcode"@en ;
    skos:inScheme cs: ;
    skos:prefLabel "Locality-Stname-Sttype-Nofirst-Lotno-Levelno-Postcode"@en ;
    skos:topConceptOf cs: .

:LOC-STN-STT-NOF-LOT-PPC a skos:Concept ;
    dcterms:identifier "LOC-STN-STT-NOF-LOT-PPC"^^xsd:token ;
    status:status iso19153:original ;
    rdfs:isDefinedBy cs: ;
    skos:definition "Change To Locality Name, Street Name, Street Type, Number First, Lot Number And Primary Postcode"@en ;
    skos:inScheme cs: ;
    skos:prefLabel "Locality-Stname-Sttype-Nofirst-Lotno-Postcode"@en ;
    skos:topConceptOf cs: .

:LOC-STN-STT-NOF-LVN a skos:Concept ;
    dcterms:identifier "LOC-STN-STT-NOF-LVN"^^xsd:token ;
    status:status iso19153:original ;
    rdfs:isDefinedBy cs: ;
    skos:definition "Change To Locality Name, Street Name, Street Type, Number First And Level Number"@en ;
    skos:inScheme cs: ;
    skos:prefLabel "Locality-Stname-Sttype-Nofirst-Levelno"@en ;
    skos:topConceptOf cs: .

:LOC-STN-STT-NOF-LVN-PPC a skos:Concept ;
    dcterms:identifier "LOC-STN-STT-NOF-LVN-PPC"^^xsd:token ;
    status:status iso19153:original ;
    rdfs:isDefinedBy cs: ;
    skos:definition "Change To Locality Name, Street Name, Street Type, Number First, Level Number And Primary Postcode"@en ;
    skos:inScheme cs: ;
    skos:prefLabel "Locality-Stname-Sttype-Nofirst-Levelno-Postcode"@en ;
    skos:topConceptOf cs: .

:LOC-STN-STT-NOF-NOL a skos:Concept ;
    dcterms:identifier "LOC-STN-STT-NOF-NOL"^^xsd:token ;
    status:status iso19153:original ;
    rdfs:isDefinedBy cs: ;
    skos:definition "Change To Locality Name, Street Name, Street Type, Number First And Number Last"@en ;
    skos:inScheme cs: ;
    skos:prefLabel "Locality-Stname-Sttype-Nofirst-Nolast"@en ;
    skos:topConceptOf cs: .

:LOC-STN-STT-NOF-NOL-LOT a skos:Concept ;
    dcterms:identifier "LOC-STN-STT-NOF-NOL-LOT"^^xsd:token ;
    status:status iso19153:original ;
    rdfs:isDefinedBy cs: ;
    skos:definition "Change To Locality Name, Street Name, Street Type, Number First, Number Last And Lot Number"@en ;
    skos:inScheme cs: ;
    skos:prefLabel "Locality-Stname-Sttype-Nofirst-Nolast-Lotno"@en ;
    skos:topConceptOf cs: .

:LOC-STN-STT-NOF-NOL-LOT-LVN a skos:Concept ;
    dcterms:identifier "LOC-STN-STT-NOF-NOL-LOT-LVN"^^xsd:token ;
    status:status iso19153:original ;
    rdfs:isDefinedBy cs: ;
    skos:definition "Change To Locality Name, Street Name, Street Type, Number First, Number Last, Lot Number And Level Number"@en ;
    skos:inScheme cs: ;
    skos:prefLabel "Locality-Stname-Sttype-Nofirst-Nolast-Lotno-Levelno"@en ;
    skos:topConceptOf cs: .

:LOC-STN-STT-NOF-NOL-LOT-LVN-PPC a skos:Concept ;
    dcterms:identifier "LOC-STN-STT-NOF-NOL-LOT-LVN-PPC"^^xsd:token ;
    status:status iso19153:original ;
    rdfs:isDefinedBy cs: ;
    skos:definition "Change To Locality Name, Street Name, Street Type, Number First, Number Last, Lot Number, Level Number And Primary Postcode"@en ;
    skos:inScheme cs: ;
    skos:prefLabel "Locality-Stname-Sttype-Nofirst-Nolast-Lotno-Levelno-Postcode"@en ;
    skos:topConceptOf cs: .

:LOC-STN-STT-NOF-NOL-LOT-PPC a skos:Concept ;
    dcterms:identifier "LOC-STN-STT-NOF-NOL-LOT-PPC"^^xsd:token ;
    status:status iso19153:original ;
    rdfs:isDefinedBy cs: ;
    skos:definition "Change To Locality Name, Street Name, Street Type, Number First, Number Last, Lot Number And Primary Postcode"@en ;
    skos:inScheme cs: ;
    skos:prefLabel "Locality-Stname-Sttype-Nofirst-Nolast-Lotno-Postcode"@en ;
    skos:topConceptOf cs: .

:LOC-STN-STT-NOF-NOL-LVN a skos:Concept ;
    dcterms:identifier "LOC-STN-STT-NOF-NOL-LVN"^^xsd:token ;
    status:status iso19153:original ;
    rdfs:isDefinedBy cs: ;
    skos:definition "Change To Locality Name, Street Name, Street Type, Number First, Number Last And Level Number"@en ;
    skos:inScheme cs: ;
    skos:prefLabel "Locality-Stname-Sttype-Nofirst-Nolast-Levelno"@en ;
    skos:topConceptOf cs: .

:LOC-STN-STT-NOF-NOL-LVN-PPC a skos:Concept ;
    dcterms:identifier "LOC-STN-STT-NOF-NOL-LVN-PPC"^^xsd:token ;
    status:status iso19153:original ;
    rdfs:isDefinedBy cs: ;
    skos:definition "Change To Locality Name, Street Name, Street Type, Number First, Number Last, Level Number And Primary Postcode"@en ;
    skos:inScheme cs: ;
    skos:prefLabel "Locality-Stname-Sttype-Nofirst-Nolast-Levelno-Postcode"@en ;
    skos:topConceptOf cs: .

:LOC-STN-STT-NOF-NOL-PPC a skos:Concept ;
    dcterms:identifier "LOC-STN-STT-NOF-NOL-PPC"^^xsd:token ;
    status:status iso19153:original ;
    rdfs:isDefinedBy cs: ;
    skos:definition "Change To Locality Name, Street Name, Street Type, Number First, Number Last And Primary Postcode"@en ;
    skos:inScheme cs: ;
    skos:prefLabel "Locality-Stname-Sttype-Nofirst-Nolast-Postcode"@en ;
    skos:topConceptOf cs: .

:LOC-STN-STT-NOF-PPC a skos:Concept ;
    dcterms:identifier "LOC-STN-STT-NOF-PPC"^^xsd:token ;
    status:status iso19153:original ;
    rdfs:isDefinedBy cs: ;
    skos:definition "Change To Locality Name, Street Name, Street Type, Number First And Primary Postcode"@en ;
    skos:inScheme cs: ;
    skos:prefLabel "Locality-Stname-Sttype-Nofirst-Postcode"@en ;
    skos:topConceptOf cs: .

:LOC-STN-STT-NOL a skos:Concept ;
    dcterms:identifier "LOC-STN-STT-NOL"^^xsd:token ;
    status:status iso19153:original ;
    rdfs:isDefinedBy cs: ;
    skos:definition "Change To Locality Name, Street Name, Street Type And Number Last"@en ;
    skos:inScheme cs: ;
    skos:prefLabel "Locality-Stname-Sttype-Nolast"@en ;
    skos:topConceptOf cs: .

:LOC-STN-STT-NOL-LOT a skos:Concept ;
    dcterms:identifier "LOC-STN-STT-NOL-LOT"^^xsd:token ;
    status:status iso19153:original ;
    rdfs:isDefinedBy cs: ;
    skos:definition "Change To Locality Name, Street Name, Street Type, Number Last And Lot Number"@en ;
    skos:inScheme cs: ;
    skos:prefLabel "Locality-Stname-Sttype-Nolast-Lotno"@en ;
    skos:topConceptOf cs: .

:LOC-STN-STT-NOL-LOT-LVN a skos:Concept ;
    dcterms:identifier "LOC-STN-STT-NOL-LOT-LVN"^^xsd:token ;
    status:status iso19153:original ;
    rdfs:isDefinedBy cs: ;
    skos:definition "Change To Locality Name, Street Name, Street Type, Number Last, Lot Number And Level Number"@en ;
    skos:inScheme cs: ;
    skos:prefLabel "Locality-Stname-Sttype-Nolast-Lotno-Levelno"@en ;
    skos:topConceptOf cs: .

:LOC-STN-STT-NOL-LOT-LVN-PPC a skos:Concept ;
    dcterms:identifier "LOC-STN-STT-NOL-LOT-LVN-PPC"^^xsd:token ;
    status:status iso19153:original ;
    rdfs:isDefinedBy cs: ;
    skos:definition "Change To Locality Name, Street Name, Street Type, Number Last, Lot Number, Level Number And Primary Postcode"@en ;
    skos:inScheme cs: ;
    skos:prefLabel "Locality-Stname-Sttype-Nolast-Lotno-Levelno-Postcode"@en ;
    skos:topConceptOf cs: .

:LOC-STN-STT-NOL-LOT-PPC a skos:Concept ;
    dcterms:identifier "LOC-STN-STT-NOL-LOT-PPC"^^xsd:token ;
    status:status iso19153:original ;
    rdfs:isDefinedBy cs: ;
    skos:definition "Change To Locality Name, Street Name, Street Type, Number Last, Lot Number And Primary Postcode"@en ;
    skos:inScheme cs: ;
    skos:prefLabel "Locality-Stname-Sttype-Nolast-Lotno-Postcode"@en ;
    skos:topConceptOf cs: .

:LOC-STN-STT-NOL-LVN a skos:Concept ;
    dcterms:identifier "LOC-STN-STT-NOL-LVN"^^xsd:token ;
    status:status iso19153:original ;
    rdfs:isDefinedBy cs: ;
    skos:definition "Change To Locality Name, Street Name, Street Type, Number Last And Level Number"@en ;
    skos:inScheme cs: ;
    skos:prefLabel "Locality-Stname-Sttype-Nolast-Levelno"@en ;
    skos:topConceptOf cs: .

:LOC-STN-STT-NOL-LVN-PPC a skos:Concept ;
    dcterms:identifier "LOC-STN-STT-NOL-LVN-PPC"^^xsd:token ;
    status:status iso19153:original ;
    rdfs:isDefinedBy cs: ;
    skos:definition "Change To Locality Name, Street Name, Street Type, Number Last, Level Number And Primary Postcode"@en ;
    skos:inScheme cs: ;
    skos:prefLabel "Locality-Stname-Sttype-Nolast-Levelno-Postcode"@en ;
    skos:topConceptOf cs: .

:LOC-STN-STT-NOL-PPC a skos:Concept ;
    dcterms:identifier "LOC-STN-STT-NOL-PPC"^^xsd:token ;
    status:status iso19153:original ;
    rdfs:isDefinedBy cs: ;
    skos:definition "Change To Locality Name, Street Name, Street Type, Number Last And Primary Postcode"@en ;
    skos:inScheme cs: ;
    skos:prefLabel "Locality-Stname-Sttype-Nolast-Postcode"@en ;
    skos:topConceptOf cs: .

:LOC-STN-STT-PPC a skos:Concept ;
    dcterms:identifier "LOC-STN-STT-PPC"^^xsd:token ;
    status:status iso19153:original ;
    rdfs:isDefinedBy cs: ;
    skos:definition "Change To Locality Name, Street Name, Street Type And Primary Postcode"@en ;
    skos:inScheme cs: ;
    skos:prefLabel "Locality-Stname-Sttype-Postcode"@en ;
    skos:topConceptOf cs: .

:LOC-STN-STT-STS a skos:Concept ;
    dcterms:identifier "LOC-STN-STT-STS"^^xsd:token ;
    status:status iso19153:original ;
    rdfs:isDefinedBy cs: ;
    skos:definition "Change To Locality Name, Street Name, Street Type And Street Suffix"@en ;
    skos:inScheme cs: ;
    skos:prefLabel "Locality-Stname-Sttype-Stsuffix"@en ;
    skos:topConceptOf cs: .

:LOC-STN-STT-STS-LOT a skos:Concept ;
    dcterms:identifier "LOC-STN-STT-STS-LOT"^^xsd:token ;
    status:status iso19153:original ;
    rdfs:isDefinedBy cs: ;
    skos:definition "Change To Locality Name, Street Name, Street Type, Street Suffix And Lot Number"@en ;
    skos:inScheme cs: ;
    skos:prefLabel "Locality-Stname-Sttype-Stsuffix-Lotno"@en ;
    skos:topConceptOf cs: .

:LOC-STN-STT-STS-LOT-LVN a skos:Concept ;
    dcterms:identifier "LOC-STN-STT-STS-LOT-LVN"^^xsd:token ;
    status:status iso19153:original ;
    rdfs:isDefinedBy cs: ;
    skos:definition "Change To Locality Name, Street Name, Street Type, Street Suffix, Lot Number And Level Number"@en ;
    skos:inScheme cs: ;
    skos:prefLabel "Locality-Stname-Sttype-Stsuffix-Lotno-Levelno"@en ;
    skos:topConceptOf cs: .

:LOC-STN-STT-STS-LOT-LVN-PPC a skos:Concept ;
    dcterms:identifier "LOC-STN-STT-STS-LOT-LVN-PPC"^^xsd:token ;
    status:status iso19153:original ;
    rdfs:isDefinedBy cs: ;
    skos:definition "Change To Locality Name, Street Name, Street Type, Street Suffix, Lot Number, Level Number And Primary Postcode"@en ;
    skos:inScheme cs: ;
    skos:prefLabel "Locality-Stname-Sttype-Stsuffix-Lotno-Levelno-Postcode"@en ;
    skos:topConceptOf cs: .

:LOC-STN-STT-STS-LOT-PPC a skos:Concept ;
    dcterms:identifier "LOC-STN-STT-STS-LOT-PPC"^^xsd:token ;
    status:status iso19153:original ;
    rdfs:isDefinedBy cs: ;
    skos:definition "Change To Locality Name, Street Name, Street Type, Street Suffix, Lot Number And Primary Postcode"@en ;
    skos:inScheme cs: ;
    skos:prefLabel "Locality-Stname-Sttype-Stsuffix-Lotno-Postcode"@en ;
    skos:topConceptOf cs: .

:LOC-STN-STT-STS-LVN a skos:Concept ;
    dcterms:identifier "LOC-STN-STT-STS-LVN"^^xsd:token ;
    status:status iso19153:original ;
    rdfs:isDefinedBy cs: ;
    skos:definition "Change To Locality Name, Street Name, Street Type, Street Suffix And Level Number"@en ;
    skos:inScheme cs: ;
    skos:prefLabel "Locality-Stname-Sttype-Stsuffix-Levelno"@en ;
    skos:topConceptOf cs: .

:LOC-STN-STT-STS-LVN-PPC a skos:Concept ;
    dcterms:identifier "LOC-STN-STT-STS-LVN-PPC"^^xsd:token ;
    status:status iso19153:original ;
    rdfs:isDefinedBy cs: ;
    skos:definition "Change To Locality Name, Street Name, Street Type, Street Suffix, Level Number And Primary Postcode"@en ;
    skos:inScheme cs: ;
    skos:prefLabel "Locality-Stname-Sttype-Stsuffix-Levelno-Postcode"@en ;
    skos:topConceptOf cs: .

:LOC-STN-STT-STS-NOF a skos:Concept ;
    dcterms:identifier "LOC-STN-STT-STS-NOF"^^xsd:token ;
    status:status iso19153:original ;
    rdfs:isDefinedBy cs: ;
    skos:definition "Change To Locality Name, Street Name, Street Type, Street Suffix And Number First"@en ;
    skos:inScheme cs: ;
    skos:prefLabel "Locality-Stname-Sttype-Stsuffix-Nofirst"@en ;
    skos:topConceptOf cs: .

:LOC-STN-STT-STS-NOF-LOT a skos:Concept ;
    dcterms:identifier "LOC-STN-STT-STS-NOF-LOT"^^xsd:token ;
    status:status iso19153:original ;
    rdfs:isDefinedBy cs: ;
    skos:definition "Change To Locality Name, Street Name, Street Type, Street Suffix, Number First And Lot Number"@en ;
    skos:inScheme cs: ;
    skos:prefLabel "Locality-Stname-Sttype-Stsuffix-Nofirst-Lotno"@en ;
    skos:topConceptOf cs: .

:LOC-STN-STT-STS-NOF-LOT-LVN a skos:Concept ;
    dcterms:identifier "LOC-STN-STT-STS-NOF-LOT-LVN"^^xsd:token ;
    status:status iso19153:original ;
    rdfs:isDefinedBy cs: ;
    skos:definition "Change To Locality Name, Street Name, Street Type, Street Suffix, Number First, Lot Number And Level Number"@en ;
    skos:inScheme cs: ;
    skos:prefLabel "Locality-Stname-Sttype-Stsuffix-Nofirst-Lotno-Levelno"@en ;
    skos:topConceptOf cs: .

:LOC-STN-STT-STS-NOF-LOT-LVN-PPC a skos:Concept ;
    dcterms:identifier "LOC-STN-STT-STS-NOF-LOT-LVN-PPC"^^xsd:token ;
    status:status iso19153:original ;
    rdfs:isDefinedBy cs: ;
    skos:definition "Change To Locality Name, Street Name, Street Type, Street Suffix, Number First, Lot Number, Level Number And Primary Postcode"@en ;
    skos:inScheme cs: ;
    skos:prefLabel "Locality-Stname-Sttype-Stsuffix-Nofirst-Lotno-Levelno-Postcode"@en ;
    skos:topConceptOf cs: .

:LOC-STN-STT-STS-NOF-LOT-PPC a skos:Concept ;
    dcterms:identifier "LOC-STN-STT-STS-NOF-LOT-PPC"^^xsd:token ;
    status:status iso19153:original ;
    rdfs:isDefinedBy cs: ;
    skos:definition "Change To Locality Name, Street Name, Street Type, Street Suffix, Number First, Lot Number And Primary Postcode"@en ;
    skos:inScheme cs: ;
    skos:prefLabel "Locality-Stname-Sttype-Stsuffix-Nofirst-Lotno-Postcode"@en ;
    skos:topConceptOf cs: .

:LOC-STN-STT-STS-NOF-LVN a skos:Concept ;
    dcterms:identifier "LOC-STN-STT-STS-NOF-LVN"^^xsd:token ;
    status:status iso19153:original ;
    rdfs:isDefinedBy cs: ;
    skos:definition "Change To Locality Name, Street Name, Street Type, Street Suffix, Number First And Level Number"@en ;
    skos:inScheme cs: ;
    skos:prefLabel "Locality-Stname-Sttype-Stsuffix-Nofirst-Levelno"@en ;
    skos:topConceptOf cs: .

:LOC-STN-STT-STS-NOF-LVN-PPC a skos:Concept ;
    dcterms:identifier "LOC-STN-STT-STS-NOF-LVN-PPC"^^xsd:token ;
    status:status iso19153:original ;
    rdfs:isDefinedBy cs: ;
    skos:definition "Change To Locality Name, Street Name, Street Type, Street Suffix, Number First, Level Number And Primary Postcode"@en ;
    skos:inScheme cs: ;
    skos:prefLabel "Locality-Stname-Sttype-Stsuffix-Nofirst-Levelno-Postcode"@en ;
    skos:topConceptOf cs: .

:LOC-STN-STT-STS-NOF-NOL a skos:Concept ;
    dcterms:identifier "LOC-STN-STT-STS-NOF-NOL"^^xsd:token ;
    status:status iso19153:original ;
    rdfs:isDefinedBy cs: ;
    skos:definition "Change To Locality Name, Street Name, Street Type, Street Suffix, Number First And Number Last"@en ;
    skos:inScheme cs: ;
    skos:prefLabel "Locality-Stname-Sttype-Stsuffix-Nofirst-Nolast"@en ;
    skos:topConceptOf cs: .

:LOC-STN-STT-STS-NOF-NOL-LOT a skos:Concept ;
    dcterms:identifier "LOC-STN-STT-STS-NOF-NOL-LOT"^^xsd:token ;
    status:status iso19153:original ;
    rdfs:isDefinedBy cs: ;
    skos:definition "Change To Locality Name, Street Name, Street Type, Street Suffix, Number First, Number Last And Lot Number"@en ;
    skos:inScheme cs: ;
    skos:prefLabel "Locality-Stname-Sttype-Stsuffix-Nofirst-Nolast-Lotno"@en ;
    skos:topConceptOf cs: .

:LOC-STN-STT-STS-NOF-NOL-LOT-LVN a skos:Concept ;
    dcterms:identifier "LOC-STN-STT-STS-NOF-NOL-LOT-LVN"^^xsd:token ;
    status:status iso19153:original ;
    rdfs:isDefinedBy cs: ;
    skos:definition "Change To Locality Name, Street Name, Street Type, Street Suffix, Number First, Number Last, Lot Number And Level Number"@en ;
    skos:inScheme cs: ;
    skos:prefLabel "Locality-Stname-Sttype-Stsuffix-Nofirst-Nolast-Lotno-Levelno"@en ;
    skos:topConceptOf cs: .

:LOC-STN-STT-STS-NOF-NOL-LOT-LVN-PPC a skos:Concept ;
    dcterms:identifier "LOC-STN-STT-STS-NOF-NOL-LOT-LVN-PPC"^^xsd:token ;
    status:status iso19153:original ;
    rdfs:isDefinedBy cs: ;
    skos:definition "Change To Locality Name, Street Name, Street Type, Street Suffix, Number First, Number Last, Lot Number, Level Number And Primary Postcode"@en ;
    skos:inScheme cs: ;
    skos:prefLabel "Locality-Stname-Sttype-Stsuffix-Nofirst-Nolast-Lotno-Levelno-Postcode"@en ;
    skos:topConceptOf cs: .

:LOC-STN-STT-STS-NOF-NOL-LOT-PPC a skos:Concept ;
    dcterms:identifier "LOC-STN-STT-STS-NOF-NOL-LOT-PPC"^^xsd:token ;
    status:status iso19153:original ;
    rdfs:isDefinedBy cs: ;
    skos:definition "Change To Locality Name, Street Name, Street Type, Street Suffix, Number First, Number Last, Lot Number And Primary Postcode"@en ;
    skos:inScheme cs: ;
    skos:prefLabel "Locality-Stname-Sttype-Stsuffix-Nofirst-Nolast-Lotno-Postcode"@en ;
    skos:topConceptOf cs: .

:LOC-STN-STT-STS-NOF-NOL-LVN a skos:Concept ;
    dcterms:identifier "LOC-STN-STT-STS-NOF-NOL-LVN"^^xsd:token ;
    status:status iso19153:original ;
    rdfs:isDefinedBy cs: ;
    skos:definition "Change To Locality Name, Street Name, Street Type, Street Suffix, Number First, Number Last And Level Number"@en ;
    skos:inScheme cs: ;
    skos:prefLabel "Locality-Stname-Sttype-Stsuffix-Nofirst-Nolast-Levelno"@en ;
    skos:topConceptOf cs: .

:LOC-STN-STT-STS-NOF-NOL-LVN-PPC a skos:Concept ;
    dcterms:identifier "LOC-STN-STT-STS-NOF-NOL-LVN-PPC"^^xsd:token ;
    status:status iso19153:original ;
    rdfs:isDefinedBy cs: ;
    skos:definition "Change To Locality Name, Street Name, Street Type, Street Suffix, Number First, Number Last, Level Number And Primary Postcode"@en ;
    skos:inScheme cs: ;
    skos:prefLabel "Locality-Stname-Sttype-Stsuffix-Nofirst-Nolast-Levelno-Postcode"@en ;
    skos:topConceptOf cs: .

:LOC-STN-STT-STS-NOF-NOL-PPC a skos:Concept ;
    dcterms:identifier "LOC-STN-STT-STS-NOF-NOL-PPC"^^xsd:token ;
    status:status iso19153:original ;
    rdfs:isDefinedBy cs: ;
    skos:definition "Change To Locality Name, Street Name, Street Type, Street Suffix, Number First, Number Last And Primary Postcode"@en ;
    skos:inScheme cs: ;
    skos:prefLabel "Locality-Stname-Sttype-Stsuffix-Nofirst-Nolast-Postcode"@en ;
    skos:topConceptOf cs: .

:LOC-STN-STT-STS-NOF-PPC a skos:Concept ;
    dcterms:identifier "LOC-STN-STT-STS-NOF-PPC"^^xsd:token ;
    status:status iso19153:original ;
    rdfs:isDefinedBy cs: ;
    skos:definition "Change To Locality Name, Street Name, Street Type, Street Suffix, Number First And Primary Postcode"@en ;
    skos:inScheme cs: ;
    skos:prefLabel "Locality-Stname-Sttype-Stsuffix-Nofirst-Postcode"@en ;
    skos:topConceptOf cs: .

:LOC-STN-STT-STS-NOL a skos:Concept ;
    dcterms:identifier "LOC-STN-STT-STS-NOL"^^xsd:token ;
    status:status iso19153:original ;
    rdfs:isDefinedBy cs: ;
    skos:definition "Change To Locality Name, Street Name, Street Type, Street Suffix And Number Last"@en ;
    skos:inScheme cs: ;
    skos:prefLabel "Locality-Stname-Sttype-Stsuffix-Nolast"@en ;
    skos:topConceptOf cs: .

:LOC-STN-STT-STS-NOL-LOT a skos:Concept ;
    dcterms:identifier "LOC-STN-STT-STS-NOL-LOT"^^xsd:token ;
    status:status iso19153:original ;
    rdfs:isDefinedBy cs: ;
    skos:definition "Change To Locality Name, Street Name, Street Type, Street Suffix, Number Last And Lot Number"@en ;
    skos:inScheme cs: ;
    skos:prefLabel "Locality-Stname-Sttype-Stsuffix-Nolast-Lotno"@en ;
    skos:topConceptOf cs: .

:LOC-STN-STT-STS-NOL-LOT-LVN a skos:Concept ;
    dcterms:identifier "LOC-STN-STT-STS-NOL-LOT-LVN"^^xsd:token ;
    status:status iso19153:original ;
    rdfs:isDefinedBy cs: ;
    skos:definition "Change To Locality Name, Street Name, Street Type, Street Suffix, Number Last, Lot Number And Level Number"@en ;
    skos:inScheme cs: ;
    skos:prefLabel "Locality-Stname-Sttype-Stsuffix-Nolast-Lotno-Levelno"@en ;
    skos:topConceptOf cs: .

:LOC-STN-STT-STS-NOL-LOT-LVN-PPC a skos:Concept ;
    dcterms:identifier "LOC-STN-STT-STS-NOL-LOT-LVN-PPC"^^xsd:token ;
    status:status iso19153:original ;
    rdfs:isDefinedBy cs: ;
    skos:definition "Change To Locality Name, Street Name, Street Type, Street Suffix, Number Last, Lot Number, Level Number And Primary Postcode"@en ;
    skos:inScheme cs: ;
    skos:prefLabel "Locality-Stname-Sttype-Stsuffix-Nolast-Lotno-Levelno-Postcode"@en ;
    skos:topConceptOf cs: .

:LOC-STN-STT-STS-NOL-LOT-PPC a skos:Concept ;
    dcterms:identifier "LOC-STN-STT-STS-NOL-LOT-PPC"^^xsd:token ;
    status:status iso19153:original ;
    rdfs:isDefinedBy cs: ;
    skos:definition "Change To Locality Name, Street Name, Street Type, Street Suffix, Number Last, Lot Number And Primary Postcode"@en ;
    skos:inScheme cs: ;
    skos:prefLabel "Locality-Stname-Sttype-Stsuffix-Nolast-Lotno-Postcode"@en ;
    skos:topConceptOf cs: .

:LOC-STN-STT-STS-NOL-LVN a skos:Concept ;
    dcterms:identifier "LOC-STN-STT-STS-NOL-LVN"^^xsd:token ;
    status:status iso19153:original ;
    rdfs:isDefinedBy cs: ;
    skos:definition "Change To Locality Name, Street Name, Street Type, Street Suffix, Number Last And Level Number"@en ;
    skos:inScheme cs: ;
    skos:prefLabel "Locality-Stname-Sttype-Stsuffix-Nolast-Levelno"@en ;
    skos:topConceptOf cs: .

:LOC-STN-STT-STS-NOL-LVN-PPC a skos:Concept ;
    dcterms:identifier "LOC-STN-STT-STS-NOL-LVN-PPC"^^xsd:token ;
    status:status iso19153:original ;
    rdfs:isDefinedBy cs: ;
    skos:definition "Change To Locality Name, Street Name, Street Type, Street Suffix, Number Last, Level Number And Primary Postcode"@en ;
    skos:inScheme cs: ;
    skos:prefLabel "Locality-Stname-Sttype-Stsuffix-Nolast-Levelno-Postcode"@en ;
    skos:topConceptOf cs: .

:LOC-STN-STT-STS-NOL-PPC a skos:Concept ;
    dcterms:identifier "LOC-STN-STT-STS-NOL-PPC"^^xsd:token ;
    status:status iso19153:original ;
    rdfs:isDefinedBy cs: ;
    skos:definition "Change To Locality Name, Street Name, Street Type, Street Suffix, Number Last And Primary Postcode"@en ;
    skos:inScheme cs: ;
    skos:prefLabel "Locality-Stname-Sttype-Stsuffix-Nolast-Postcode"@en ;
    skos:topConceptOf cs: .

:LOC-STN-STT-STS-PPC a skos:Concept ;
    dcterms:identifier "LOC-STN-STT-STS-PPC"^^xsd:token ;
    status:status iso19153:original ;
    rdfs:isDefinedBy cs: ;
    skos:definition "Change To Locality Name, Street Name, Street Type, Street Suffix And Primary Postcode"@en ;
    skos:inScheme cs: ;
    skos:prefLabel "Locality-Stname-Sttype-Stsuffix-Postcode"@en ;
    skos:topConceptOf cs: .

:LOC-STS a skos:Concept ;
    dcterms:identifier "LOC-STS"^^xsd:token ;
    status:status iso19153:original ;
    rdfs:isDefinedBy cs: ;
    skos:definition "Change To Locality Name And Street Suffix"@en ;
    skos:inScheme cs: ;
    skos:prefLabel "Locality-Stsuffix"@en ;
    skos:topConceptOf cs: .

:LOC-STS-LOT a skos:Concept ;
    dcterms:identifier "LOC-STS-LOT"^^xsd:token ;
    status:status iso19153:original ;
    rdfs:isDefinedBy cs: ;
    skos:definition "Change To Locality Name, Street Suffix And Lot Number"@en ;
    skos:inScheme cs: ;
    skos:prefLabel "Locality-Stsuffix-Lotno"@en ;
    skos:topConceptOf cs: .

:LOC-STS-LOT-LVN a skos:Concept ;
    dcterms:identifier "LOC-STS-LOT-LVN"^^xsd:token ;
    status:status iso19153:original ;
    rdfs:isDefinedBy cs: ;
    skos:definition "Change To Locality Name, Street Suffix, Lot Number And Level Number"@en ;
    skos:inScheme cs: ;
    skos:prefLabel "Locality-Stsuffix-Lotno-Levelno"@en ;
    skos:topConceptOf cs: .

:LOC-STS-LOT-LVN-PPC a skos:Concept ;
    dcterms:identifier "LOC-STS-LOT-LVN-PPC"^^xsd:token ;
    status:status iso19153:original ;
    rdfs:isDefinedBy cs: ;
    skos:definition "Change To Locality Name, Street Suffix, Lot Number, Level Number And Primary Postcode"@en ;
    skos:inScheme cs: ;
    skos:prefLabel "Locality-Stsuffix-Lotno-Levelno-Postcode"@en ;
    skos:topConceptOf cs: .

:LOC-STS-LOT-PPC a skos:Concept ;
    dcterms:identifier "LOC-STS-LOT-PPC"^^xsd:token ;
    status:status iso19153:original ;
    rdfs:isDefinedBy cs: ;
    skos:definition "Change To Locality Name, Street Suffix, Lot Number And Primary Postcode"@en ;
    skos:inScheme cs: ;
    skos:prefLabel "Locality-Stsuffix-Lotno-Postcode"@en ;
    skos:topConceptOf cs: .

:LOC-STS-LVN a skos:Concept ;
    dcterms:identifier "LOC-STS-LVN"^^xsd:token ;
    status:status iso19153:original ;
    rdfs:isDefinedBy cs: ;
    skos:definition "Change To Locality Name, Street Suffix And Level Number"@en ;
    skos:inScheme cs: ;
    skos:prefLabel "Locality-Stsuffix-Levelno"@en ;
    skos:topConceptOf cs: .

:LOC-STS-LVN-PPC a skos:Concept ;
    dcterms:identifier "LOC-STS-LVN-PPC"^^xsd:token ;
    status:status iso19153:original ;
    rdfs:isDefinedBy cs: ;
    skos:definition "Change To Locality Name, Street Suffix, Level Number And Primary Postcode"@en ;
    skos:inScheme cs: ;
    skos:prefLabel "Locality-Stsuffix-Levelno-Postcode"@en ;
    skos:topConceptOf cs: .

:LOC-STS-NOF a skos:Concept ;
    dcterms:identifier "LOC-STS-NOF"^^xsd:token ;
    status:status iso19153:original ;
    rdfs:isDefinedBy cs: ;
    skos:definition "Change To Locality Name, Street Suffix And Number First"@en ;
    skos:inScheme cs: ;
    skos:prefLabel "Locality-Stsuffix-Nofirst"@en ;
    skos:topConceptOf cs: .

:LOC-STS-NOF-LOT a skos:Concept ;
    dcterms:identifier "LOC-STS-NOF-LOT"^^xsd:token ;
    status:status iso19153:original ;
    rdfs:isDefinedBy cs: ;
    skos:definition "Change To Locality Name, Street Suffix, Number First And Lot Number"@en ;
    skos:inScheme cs: ;
    skos:prefLabel "Locality-Stsuffix-Nofirst-Lotno"@en ;
    skos:topConceptOf cs: .

:LOC-STS-NOF-LOT-LVN a skos:Concept ;
    dcterms:identifier "LOC-STS-NOF-LOT-LVN"^^xsd:token ;
    status:status iso19153:original ;
    rdfs:isDefinedBy cs: ;
    skos:definition "Change To Locality Name, Street Suffix, Number First, Lot Number And Level Number"@en ;
    skos:inScheme cs: ;
    skos:prefLabel "Locality-Stsuffix-Nofirst-Lotno-Levelno"@en ;
    skos:topConceptOf cs: .

:LOC-STS-NOF-LOT-LVN-PPC a skos:Concept ;
    dcterms:identifier "LOC-STS-NOF-LOT-LVN-PPC"^^xsd:token ;
    status:status iso19153:original ;
    rdfs:isDefinedBy cs: ;
    skos:definition "Change To Locality Name, Street Suffix, Number First, Lot Number, Level Number And Primary Postcode"@en ;
    skos:inScheme cs: ;
    skos:prefLabel "Locality-Stsuffix-Nofirst-Lotno-Levelno-Postcode"@en ;
    skos:topConceptOf cs: .

:LOC-STS-NOF-LOT-PPC a skos:Concept ;
    dcterms:identifier "LOC-STS-NOF-LOT-PPC"^^xsd:token ;
    status:status iso19153:original ;
    rdfs:isDefinedBy cs: ;
    skos:definition "Change To Locality Name, Street Suffix, Number First, Lot Number And Primary Postcode"@en ;
    skos:inScheme cs: ;
    skos:prefLabel "Locality-Stsuffix-Nofirst-Lotno-Postcode"@en ;
    skos:topConceptOf cs: .

:LOC-STS-NOF-LVN a skos:Concept ;
    dcterms:identifier "LOC-STS-NOF-LVN"^^xsd:token ;
    status:status iso19153:original ;
    rdfs:isDefinedBy cs: ;
    skos:definition "Change To Locality Name, Street Suffix, Number First And Level Number"@en ;
    skos:inScheme cs: ;
    skos:prefLabel "Locality-Stsuffix-Nofirst-Levelno"@en ;
    skos:topConceptOf cs: .

:LOC-STS-NOF-LVN-PPC a skos:Concept ;
    dcterms:identifier "LOC-STS-NOF-LVN-PPC"^^xsd:token ;
    status:status iso19153:original ;
    rdfs:isDefinedBy cs: ;
    skos:definition "Change To Locality Name, Street Suffix, Number First, Level Number And Primary Postcode"@en ;
    skos:inScheme cs: ;
    skos:prefLabel "Locality-Stsuffix-Nofirst-Levelno-Postcode"@en ;
    skos:topConceptOf cs: .

:LOC-STS-NOF-NOL a skos:Concept ;
    dcterms:identifier "LOC-STS-NOF-NOL"^^xsd:token ;
    status:status iso19153:original ;
    rdfs:isDefinedBy cs: ;
    skos:definition "Change To Locality Name, Street Suffix, Number First And Number Last"@en ;
    skos:inScheme cs: ;
    skos:prefLabel "Locality-Stsuffix-Nofirst-Nolast"@en ;
    skos:topConceptOf cs: .

:LOC-STS-NOF-NOL-LOT a skos:Concept ;
    dcterms:identifier "LOC-STS-NOF-NOL-LOT"^^xsd:token ;
    status:status iso19153:original ;
    rdfs:isDefinedBy cs: ;
    skos:definition "Change To Locality Name, Street Suffix, Number First, Number Last And Lot Number"@en ;
    skos:inScheme cs: ;
    skos:prefLabel "Locality-Stsuffix-Nofirst-Nolast-Lotno"@en ;
    skos:topConceptOf cs: .

:LOC-STS-NOF-NOL-LOT-LVN a skos:Concept ;
    dcterms:identifier "LOC-STS-NOF-NOL-LOT-LVN"^^xsd:token ;
    status:status iso19153:original ;
    rdfs:isDefinedBy cs: ;
    skos:definition "Change To Locality Name, Street Suffix, Number First, Number Last, Lot Number And Level Number"@en ;
    skos:inScheme cs: ;
    skos:prefLabel "Locality-Stsuffix-Nofirst-Nolast-Lotno-Levelno"@en ;
    skos:topConceptOf cs: .

:LOC-STS-NOF-NOL-LOT-LVN-PPC a skos:Concept ;
    dcterms:identifier "LOC-STS-NOF-NOL-LOT-LVN-PPC"^^xsd:token ;
    status:status iso19153:original ;
    rdfs:isDefinedBy cs: ;
    skos:definition "Change To Locality Name, Street Suffix, Number First, Number Last, Lot Number, Level Number And Primary Postcode"@en ;
    skos:inScheme cs: ;
    skos:prefLabel "Locality-Stsuffix-Nofirst-Nolast-Lotno-Levelno-Postcode"@en ;
    skos:topConceptOf cs: .

:LOC-STS-NOF-NOL-LOT-PPC a skos:Concept ;
    dcterms:identifier "LOC-STS-NOF-NOL-LOT-PPC"^^xsd:token ;
    status:status iso19153:original ;
    rdfs:isDefinedBy cs: ;
    skos:definition "Change To Locality Name, Street Suffix, Number First, Number Last, Lot Number And Primary Postcode"@en ;
    skos:inScheme cs: ;
    skos:prefLabel "Locality-Stsuffix-Nofirst-Nolast-Lotno-Postcode"@en ;
    skos:topConceptOf cs: .

:LOC-STS-NOF-NOL-LVN a skos:Concept ;
    dcterms:identifier "LOC-STS-NOF-NOL-LVN"^^xsd:token ;
    status:status iso19153:original ;
    rdfs:isDefinedBy cs: ;
    skos:definition "Change To Locality Name, Street Suffix, Number First, Number Last And Level Number"@en ;
    skos:inScheme cs: ;
    skos:prefLabel "Locality-Stsuffix-Nofirst-Nolast-Levelno"@en ;
    skos:topConceptOf cs: .

:LOC-STS-NOF-NOL-LVN-PPC a skos:Concept ;
    dcterms:identifier "LOC-STS-NOF-NOL-LVN-PPC"^^xsd:token ;
    status:status iso19153:original ;
    rdfs:isDefinedBy cs: ;
    skos:definition "Change To Locality Name, Street Suffix, Number First, Number Last, Level Number And Primary Postcode"@en ;
    skos:inScheme cs: ;
    skos:prefLabel "Locality-Stsuffix-Nofirst-Nolast-Levelno-Postcode"@en ;
    skos:topConceptOf cs: .

:LOC-STS-NOF-NOL-PPC a skos:Concept ;
    dcterms:identifier "LOC-STS-NOF-NOL-PPC"^^xsd:token ;
    status:status iso19153:original ;
    rdfs:isDefinedBy cs: ;
    skos:definition "Change To Locality Name, Street Suffix, Number First, Number Last And Primary Postcode"@en ;
    skos:inScheme cs: ;
    skos:prefLabel "Locality-Stsuffix-Nofirst-Nolast-Postcode"@en ;
    skos:topConceptOf cs: .

:LOC-STS-NOF-PPC a skos:Concept ;
    dcterms:identifier "LOC-STS-NOF-PPC"^^xsd:token ;
    status:status iso19153:original ;
    rdfs:isDefinedBy cs: ;
    skos:definition "Change To Locality Name, Street Suffix, Number First And Primary Postcode"@en ;
    skos:inScheme cs: ;
    skos:prefLabel "Locality-Stsuffix-Nofirst-Postcode"@en ;
    skos:topConceptOf cs: .

:LOC-STS-NOL a skos:Concept ;
    dcterms:identifier "LOC-STS-NOL"^^xsd:token ;
    status:status iso19153:original ;
    rdfs:isDefinedBy cs: ;
    skos:definition "Change To Locality Name, Street Suffix And Number Last"@en ;
    skos:inScheme cs: ;
    skos:prefLabel "Locality-Stsuffix-Nolast"@en ;
    skos:topConceptOf cs: .

:LOC-STS-NOL-LOT a skos:Concept ;
    dcterms:identifier "LOC-STS-NOL-LOT"^^xsd:token ;
    status:status iso19153:original ;
    rdfs:isDefinedBy cs: ;
    skos:definition "Change To Locality Name, Street Suffix, Number Last And Lot Number"@en ;
    skos:inScheme cs: ;
    skos:prefLabel "Locality-Stsuffix-Nolast-Lotno"@en ;
    skos:topConceptOf cs: .

:LOC-STS-NOL-LOT-LVN a skos:Concept ;
    dcterms:identifier "LOC-STS-NOL-LOT-LVN"^^xsd:token ;
    status:status iso19153:original ;
    rdfs:isDefinedBy cs: ;
    skos:definition "Change To Locality Name, Street Suffix, Number Last, Lot Number And Level Number"@en ;
    skos:inScheme cs: ;
    skos:prefLabel "Locality-Stsuffix-Nolast-Lotno-Levelno"@en ;
    skos:topConceptOf cs: .

:LOC-STS-NOL-LOT-LVN-PPC a skos:Concept ;
    dcterms:identifier "LOC-STS-NOL-LOT-LVN-PPC"^^xsd:token ;
    status:status iso19153:original ;
    rdfs:isDefinedBy cs: ;
    skos:definition "Change To Locality Name, Street Suffix, Number Last, Lot Number, Level Number And Primary Postcode"@en ;
    skos:inScheme cs: ;
    skos:prefLabel "Locality-Stsuffix-Nolast-Lotno-Levelno-Postcode"@en ;
    skos:topConceptOf cs: .

:LOC-STS-NOL-LOT-PPC a skos:Concept ;
    dcterms:identifier "LOC-STS-NOL-LOT-PPC"^^xsd:token ;
    status:status iso19153:original ;
    rdfs:isDefinedBy cs: ;
    skos:definition "Change To Locality Name, Street Suffix, Number Last, Lot Number And Primary Postcode"@en ;
    skos:inScheme cs: ;
    skos:prefLabel "Locality-Stsuffix-Nolast-Lotno-Postcode"@en ;
    skos:topConceptOf cs: .

:LOC-STS-NOL-LVN a skos:Concept ;
    dcterms:identifier "LOC-STS-NOL-LVN"^^xsd:token ;
    status:status iso19153:original ;
    rdfs:isDefinedBy cs: ;
    skos:definition "Change To Locality Name, Street Suffix, Number Last And Level Number"@en ;
    skos:inScheme cs: ;
    skos:prefLabel "Locality-Stsuffix-Nolast-Levelno"@en ;
    skos:topConceptOf cs: .

:LOC-STS-NOL-LVN-PPC a skos:Concept ;
    dcterms:identifier "LOC-STS-NOL-LVN-PPC"^^xsd:token ;
    status:status iso19153:original ;
    rdfs:isDefinedBy cs: ;
    skos:definition "Change To Locality Name, Street Suffix, Number Last, Level Number And Primary Postcode"@en ;
    skos:inScheme cs: ;
    skos:prefLabel "Locality-Stsuffix-Nolast-Levelno-Postcode"@en ;
    skos:topConceptOf cs: .

:LOC-STS-NOL-PPC a skos:Concept ;
    dcterms:identifier "LOC-STS-NOL-PPC"^^xsd:token ;
    status:status iso19153:original ;
    rdfs:isDefinedBy cs: ;
    skos:definition "Change To Locality Name, Street Suffix, Number Last And Primary Postcode"@en ;
    skos:inScheme cs: ;
    skos:prefLabel "Locality-Stsuffix-Nolast-Postcode"@en ;
    skos:topConceptOf cs: .

:LOC-STS-PPC a skos:Concept ;
    dcterms:identifier "LOC-STS-PPC"^^xsd:token ;
    status:status iso19153:original ;
    rdfs:isDefinedBy cs: ;
    skos:definition "Change To Locality Name, Street Suffix And Primary Postcode"@en ;
    skos:inScheme cs: ;
    skos:prefLabel "Locality-Stsuffix-Postcode"@en ;
    skos:topConceptOf cs: .

:LOC-STT a skos:Concept ;
    dcterms:identifier "LOC-STT"^^xsd:token ;
    status:status iso19153:original ;
    rdfs:isDefinedBy cs: ;
    skos:definition "Change To Locality Name And Street Type"@en ;
    skos:inScheme cs: ;
    skos:prefLabel "Locality-Sttype"@en ;
    skos:topConceptOf cs: .

:LOC-STT-LOT a skos:Concept ;
    dcterms:identifier "LOC-STT-LOT"^^xsd:token ;
    status:status iso19153:original ;
    rdfs:isDefinedBy cs: ;
    skos:definition "Change To Locality Name, Street Type And Lot Number"@en ;
    skos:inScheme cs: ;
    skos:prefLabel "Locality-Sttype-Lotno"@en ;
    skos:topConceptOf cs: .

:LOC-STT-LOT-LVN a skos:Concept ;
    dcterms:identifier "LOC-STT-LOT-LVN"^^xsd:token ;
    status:status iso19153:original ;
    rdfs:isDefinedBy cs: ;
    skos:definition "Change To Locality Name, Street Type, Lot Number And Level Number"@en ;
    skos:inScheme cs: ;
    skos:prefLabel "Locality-Sttype-Lotno-Levelno"@en ;
    skos:topConceptOf cs: .

:LOC-STT-LOT-LVN-PPC a skos:Concept ;
    dcterms:identifier "LOC-STT-LOT-LVN-PPC"^^xsd:token ;
    status:status iso19153:original ;
    rdfs:isDefinedBy cs: ;
    skos:definition "Change To Locality Name, Street Type, Lot Number, Level Number And Primary Postcode"@en ;
    skos:inScheme cs: ;
    skos:prefLabel "Locality-Sttype-Lotno-Levelno-Postcode"@en ;
    skos:topConceptOf cs: .

:LOC-STT-LOT-PPC a skos:Concept ;
    dcterms:identifier "LOC-STT-LOT-PPC"^^xsd:token ;
    status:status iso19153:original ;
    rdfs:isDefinedBy cs: ;
    skos:definition "Change To Locality Name, Street Type, Lot Number And Primary Postcode"@en ;
    skos:inScheme cs: ;
    skos:prefLabel "Locality-Sttype-Lotno-Postcode"@en ;
    skos:topConceptOf cs: .

:LOC-STT-LVN a skos:Concept ;
    dcterms:identifier "LOC-STT-LVN"^^xsd:token ;
    status:status iso19153:original ;
    rdfs:isDefinedBy cs: ;
    skos:definition "Change To Locality Name, Street Type And Level Number"@en ;
    skos:inScheme cs: ;
    skos:prefLabel "Locality-Sttype-Levelno"@en ;
    skos:topConceptOf cs: .

:LOC-STT-LVN-PPC a skos:Concept ;
    dcterms:identifier "LOC-STT-LVN-PPC"^^xsd:token ;
    status:status iso19153:original ;
    rdfs:isDefinedBy cs: ;
    skos:definition "Change To Locality Name, Street Type, Level Number And Primary Postcode"@en ;
    skos:inScheme cs: ;
    skos:prefLabel "Locality-Sttype-Levelno-Postcode"@en ;
    skos:topConceptOf cs: .

:LOC-STT-NOF a skos:Concept ;
    dcterms:identifier "LOC-STT-NOF"^^xsd:token ;
    status:status iso19153:original ;
    rdfs:isDefinedBy cs: ;
    skos:definition "Change To Locality Name, Street Type And Number First"@en ;
    skos:inScheme cs: ;
    skos:prefLabel "Locality-Sttype-Nofirst"@en ;
    skos:topConceptOf cs: .

:LOC-STT-NOF-LOT a skos:Concept ;
    dcterms:identifier "LOC-STT-NOF-LOT"^^xsd:token ;
    status:status iso19153:original ;
    rdfs:isDefinedBy cs: ;
    skos:definition "Change To Locality Name, Street Type, Number First And Lot Number"@en ;
    skos:inScheme cs: ;
    skos:prefLabel "Locality-Sttype-Nofirst-Lotno"@en ;
    skos:topConceptOf cs: .

:LOC-STT-NOF-LOT-LVN a skos:Concept ;
    dcterms:identifier "LOC-STT-NOF-LOT-LVN"^^xsd:token ;
    status:status iso19153:original ;
    rdfs:isDefinedBy cs: ;
    skos:definition "Change To Locality Name, Street Type, Number First, Lot Number And Level Number"@en ;
    skos:inScheme cs: ;
    skos:prefLabel "Locality-Sttype-Nofirst-Lotno-Levelno"@en ;
    skos:topConceptOf cs: .

:LOC-STT-NOF-LOT-LVN-PPC a skos:Concept ;
    dcterms:identifier "LOC-STT-NOF-LOT-LVN-PPC"^^xsd:token ;
    status:status iso19153:original ;
    rdfs:isDefinedBy cs: ;
    skos:definition "Change To Locality Name, Street Type, Number First, Lot Number, Level Number And Primary Postcode"@en ;
    skos:inScheme cs: ;
    skos:prefLabel "Locality-Sttype-Nofirst-Lotno-Levelno-Postcode"@en ;
    skos:topConceptOf cs: .

:LOC-STT-NOF-LOT-PPC a skos:Concept ;
    dcterms:identifier "LOC-STT-NOF-LOT-PPC"^^xsd:token ;
    status:status iso19153:original ;
    rdfs:isDefinedBy cs: ;
    skos:definition "Change To Locality Name, Street Type, Number First, Lot Number And Primary Postcode"@en ;
    skos:inScheme cs: ;
    skos:prefLabel "Locality-Sttype-Nofirst-Lotno-Postcode"@en ;
    skos:topConceptOf cs: .

:LOC-STT-NOF-LVN a skos:Concept ;
    dcterms:identifier "LOC-STT-NOF-LVN"^^xsd:token ;
    status:status iso19153:original ;
    rdfs:isDefinedBy cs: ;
    skos:definition "Change To Locality Name, Street Type, Number First And Level Number"@en ;
    skos:inScheme cs: ;
    skos:prefLabel "Locality-Sttype-Nofirst-Levelno"@en ;
    skos:topConceptOf cs: .

:LOC-STT-NOF-LVN-PPC a skos:Concept ;
    dcterms:identifier "LOC-STT-NOF-LVN-PPC"^^xsd:token ;
    status:status iso19153:original ;
    rdfs:isDefinedBy cs: ;
    skos:definition "Change To Locality Name, Street Type, Number First, Level Number And Primary Postcode"@en ;
    skos:inScheme cs: ;
    skos:prefLabel "Locality-Sttype-Nofirst-Levelno-Postcode"@en ;
    skos:topConceptOf cs: .

:LOC-STT-NOF-NOL a skos:Concept ;
    dcterms:identifier "LOC-STT-NOF-NOL"^^xsd:token ;
    status:status iso19153:original ;
    rdfs:isDefinedBy cs: ;
    skos:definition "Change To Locality Name, Street Type, Number First And Number Last"@en ;
    skos:inScheme cs: ;
    skos:prefLabel "Locality-Sttype-Nofirst-Nolast"@en ;
    skos:topConceptOf cs: .

:LOC-STT-NOF-NOL-LOT a skos:Concept ;
    dcterms:identifier "LOC-STT-NOF-NOL-LOT"^^xsd:token ;
    status:status iso19153:original ;
    rdfs:isDefinedBy cs: ;
    skos:definition "Change To Locality Name, Street Type, Number First, Number Last And Lot Number"@en ;
    skos:inScheme cs: ;
    skos:prefLabel "Locality-Sttype-Nofirst-Nolast-Lotno"@en ;
    skos:topConceptOf cs: .

:LOC-STT-NOF-NOL-LOT-LVN a skos:Concept ;
    dcterms:identifier "LOC-STT-NOF-NOL-LOT-LVN"^^xsd:token ;
    status:status iso19153:original ;
    rdfs:isDefinedBy cs: ;
    skos:definition "Change To Locality Name, Street Type, Number First, Number Last, Lot Number And Level Number"@en ;
    skos:inScheme cs: ;
    skos:prefLabel "Locality-Sttype-Nofirst-Nolast-Lotno-Levelno"@en ;
    skos:topConceptOf cs: .

:LOC-STT-NOF-NOL-LOT-LVN-PPC a skos:Concept ;
    dcterms:identifier "LOC-STT-NOF-NOL-LOT-LVN-PPC"^^xsd:token ;
    status:status iso19153:original ;
    rdfs:isDefinedBy cs: ;
    skos:definition "Change To Locality Name, Street Type, Number First, Number Last, Lot Number, Level Number And Primary Postcode"@en ;
    skos:inScheme cs: ;
    skos:prefLabel "Locality-Sttype-Nofirst-Nolast-Lotno-Levelno-Postcode"@en ;
    skos:topConceptOf cs: .

:LOC-STT-NOF-NOL-LOT-PPC a skos:Concept ;
    dcterms:identifier "LOC-STT-NOF-NOL-LOT-PPC"^^xsd:token ;
    status:status iso19153:original ;
    rdfs:isDefinedBy cs: ;
    skos:definition "Change To Locality Name, Street Type, Number First, Number Last, Lot Number And Primary Postcode"@en ;
    skos:inScheme cs: ;
    skos:prefLabel "Locality-Sttype-Nofirst-Nolast-Lotno-Postcode"@en ;
    skos:topConceptOf cs: .

:LOC-STT-NOF-NOL-LVN a skos:Concept ;
    dcterms:identifier "LOC-STT-NOF-NOL-LVN"^^xsd:token ;
    status:status iso19153:original ;
    rdfs:isDefinedBy cs: ;
    skos:definition "Change To Locality Name, Street Type, Number First, Number Last And Level Number"@en ;
    skos:inScheme cs: ;
    skos:prefLabel "Locality-Sttype-Nofirst-Nolast-Levelno"@en ;
    skos:topConceptOf cs: .

:LOC-STT-NOF-NOL-LVN-PPC a skos:Concept ;
    dcterms:identifier "LOC-STT-NOF-NOL-LVN-PPC"^^xsd:token ;
    status:status iso19153:original ;
    rdfs:isDefinedBy cs: ;
    skos:definition "Change To Locality Name, Street Type, Number First, Number Last, Level Number And Primary Postcode"@en ;
    skos:inScheme cs: ;
    skos:prefLabel "Locality-Sttype-Nofirst-Nolast-Levelno-Postcode"@en ;
    skos:topConceptOf cs: .

:LOC-STT-NOF-NOL-PPC a skos:Concept ;
    dcterms:identifier "LOC-STT-NOF-NOL-PPC"^^xsd:token ;
    status:status iso19153:original ;
    rdfs:isDefinedBy cs: ;
    skos:definition "Change To Locality Name, Street Type, Number First, Number Last And Primary Postcode"@en ;
    skos:inScheme cs: ;
    skos:prefLabel "Locality-Sttype-Nofirst-Nolast-Postcode"@en ;
    skos:topConceptOf cs: .

:LOC-STT-NOF-PPC a skos:Concept ;
    dcterms:identifier "LOC-STT-NOF-PPC"^^xsd:token ;
    status:status iso19153:original ;
    rdfs:isDefinedBy cs: ;
    skos:definition "Change To Locality Name, Street Type, Number First And Primary Postcode"@en ;
    skos:inScheme cs: ;
    skos:prefLabel "Locality-Sttype-Nofirst-Postcode"@en ;
    skos:topConceptOf cs: .

:LOC-STT-NOL a skos:Concept ;
    dcterms:identifier "LOC-STT-NOL"^^xsd:token ;
    status:status iso19153:original ;
    rdfs:isDefinedBy cs: ;
    skos:definition "Change To Locality Name, Street Type And Number Last"@en ;
    skos:inScheme cs: ;
    skos:prefLabel "Locality-Sttype-Nolast"@en ;
    skos:topConceptOf cs: .

:LOC-STT-NOL-LOT a skos:Concept ;
    dcterms:identifier "LOC-STT-NOL-LOT"^^xsd:token ;
    status:status iso19153:original ;
    rdfs:isDefinedBy cs: ;
    skos:definition "Change To Locality Name, Street Type, Number Last And Lot Number"@en ;
    skos:inScheme cs: ;
    skos:prefLabel "Locality-Sttype-Nolast-Lotno"@en ;
    skos:topConceptOf cs: .

:LOC-STT-NOL-LOT-LVN a skos:Concept ;
    dcterms:identifier "LOC-STT-NOL-LOT-LVN"^^xsd:token ;
    status:status iso19153:original ;
    rdfs:isDefinedBy cs: ;
    skos:definition "Change To Locality Name, Street Type, Number Last, Lot Number And Level Number"@en ;
    skos:inScheme cs: ;
    skos:prefLabel "Locality-Sttype-Nolast-Lotno-Levelno"@en ;
    skos:topConceptOf cs: .

:LOC-STT-NOL-LOT-LVN-PPC a skos:Concept ;
    dcterms:identifier "LOC-STT-NOL-LOT-LVN-PPC"^^xsd:token ;
    status:status iso19153:original ;
    rdfs:isDefinedBy cs: ;
    skos:definition "Change To Locality Name, Street Type, Number Last, Lot Number, Level Number And Primary Postcode"@en ;
    skos:inScheme cs: ;
    skos:prefLabel "Locality-Sttype-Nolast-Lotno-Levelno-Postcode"@en ;
    skos:topConceptOf cs: .

:LOC-STT-NOL-LOT-PPC a skos:Concept ;
    dcterms:identifier "LOC-STT-NOL-LOT-PPC"^^xsd:token ;
    status:status iso19153:original ;
    rdfs:isDefinedBy cs: ;
    skos:definition "Change To Locality Name, Street Type, Number Last, Lot Number And Primary Postcode"@en ;
    skos:inScheme cs: ;
    skos:prefLabel "Locality-Sttype-Nolast-Lotno-Postcode"@en ;
    skos:topConceptOf cs: .

:LOC-STT-NOL-LVN a skos:Concept ;
    dcterms:identifier "LOC-STT-NOL-LVN"^^xsd:token ;
    status:status iso19153:original ;
    rdfs:isDefinedBy cs: ;
    skos:definition "Change To Locality Name, Street Type, Number Last And Level Number"@en ;
    skos:inScheme cs: ;
    skos:prefLabel "Locality-Sttype-Nolast-Levelno"@en ;
    skos:topConceptOf cs: .

:LOC-STT-NOL-LVN-PPC a skos:Concept ;
    dcterms:identifier "LOC-STT-NOL-LVN-PPC"^^xsd:token ;
    status:status iso19153:original ;
    rdfs:isDefinedBy cs: ;
    skos:definition "Change To Locality Name, Street Type, Number Last, Level Number And Primary Postcode"@en ;
    skos:inScheme cs: ;
    skos:prefLabel "Locality-Sttype-Nolast-Levelno-Postcode"@en ;
    skos:topConceptOf cs: .

:LOC-STT-NOL-PPC a skos:Concept ;
    dcterms:identifier "LOC-STT-NOL-PPC"^^xsd:token ;
    status:status iso19153:original ;
    rdfs:isDefinedBy cs: ;
    skos:definition "Change To Locality Name, Street Type, Number Last And Primary Postcode"@en ;
    skos:inScheme cs: ;
    skos:prefLabel "Locality-Sttype-Nolast-Postcode"@en ;
    skos:topConceptOf cs: .

:LOC-STT-PPC a skos:Concept ;
    dcterms:identifier "LOC-STT-PPC"^^xsd:token ;
    status:status iso19153:original ;
    rdfs:isDefinedBy cs: ;
    skos:definition "Change To Locality Name, Street Type And Primary Postcode"@en ;
    skos:inScheme cs: ;
    skos:prefLabel "Locality-Sttype-Postcode"@en ;
    skos:topConceptOf cs: .

:LOC-STT-STS a skos:Concept ;
    dcterms:identifier "LOC-STT-STS"^^xsd:token ;
    status:status iso19153:original ;
    rdfs:isDefinedBy cs: ;
    skos:definition "Change To Locality Name, Street Type And Street Suffix"@en ;
    skos:inScheme cs: ;
    skos:prefLabel "Locality-Sttype-Stsuffix"@en ;
    skos:topConceptOf cs: .

:LOC-STT-STS-LOT a skos:Concept ;
    dcterms:identifier "LOC-STT-STS-LOT"^^xsd:token ;
    status:status iso19153:original ;
    rdfs:isDefinedBy cs: ;
    skos:definition "Change To Locality Name, Street Type, Street Suffix And Lot Number"@en ;
    skos:inScheme cs: ;
    skos:prefLabel "Locality-Sttype-Stsuffix-Lotno"@en ;
    skos:topConceptOf cs: .

:LOC-STT-STS-LOT-LVN a skos:Concept ;
    dcterms:identifier "LOC-STT-STS-LOT-LVN"^^xsd:token ;
    status:status iso19153:original ;
    rdfs:isDefinedBy cs: ;
    skos:definition "Change To Locality Name, Street Type, Street Suffix, Lot Number And Level Number"@en ;
    skos:inScheme cs: ;
    skos:prefLabel "Locality-Sttype-Stsuffix-Lotno-Levelno"@en ;
    skos:topConceptOf cs: .

:LOC-STT-STS-LOT-LVN-PPC a skos:Concept ;
    dcterms:identifier "LOC-STT-STS-LOT-LVN-PPC"^^xsd:token ;
    status:status iso19153:original ;
    rdfs:isDefinedBy cs: ;
    skos:definition "Change To Locality Name, Street Type, Street Suffix, Lot Number, Level Number And Primary Postcode"@en ;
    skos:inScheme cs: ;
    skos:prefLabel "Locality-Sttype-Stsuffix-Lotno-Levelno-Postcode"@en ;
    skos:topConceptOf cs: .

:LOC-STT-STS-LOT-PPC a skos:Concept ;
    dcterms:identifier "LOC-STT-STS-LOT-PPC"^^xsd:token ;
    status:status iso19153:original ;
    rdfs:isDefinedBy cs: ;
    skos:definition "Change To Locality Name, Street Type, Street Suffix, Lot Number And Primary Postcode"@en ;
    skos:inScheme cs: ;
    skos:prefLabel "Locality-Sttype-Stsuffix-Lotno-Postcode"@en ;
    skos:topConceptOf cs: .

:LOC-STT-STS-LVN a skos:Concept ;
    dcterms:identifier "LOC-STT-STS-LVN"^^xsd:token ;
    status:status iso19153:original ;
    rdfs:isDefinedBy cs: ;
    skos:definition "Change To Locality Name, Street Type, Street Suffix And Level Number"@en ;
    skos:inScheme cs: ;
    skos:prefLabel "Locality-Sttype-Stsuffix-Levelno"@en ;
    skos:topConceptOf cs: .

:LOC-STT-STS-LVN-PPC a skos:Concept ;
    dcterms:identifier "LOC-STT-STS-LVN-PPC"^^xsd:token ;
    status:status iso19153:original ;
    rdfs:isDefinedBy cs: ;
    skos:definition "Change To Locality Name, Street Type, Street Suffix, Level Number And Primary Postcode"@en ;
    skos:inScheme cs: ;
    skos:prefLabel "Locality-Sttype-Stsuffix-Levelno-Postcode"@en ;
    skos:topConceptOf cs: .

:LOC-STT-STS-NOF a skos:Concept ;
    dcterms:identifier "LOC-STT-STS-NOF"^^xsd:token ;
    status:status iso19153:original ;
    rdfs:isDefinedBy cs: ;
    skos:definition "Change To Locality Name, Street Type, Street Suffix And Number First"@en ;
    skos:inScheme cs: ;
    skos:prefLabel "Locality-Sttype-Stsuffix-Nofirst"@en ;
    skos:topConceptOf cs: .

:LOC-STT-STS-NOF-LOT a skos:Concept ;
    dcterms:identifier "LOC-STT-STS-NOF-LOT"^^xsd:token ;
    status:status iso19153:original ;
    rdfs:isDefinedBy cs: ;
    skos:definition "Change To Locality Name, Street Type, Street Suffix, Number First And Lot Number"@en ;
    skos:inScheme cs: ;
    skos:prefLabel "Locality-Sttype-Stsuffix-Nofirst-Lotno"@en ;
    skos:topConceptOf cs: .

:LOC-STT-STS-NOF-LOT-LVN a skos:Concept ;
    dcterms:identifier "LOC-STT-STS-NOF-LOT-LVN"^^xsd:token ;
    status:status iso19153:original ;
    rdfs:isDefinedBy cs: ;
    skos:definition "Change To Locality Name, Street Type, Street Suffix, Number First, Lot Number And Level Number"@en ;
    skos:inScheme cs: ;
    skos:prefLabel "Locality-Sttype-Stsuffix-Nofirst-Lotno-Levelno"@en ;
    skos:topConceptOf cs: .

:LOC-STT-STS-NOF-LOT-LVN-PPC a skos:Concept ;
    dcterms:identifier "LOC-STT-STS-NOF-LOT-LVN-PPC"^^xsd:token ;
    status:status iso19153:original ;
    rdfs:isDefinedBy cs: ;
    skos:definition "Change To Locality Name, Street Type, Street Suffix, Number First, Lot Number, Level Number And Primary Postcode"@en ;
    skos:inScheme cs: ;
    skos:prefLabel "Locality-Sttype-Stsuffix-Nofirst-Lotno-Levelno-Postcode"@en ;
    skos:topConceptOf cs: .

:LOC-STT-STS-NOF-LOT-PPC a skos:Concept ;
    dcterms:identifier "LOC-STT-STS-NOF-LOT-PPC"^^xsd:token ;
    status:status iso19153:original ;
    rdfs:isDefinedBy cs: ;
    skos:definition "Change To Locality Name, Street Type, Street Suffix, Number First, Lot Number And Primary Postcode"@en ;
    skos:inScheme cs: ;
    skos:prefLabel "Locality-Sttype-Stsuffix-Nofirst-Lotno-Postcode"@en ;
    skos:topConceptOf cs: .

:LOC-STT-STS-NOF-LVN a skos:Concept ;
    dcterms:identifier "LOC-STT-STS-NOF-LVN"^^xsd:token ;
    status:status iso19153:original ;
    rdfs:isDefinedBy cs: ;
    skos:definition "Change To Locality Name, Street Type, Street Suffix, Number First And Level Number"@en ;
    skos:inScheme cs: ;
    skos:prefLabel "Locality-Sttype-Stsuffix-Nofirst-Levelno"@en ;
    skos:topConceptOf cs: .

:LOC-STT-STS-NOF-LVN-PPC a skos:Concept ;
    dcterms:identifier "LOC-STT-STS-NOF-LVN-PPC"^^xsd:token ;
    status:status iso19153:original ;
    rdfs:isDefinedBy cs: ;
    skos:definition "Change To Locality Name, Street Type, Street Suffix, Number First, Level Number And Primary Postcode"@en ;
    skos:inScheme cs: ;
    skos:prefLabel "Locality-Sttype-Stsuffix-Nofirst-Levelno-Postcode"@en ;
    skos:topConceptOf cs: .

:LOC-STT-STS-NOF-NOL a skos:Concept ;
    dcterms:identifier "LOC-STT-STS-NOF-NOL"^^xsd:token ;
    status:status iso19153:original ;
    rdfs:isDefinedBy cs: ;
    skos:definition "Change To Locality Name, Street Type, Street Suffix, Number First And Number Last"@en ;
    skos:inScheme cs: ;
    skos:prefLabel "Locality-Sttype-Stsuffix-Nofirst-Nolast"@en ;
    skos:topConceptOf cs: .

:LOC-STT-STS-NOF-NOL-LOT a skos:Concept ;
    dcterms:identifier "LOC-STT-STS-NOF-NOL-LOT"^^xsd:token ;
    status:status iso19153:original ;
    rdfs:isDefinedBy cs: ;
    skos:definition "Change To Locality Name, Street Type, Street Suffix, Number First, Number Last And Lot Number"@en ;
    skos:inScheme cs: ;
    skos:prefLabel "Locality-Sttype-Stsuffix-Nofirst-Nolast-Lotno"@en ;
    skos:topConceptOf cs: .

:LOC-STT-STS-NOF-NOL-LOT-LVN a skos:Concept ;
    dcterms:identifier "LOC-STT-STS-NOF-NOL-LOT-LVN"^^xsd:token ;
    status:status iso19153:original ;
    rdfs:isDefinedBy cs: ;
    skos:definition "Change To Locality Name, Street Type, Street Suffix, Number First, Number Last, Lot Number And Level Number"@en ;
    skos:inScheme cs: ;
    skos:prefLabel "Locality-Sttype-Stsuffix-Nofirst-Nolast-Lotno-Levelno"@en ;
    skos:topConceptOf cs: .

:LOC-STT-STS-NOF-NOL-LOT-LVN-PPC a skos:Concept ;
    dcterms:identifier "LOC-STT-STS-NOF-NOL-LOT-LVN-PPC"^^xsd:token ;
    status:status iso19153:original ;
    rdfs:isDefinedBy cs: ;
    skos:definition "Change To Locality Name, Street Type, Street Suffix, Number First, Number Last, Lot Number, Level Number And Primary Postcode"@en ;
    skos:inScheme cs: ;
    skos:prefLabel "Locality-Sttype-Stsuffix-Nofirst-Nolast-Lotno-Levelno-Postcode"@en ;
    skos:topConceptOf cs: .

:LOC-STT-STS-NOF-NOL-LOT-PPC a skos:Concept ;
    dcterms:identifier "LOC-STT-STS-NOF-NOL-LOT-PPC"^^xsd:token ;
    status:status iso19153:original ;
    rdfs:isDefinedBy cs: ;
    skos:definition "Change To Locality Name, Street Type, Street Suffix, Number First, Number Last, Lot Number And Primary Postcode"@en ;
    skos:inScheme cs: ;
    skos:prefLabel "Locality-Sttype-Stsuffix-Nofirst-Nolast-Lotno-Postcode"@en ;
    skos:topConceptOf cs: .

:LOC-STT-STS-NOF-NOL-LVN a skos:Concept ;
    dcterms:identifier "LOC-STT-STS-NOF-NOL-LVN"^^xsd:token ;
    status:status iso19153:original ;
    rdfs:isDefinedBy cs: ;
    skos:definition "Change To Locality Name, Street Type, Street Suffix, Number First, Number Last And Level Number"@en ;
    skos:inScheme cs: ;
    skos:prefLabel "Locality-Sttype-Stsuffix-Nofirst-Nolast-Levelno"@en ;
    skos:topConceptOf cs: .

:LOC-STT-STS-NOF-NOL-LVN-PPC a skos:Concept ;
    dcterms:identifier "LOC-STT-STS-NOF-NOL-LVN-PPC"^^xsd:token ;
    status:status iso19153:original ;
    rdfs:isDefinedBy cs: ;
    skos:definition "Change To Locality Name, Street Type, Street Suffix, Number First, Number Last, Level Number And Primary Postcode"@en ;
    skos:inScheme cs: ;
    skos:prefLabel "Locality-Sttype-Stsuffix-Nofirst-Nolast-Levelno-Postcode"@en ;
    skos:topConceptOf cs: .

:LOC-STT-STS-NOF-NOL-PPC a skos:Concept ;
    dcterms:identifier "LOC-STT-STS-NOF-NOL-PPC"^^xsd:token ;
    status:status iso19153:original ;
    rdfs:isDefinedBy cs: ;
    skos:definition "Change To Locality Name, Street Type, Street Suffix, Number First, Number Last And Primary Postcode"@en ;
    skos:inScheme cs: ;
    skos:prefLabel "Locality-Sttype-Stsuffix-Nofirst-Nolast-Postcode"@en ;
    skos:topConceptOf cs: .

:LOC-STT-STS-NOF-PPC a skos:Concept ;
    dcterms:identifier "LOC-STT-STS-NOF-PPC"^^xsd:token ;
    status:status iso19153:original ;
    rdfs:isDefinedBy cs: ;
    skos:definition "Change To Locality Name, Street Type, Street Suffix, Number First And Primary Postcode"@en ;
    skos:inScheme cs: ;
    skos:prefLabel "Locality-Sttype-Stsuffix-Nofirst-Postcode"@en ;
    skos:topConceptOf cs: .

:LOC-STT-STS-NOL a skos:Concept ;
    dcterms:identifier "LOC-STT-STS-NOL"^^xsd:token ;
    status:status iso19153:original ;
    rdfs:isDefinedBy cs: ;
    skos:definition "Change To Locality Name, Street Type, Street Suffix And Number Last"@en ;
    skos:inScheme cs: ;
    skos:prefLabel "Locality-Sttype-Stsuffix-Nolast"@en ;
    skos:topConceptOf cs: .

:LOC-STT-STS-NOL-LOT a skos:Concept ;
    dcterms:identifier "LOC-STT-STS-NOL-LOT"^^xsd:token ;
    status:status iso19153:original ;
    rdfs:isDefinedBy cs: ;
    skos:definition "Change To Locality Name, Street Type, Street Suffix, Number Last And Lot Number"@en ;
    skos:inScheme cs: ;
    skos:prefLabel "Locality-Sttype-Stsuffix-Nolast-Lotno"@en ;
    skos:topConceptOf cs: .

:LOC-STT-STS-NOL-LOT-LVN a skos:Concept ;
    dcterms:identifier "LOC-STT-STS-NOL-LOT-LVN"^^xsd:token ;
    status:status iso19153:original ;
    rdfs:isDefinedBy cs: ;
    skos:definition "Change To Locality Name, Street Type, Street Suffix, Number Last, Lot Number And Level Number"@en ;
    skos:inScheme cs: ;
    skos:prefLabel "Locality-Sttype-Stsuffix-Nolast-Lotno-Levelno"@en ;
    skos:topConceptOf cs: .

:LOC-STT-STS-NOL-LOT-LVN-PPC a skos:Concept ;
    dcterms:identifier "LOC-STT-STS-NOL-LOT-LVN-PPC"^^xsd:token ;
    status:status iso19153:original ;
    rdfs:isDefinedBy cs: ;
    skos:definition "Change To Locality Name, Street Type, Street Suffix, Number Last, Lot Number, Level Number And Primary Postcode"@en ;
    skos:inScheme cs: ;
    skos:prefLabel "Locality-Sttype-Stsuffix-Nolast-Lotno-Levelno-Postcode"@en ;
    skos:topConceptOf cs: .

:LOC-STT-STS-NOL-LOT-PPC a skos:Concept ;
    dcterms:identifier "LOC-STT-STS-NOL-LOT-PPC"^^xsd:token ;
    status:status iso19153:original ;
    rdfs:isDefinedBy cs: ;
    skos:definition "Change To Locality Name, Street Type, Street Suffix, Number Last, Lot Number And Primary Postcode"@en ;
    skos:inScheme cs: ;
    skos:prefLabel "Locality-Sttype-Stsuffix-Nolast-Lotno-Postcode"@en ;
    skos:topConceptOf cs: .

:LOC-STT-STS-NOL-LVN a skos:Concept ;
    dcterms:identifier "LOC-STT-STS-NOL-LVN"^^xsd:token ;
    status:status iso19153:original ;
    rdfs:isDefinedBy cs: ;
    skos:definition "Change To Locality Name, Street Type, Street Suffix, Number Last And Level Number"@en ;
    skos:inScheme cs: ;
    skos:prefLabel "Locality-Sttype-Stsuffix-Nolast-Levelno"@en ;
    skos:topConceptOf cs: .

:LOC-STT-STS-NOL-LVN-PPC a skos:Concept ;
    dcterms:identifier "LOC-STT-STS-NOL-LVN-PPC"^^xsd:token ;
    status:status iso19153:original ;
    rdfs:isDefinedBy cs: ;
    skos:definition "Change To Locality Name, Street Type, Street Suffix, Number Last, Level Number And Primary Postcode"@en ;
    skos:inScheme cs: ;
    skos:prefLabel "Locality-Sttype-Stsuffix-Nolast-Levelno-Postcode"@en ;
    skos:topConceptOf cs: .

:LOC-STT-STS-NOL-PPC a skos:Concept ;
    dcterms:identifier "LOC-STT-STS-NOL-PPC"^^xsd:token ;
    status:status iso19153:original ;
    rdfs:isDefinedBy cs: ;
    skos:definition "Change To Locality Name, Street Type, Street Suffix, Number Last And Primary Postcode"@en ;
    skos:inScheme cs: ;
    skos:prefLabel "Locality-Sttype-Stsuffix-Nolast-Postcode"@en ;
    skos:topConceptOf cs: .

:LOC-STT-STS-PPC a skos:Concept ;
    dcterms:identifier "LOC-STT-STS-PPC"^^xsd:token ;
    status:status iso19153:original ;
    rdfs:isDefinedBy cs: ;
    skos:definition "Change To Locality Name, Street Type, Street Suffix And Primary Postcode"@en ;
    skos:inScheme cs: ;
    skos:prefLabel "Locality-Sttype-Stsuffix-Postcode"@en ;
    skos:topConceptOf cs: .

:LOT a skos:Concept ;
    dcterms:identifier "LOT"^^xsd:token ;
    status:status iso19153:original ;
    rdfs:isDefinedBy cs: ;
    skos:definition "Change To Lot Number Only"@en ;
    skos:inScheme cs: ;
    skos:prefLabel "Lotno"@en ;
    skos:topConceptOf cs: .

:LOT-LVN a skos:Concept ;
    dcterms:identifier "LOT-LVN"^^xsd:token ;
    status:status iso19153:original ;
    rdfs:isDefinedBy cs: ;
    skos:definition "Change To Lot Number And Level Number"@en ;
    skos:inScheme cs: ;
    skos:prefLabel "Lotno-Levelno"@en ;
    skos:topConceptOf cs: .

:LOT-LVN-PPC a skos:Concept ;
    dcterms:identifier "LOT-LVN-PPC"^^xsd:token ;
    status:status iso19153:original ;
    rdfs:isDefinedBy cs: ;
    skos:definition "Change To Lot Number, Level Number And Primary Postcode"@en ;
    skos:inScheme cs: ;
    skos:prefLabel "Lotno-Levelno-Postcode"@en ;
    skos:topConceptOf cs: .

:LOT-PPC a skos:Concept ;
    dcterms:identifier "LOT-PPC"^^xsd:token ;
    status:status iso19153:original ;
    rdfs:isDefinedBy cs: ;
    skos:definition "Change To Lot Number And Primary Postcode"@en ;
    skos:inScheme cs: ;
    skos:prefLabel "Lotno-Postcode"@en ;
    skos:topConceptOf cs: .

:LVN a skos:Concept ;
    dcterms:identifier "LVN"^^xsd:token ;
    status:status iso19153:original ;
    rdfs:isDefinedBy cs: ;
    skos:definition "Change To Level Number Only"@en ;
    skos:inScheme cs: ;
    skos:prefLabel "Levelno"@en ;
    skos:topConceptOf cs: .

:LVN-PPC a skos:Concept ;
    dcterms:identifier "LVN-PPC"^^xsd:token ;
    status:status iso19153:original ;
    rdfs:isDefinedBy cs: ;
    skos:definition "Change To Level Number And Primary Postcode"@en ;
    skos:inScheme cs: ;
    skos:prefLabel "Levelno-Postcode"@en ;
    skos:topConceptOf cs: .

:NOF a skos:Concept ;
    dcterms:identifier "NOF"^^xsd:token ;
    status:status iso19153:original ;
    rdfs:isDefinedBy cs: ;
    skos:definition "Change To Number First Only"@en ;
    skos:inScheme cs: ;
    skos:prefLabel "Nofirst"@en ;
    skos:topConceptOf cs: .

:NOF-LOT a skos:Concept ;
    dcterms:identifier "NOF-LOT"^^xsd:token ;
    status:status iso19153:original ;
    rdfs:isDefinedBy cs: ;
    skos:definition "Change To Number First And Lot Number"@en ;
    skos:inScheme cs: ;
    skos:prefLabel "Nofirst-Lotno"@en ;
    skos:topConceptOf cs: .

:NOF-LOT-LVN a skos:Concept ;
    dcterms:identifier "NOF-LOT-LVN"^^xsd:token ;
    status:status iso19153:original ;
    rdfs:isDefinedBy cs: ;
    skos:definition "Change To Number First, Lot Number And Level Number"@en ;
    skos:inScheme cs: ;
    skos:prefLabel "Nofirst-Lotno-Levelno"@en ;
    skos:topConceptOf cs: .

:NOF-LOT-LVN-PPC a skos:Concept ;
    dcterms:identifier "NOF-LOT-LVN-PPC"^^xsd:token ;
    status:status iso19153:original ;
    rdfs:isDefinedBy cs: ;
    skos:definition "Change To Number First, Lot Number, Level Number And Primary Postcode"@en ;
    skos:inScheme cs: ;
    skos:prefLabel "Nofirst-Lotno-Levelno-Postcode"@en ;
    skos:topConceptOf cs: .

:NOF-LOT-PPC a skos:Concept ;
    dcterms:identifier "NOF-LOT-PPC"^^xsd:token ;
    status:status iso19153:original ;
    rdfs:isDefinedBy cs: ;
    skos:definition "Change To Number First, Lot Number And Primary Postcode"@en ;
    skos:inScheme cs: ;
    skos:prefLabel "Nofirst-Lotno-Postcode"@en ;
    skos:topConceptOf cs: .

:NOF-LVN a skos:Concept ;
    dcterms:identifier "NOF-LVN"^^xsd:token ;
    status:status iso19153:original ;
    rdfs:isDefinedBy cs: ;
    skos:definition "Change To Number First And Level Number"@en ;
    skos:inScheme cs: ;
    skos:prefLabel "Nofirst-Levelno"@en ;
    skos:topConceptOf cs: .

:NOF-LVN-PPC a skos:Concept ;
    dcterms:identifier "NOF-LVN-PPC"^^xsd:token ;
    status:status iso19153:original ;
    rdfs:isDefinedBy cs: ;
    skos:definition "Change To Number First, Level Number And Primary Postcode"@en ;
    skos:inScheme cs: ;
    skos:prefLabel "Nofirst-Levelno-Postcode"@en ;
    skos:topConceptOf cs: .

:NOF-NOL a skos:Concept ;
    dcterms:identifier "NOF-NOL"^^xsd:token ;
    status:status iso19153:original ;
    rdfs:isDefinedBy cs: ;
    skos:definition "Change To Number First And Number Last"@en ;
    skos:inScheme cs: ;
    skos:prefLabel "Nofirst-Nolast"@en ;
    skos:topConceptOf cs: .

:NOF-NOL-LOT a skos:Concept ;
    dcterms:identifier "NOF-NOL-LOT"^^xsd:token ;
    status:status iso19153:original ;
    rdfs:isDefinedBy cs: ;
    skos:definition "Change To Number First, Number Last And Lot Number"@en ;
    skos:inScheme cs: ;
    skos:prefLabel "Nofirst-Nolast-Lotno"@en ;
    skos:topConceptOf cs: .

:NOF-NOL-LOT-LVN a skos:Concept ;
    dcterms:identifier "NOF-NOL-LOT-LVN"^^xsd:token ;
    status:status iso19153:original ;
    rdfs:isDefinedBy cs: ;
    skos:definition "Change To Number First, Number Last, Lot Number And Level Number"@en ;
    skos:inScheme cs: ;
    skos:prefLabel "Nofirst-Nolast-Lotno-Levelno"@en ;
    skos:topConceptOf cs: .

:NOF-NOL-LOT-LVN-PPC a skos:Concept ;
    dcterms:identifier "NOF-NOL-LOT-LVN-PPC"^^xsd:token ;
    status:status iso19153:original ;
    rdfs:isDefinedBy cs: ;
    skos:definition "Change To Number First, Number Last, Lot Number, Level Number And Primary Postcode"@en ;
    skos:inScheme cs: ;
    skos:prefLabel "Nofirst-Nolast-Lotno-Levelno-Postcode"@en ;
    skos:topConceptOf cs: .

:NOF-NOL-LOT-PPC a skos:Concept ;
    dcterms:identifier "NOF-NOL-LOT-PPC"^^xsd:token ;
    status:status iso19153:original ;
    rdfs:isDefinedBy cs: ;
    skos:definition "Change To Number First, Number Last, Lot Number And Primary Postcode"@en ;
    skos:inScheme cs: ;
    skos:prefLabel "Nofirst-Nolast-Lotno-Postcode"@en ;
    skos:topConceptOf cs: .

:NOF-NOL-LVN a skos:Concept ;
    dcterms:identifier "NOF-NOL-LVN"^^xsd:token ;
    status:status iso19153:original ;
    rdfs:isDefinedBy cs: ;
    skos:definition "Change To Number First, Number Last And Level Number"@en ;
    skos:inScheme cs: ;
    skos:prefLabel "Nofirst-Nolast-Levelno"@en ;
    skos:topConceptOf cs: .

:NOF-NOL-LVN-PPC a skos:Concept ;
    dcterms:identifier "NOF-NOL-LVN-PPC"^^xsd:token ;
    status:status iso19153:original ;
    rdfs:isDefinedBy cs: ;
    skos:definition "Change To Number First, Number Last, Level Number And Primary Postcode"@en ;
    skos:inScheme cs: ;
    skos:prefLabel "Nofirst-Nolast-Levelno-Postcode"@en ;
    skos:topConceptOf cs: .

:NOF-NOL-PPC a skos:Concept ;
    dcterms:identifier "NOF-NOL-PPC"^^xsd:token ;
    status:status iso19153:original ;
    rdfs:isDefinedBy cs: ;
    skos:definition "Change To Number First, Number Last And Primary Postcode"@en ;
    skos:inScheme cs: ;
    skos:prefLabel "Nofirst-Nolast-Postcode"@en ;
    skos:topConceptOf cs: .

:NOF-PPC a skos:Concept ;
    dcterms:identifier "NOF-PPC"^^xsd:token ;
    status:status iso19153:original ;
    rdfs:isDefinedBy cs: ;
    skos:definition "Change To Number First And Primary Postcode"@en ;
    skos:inScheme cs: ;
    skos:prefLabel "Nofirst-Postcode"@en ;
    skos:topConceptOf cs: .

:NOL a skos:Concept ;
    dcterms:identifier "NOL"^^xsd:token ;
    status:status iso19153:original ;
    rdfs:isDefinedBy cs: ;
    skos:definition "Change To Number Last Only"@en ;
    skos:inScheme cs: ;
    skos:prefLabel "Nolast"@en ;
    skos:topConceptOf cs: .

:NOL-LOT a skos:Concept ;
    dcterms:identifier "NOL-LOT"^^xsd:token ;
    status:status iso19153:original ;
    rdfs:isDefinedBy cs: ;
    skos:definition "Change To Number Last And Lot Number"@en ;
    skos:inScheme cs: ;
    skos:prefLabel "Nolast-Lotno"@en ;
    skos:topConceptOf cs: .

:NOL-LOT-LVN a skos:Concept ;
    dcterms:identifier "NOL-LOT-LVN"^^xsd:token ;
    status:status iso19153:original ;
    rdfs:isDefinedBy cs: ;
    skos:definition "Change To Number Last, Lot Number And Level Number"@en ;
    skos:inScheme cs: ;
    skos:prefLabel "Nolast-Lotno-Levelno"@en ;
    skos:topConceptOf cs: .

:NOL-LOT-LVN-PPC a skos:Concept ;
    dcterms:identifier "NOL-LOT-LVN-PPC"^^xsd:token ;
    status:status iso19153:original ;
    rdfs:isDefinedBy cs: ;
    skos:definition "Change To Number Last, Lot Number, Level Number And Primary Postcode"@en ;
    skos:inScheme cs: ;
    skos:prefLabel "Nolast-Lotno-Levelno-Postcode"@en ;
    skos:topConceptOf cs: .

:NOL-LOT-PPC a skos:Concept ;
    dcterms:identifier "NOL-LOT-PPC"^^xsd:token ;
    status:status iso19153:original ;
    rdfs:isDefinedBy cs: ;
    skos:definition "Change To Number Last, Lot Number And Primary Postcode"@en ;
    skos:inScheme cs: ;
    skos:prefLabel "Nolast-Lotno-Postcode"@en ;
    skos:topConceptOf cs: .

:NOL-LVN a skos:Concept ;
    dcterms:identifier "NOL-LVN"^^xsd:token ;
    status:status iso19153:original ;
    rdfs:isDefinedBy cs: ;
    skos:definition "Change To Number Last And Level Number"@en ;
    skos:inScheme cs: ;
    skos:prefLabel "Nolast-Levelno"@en ;
    skos:topConceptOf cs: .

:NOL-LVN-PPC a skos:Concept ;
    dcterms:identifier "NOL-LVN-PPC"^^xsd:token ;
    status:status iso19153:original ;
    rdfs:isDefinedBy cs: ;
    skos:definition "Change To Number Last, Level Number And Primary Postcode"@en ;
    skos:inScheme cs: ;
    skos:prefLabel "Nolast-Levelno-Postcode"@en ;
    skos:topConceptOf cs: .

:NOL-PPC a skos:Concept ;
    dcterms:identifier "NOL-PPC"^^xsd:token ;
    status:status iso19153:original ;
    rdfs:isDefinedBy cs: ;
    skos:definition "Change To Number Last And Primary Postcode"@en ;
    skos:inScheme cs: ;
    skos:prefLabel "Nolast-Postcode"@en ;
    skos:topConceptOf cs: .

:PPC a skos:Concept ;
    dcterms:identifier "PPC"^^xsd:token ;
    status:status iso19153:original ;
    rdfs:isDefinedBy cs: ;
    skos:definition "Change To Primary Postcode Only"@en ;
    skos:inScheme cs: ;
    skos:prefLabel "Postcode"@en ;
    skos:topConceptOf cs: .

:STN a skos:Concept ;
    dcterms:identifier "STN"^^xsd:token ;
    status:status iso19153:original ;
    rdfs:isDefinedBy cs: ;
    skos:definition "Change To Street Name Only"@en ;
    skos:inScheme cs: ;
    skos:prefLabel "Stname"@en ;
    skos:topConceptOf cs: .

:STN-LOT a skos:Concept ;
    dcterms:identifier "STN-LOT"^^xsd:token ;
    status:status iso19153:original ;
    rdfs:isDefinedBy cs: ;
    skos:definition "Change To Street Name And Lot Number"@en ;
    skos:inScheme cs: ;
    skos:prefLabel "Stname-Lotno"@en ;
    skos:topConceptOf cs: .

:STN-LOT-LVN a skos:Concept ;
    dcterms:identifier "STN-LOT-LVN"^^xsd:token ;
    status:status iso19153:original ;
    rdfs:isDefinedBy cs: ;
    skos:definition "Change To Street Name, Lot Number And Level Number"@en ;
    skos:inScheme cs: ;
    skos:prefLabel "Stname-Lotno-Levelno"@en ;
    skos:topConceptOf cs: .

:STN-LOT-LVN-PPC a skos:Concept ;
    dcterms:identifier "STN-LOT-LVN-PPC"^^xsd:token ;
    status:status iso19153:original ;
    rdfs:isDefinedBy cs: ;
    skos:definition "Change To Street Name, Lot Number, Level Number And Primary Postcode"@en ;
    skos:inScheme cs: ;
    skos:prefLabel "Stname-Lotno-Levelno-Postcode"@en ;
    skos:topConceptOf cs: .

:STN-LOT-PPC a skos:Concept ;
    dcterms:identifier "STN-LOT-PPC"^^xsd:token ;
    status:status iso19153:original ;
    rdfs:isDefinedBy cs: ;
    skos:definition "Change To Street Name, Lot Number And Primary Postcode"@en ;
    skos:inScheme cs: ;
    skos:prefLabel "Stname-Lotno-Postcode"@en ;
    skos:topConceptOf cs: .

:STN-LVN a skos:Concept ;
    dcterms:identifier "STN-LVN"^^xsd:token ;
    status:status iso19153:original ;
    rdfs:isDefinedBy cs: ;
    skos:definition "Change To Street Name And Level Number"@en ;
    skos:inScheme cs: ;
    skos:prefLabel "Stname-Levelno"@en ;
    skos:topConceptOf cs: .

:STN-LVN-PPC a skos:Concept ;
    dcterms:identifier "STN-LVN-PPC"^^xsd:token ;
    status:status iso19153:original ;
    rdfs:isDefinedBy cs: ;
    skos:definition "Change To Street Name, Level Number And Primary Postcode"@en ;
    skos:inScheme cs: ;
    skos:prefLabel "Stname-Levelno-Postcode"@en ;
    skos:topConceptOf cs: .

:STN-NOF a skos:Concept ;
    dcterms:identifier "STN-NOF"^^xsd:token ;
    status:status iso19153:original ;
    rdfs:isDefinedBy cs: ;
    skos:definition "Change To Street Name And Number First"@en ;
    skos:inScheme cs: ;
    skos:prefLabel "Stname-Nofirst"@en ;
    skos:topConceptOf cs: .

:STN-NOF-LOT a skos:Concept ;
    dcterms:identifier "STN-NOF-LOT"^^xsd:token ;
    status:status iso19153:original ;
    rdfs:isDefinedBy cs: ;
    skos:definition "Change To Street Name, Number First And Lot Number"@en ;
    skos:inScheme cs: ;
    skos:prefLabel "Stname-Nofirst-Lotno"@en ;
    skos:topConceptOf cs: .

:STN-NOF-LOT-LVN a skos:Concept ;
    dcterms:identifier "STN-NOF-LOT-LVN"^^xsd:token ;
    status:status iso19153:original ;
    rdfs:isDefinedBy cs: ;
    skos:definition "Change To Street Name, Number First, Lot Number And Level Number"@en ;
    skos:inScheme cs: ;
    skos:prefLabel "Stname-Nofirst-Lotno-Levelno"@en ;
    skos:topConceptOf cs: .

:STN-NOF-LOT-LVN-PPC a skos:Concept ;
    dcterms:identifier "STN-NOF-LOT-LVN-PPC"^^xsd:token ;
    status:status iso19153:original ;
    rdfs:isDefinedBy cs: ;
    skos:definition "Change To Street Name, Number First, Lot Number, Level Number And Primary Postcode"@en ;
    skos:inScheme cs: ;
    skos:prefLabel "Stname-Nofirst-Lotno-Levelno-Postcode"@en ;
    skos:topConceptOf cs: .

:STN-NOF-LOT-PPC a skos:Concept ;
    dcterms:identifier "STN-NOF-LOT-PPC"^^xsd:token ;
    status:status iso19153:original ;
    rdfs:isDefinedBy cs: ;
    skos:definition "Change To Street Name, Number First, Lot Number And Primary Postcode"@en ;
    skos:inScheme cs: ;
    skos:prefLabel "Stname-Nofirst-Lotno-Postcode"@en ;
    skos:topConceptOf cs: .

:STN-NOF-LVN a skos:Concept ;
    dcterms:identifier "STN-NOF-LVN"^^xsd:token ;
    status:status iso19153:original ;
    rdfs:isDefinedBy cs: ;
    skos:definition "Change To Street Name, Number First And Level Number"@en ;
    skos:inScheme cs: ;
    skos:prefLabel "Stname-Nofirst-Levelno"@en ;
    skos:topConceptOf cs: .

:STN-NOF-LVN-PPC a skos:Concept ;
    dcterms:identifier "STN-NOF-LVN-PPC"^^xsd:token ;
    status:status iso19153:original ;
    rdfs:isDefinedBy cs: ;
    skos:definition "Change To Street Name, Number First, Level Number And Primary Postcode"@en ;
    skos:inScheme cs: ;
    skos:prefLabel "Stname-Nofirst-Levelno-Postcode"@en ;
    skos:topConceptOf cs: .

:STN-NOF-NOL a skos:Concept ;
    dcterms:identifier "STN-NOF-NOL"^^xsd:token ;
    status:status iso19153:original ;
    rdfs:isDefinedBy cs: ;
    skos:definition "Change To Street Name, Number First And Number Last"@en ;
    skos:inScheme cs: ;
    skos:prefLabel "Stname-Nofirst-Nolast"@en ;
    skos:topConceptOf cs: .

:STN-NOF-NOL-LOT a skos:Concept ;
    dcterms:identifier "STN-NOF-NOL-LOT"^^xsd:token ;
    status:status iso19153:original ;
    rdfs:isDefinedBy cs: ;
    skos:definition "Change To Street Name, Number First, Number Last And Lot Number"@en ;
    skos:inScheme cs: ;
    skos:prefLabel "Stname-Nofirst-Nolast-Lotno"@en ;
    skos:topConceptOf cs: .

:STN-NOF-NOL-LOT-LVN a skos:Concept ;
    dcterms:identifier "STN-NOF-NOL-LOT-LVN"^^xsd:token ;
    status:status iso19153:original ;
    rdfs:isDefinedBy cs: ;
    skos:definition "Change To Street Name, Number First, Number Last, Lot Number And Level Number"@en ;
    skos:inScheme cs: ;
    skos:prefLabel "Stname-Nofirst-Nolast-Lotno-Levelno"@en ;
    skos:topConceptOf cs: .

:STN-NOF-NOL-LOT-LVN-PPC a skos:Concept ;
    dcterms:identifier "STN-NOF-NOL-LOT-LVN-PPC"^^xsd:token ;
    status:status iso19153:original ;
    rdfs:isDefinedBy cs: ;
    skos:definition "Change To Street Name, Number First, Number Last, Lot Number, Level Number And Primary Postcode"@en ;
    skos:inScheme cs: ;
    skos:prefLabel "Stname-Nofirst-Nolast-Lotno-Levelno-Postcode"@en ;
    skos:topConceptOf cs: .

:STN-NOF-NOL-LOT-PPC a skos:Concept ;
    dcterms:identifier "STN-NOF-NOL-LOT-PPC"^^xsd:token ;
    status:status iso19153:original ;
    rdfs:isDefinedBy cs: ;
    skos:definition "Change To Street Name, Number First, Number Last, Lot Number And Primary Postcode"@en ;
    skos:inScheme cs: ;
    skos:prefLabel "Stname-Nofirst-Nolast-Lotno-Postcode"@en ;
    skos:topConceptOf cs: .

:STN-NOF-NOL-LVN a skos:Concept ;
    dcterms:identifier "STN-NOF-NOL-LVN"^^xsd:token ;
    status:status iso19153:original ;
    rdfs:isDefinedBy cs: ;
    skos:definition "Change To Street Name, Number First, Number Last And Level Number"@en ;
    skos:inScheme cs: ;
    skos:prefLabel "Stname-Nofirst-Nolast-Levelno"@en ;
    skos:topConceptOf cs: .

:STN-NOF-NOL-LVN-PPC a skos:Concept ;
    dcterms:identifier "STN-NOF-NOL-LVN-PPC"^^xsd:token ;
    status:status iso19153:original ;
    rdfs:isDefinedBy cs: ;
    skos:definition "Change To Street Name, Number First, Number Last, Level Number And Primary Postcode"@en ;
    skos:inScheme cs: ;
    skos:prefLabel "Stname-Nofirst-Nolast-Levelno-Postcode"@en ;
    skos:topConceptOf cs: .

:STN-NOF-NOL-PPC a skos:Concept ;
    dcterms:identifier "STN-NOF-NOL-PPC"^^xsd:token ;
    status:status iso19153:original ;
    rdfs:isDefinedBy cs: ;
    skos:definition "Change To Street Name, Number First, Number Last And Primary Postcode"@en ;
    skos:inScheme cs: ;
    skos:prefLabel "Stname-Nofirst-Nolast-Postcode"@en ;
    skos:topConceptOf cs: .

:STN-NOF-PPC a skos:Concept ;
    dcterms:identifier "STN-NOF-PPC"^^xsd:token ;
    status:status iso19153:original ;
    rdfs:isDefinedBy cs: ;
    skos:definition "Change To Street Name, Number First And Primary Postcode"@en ;
    skos:inScheme cs: ;
    skos:prefLabel "Stname-Nofirst-Postcode"@en ;
    skos:topConceptOf cs: .

:STN-NOL a skos:Concept ;
    dcterms:identifier "STN-NOL"^^xsd:token ;
    status:status iso19153:original ;
    rdfs:isDefinedBy cs: ;
    skos:definition "Change To Street Name And Number Last"@en ;
    skos:inScheme cs: ;
    skos:prefLabel "Stname-Nolast"@en ;
    skos:topConceptOf cs: .

:STN-NOL-LOT a skos:Concept ;
    dcterms:identifier "STN-NOL-LOT"^^xsd:token ;
    status:status iso19153:original ;
    rdfs:isDefinedBy cs: ;
    skos:definition "Change To Street Name, Number Last And Lot Number"@en ;
    skos:inScheme cs: ;
    skos:prefLabel "Stname-Nolast-Lotno"@en ;
    skos:topConceptOf cs: .

:STN-NOL-LOT-LVN a skos:Concept ;
    dcterms:identifier "STN-NOL-LOT-LVN"^^xsd:token ;
    status:status iso19153:original ;
    rdfs:isDefinedBy cs: ;
    skos:definition "Change To Street Name, Number Last, Lot Number And Level Number"@en ;
    skos:inScheme cs: ;
    skos:prefLabel "Stname-Nolast-Lotno-Levelno"@en ;
    skos:topConceptOf cs: .

:STN-NOL-LOT-LVN-PPC a skos:Concept ;
    dcterms:identifier "STN-NOL-LOT-LVN-PPC"^^xsd:token ;
    status:status iso19153:original ;
    rdfs:isDefinedBy cs: ;
    skos:definition "Change To Street Name, Number Last, Lot Number, Level Number And Primary Postcode"@en ;
    skos:inScheme cs: ;
    skos:prefLabel "Stname-Nolast-Lotno-Levelno-Postcode"@en ;
    skos:topConceptOf cs: .

:STN-NOL-LOT-PPC a skos:Concept ;
    dcterms:identifier "STN-NOL-LOT-PPC"^^xsd:token ;
    status:status iso19153:original ;
    rdfs:isDefinedBy cs: ;
    skos:definition "Change To Street Name, Number Last, Lot Number And Primary Postcode"@en ;
    skos:inScheme cs: ;
    skos:prefLabel "Stname-Nolast-Lotno-Postcode"@en ;
    skos:topConceptOf cs: .

:STN-NOL-LVN a skos:Concept ;
    dcterms:identifier "STN-NOL-LVN"^^xsd:token ;
    status:status iso19153:original ;
    rdfs:isDefinedBy cs: ;
    skos:definition "Change To Street Name, Number Last And Level Number"@en ;
    skos:inScheme cs: ;
    skos:prefLabel "Stname-Nolast-Levelno"@en ;
    skos:topConceptOf cs: .

:STN-NOL-LVN-PPC a skos:Concept ;
    dcterms:identifier "STN-NOL-LVN-PPC"^^xsd:token ;
    status:status iso19153:original ;
    rdfs:isDefinedBy cs: ;
    skos:definition "Change To Street Name, Number Last, Level Number And Primary Postcode"@en ;
    skos:inScheme cs: ;
    skos:prefLabel "Stname-Nolast-Levelno-Postcode"@en ;
    skos:topConceptOf cs: .

:STN-NOL-PPC a skos:Concept ;
    dcterms:identifier "STN-NOL-PPC"^^xsd:token ;
    status:status iso19153:original ;
    rdfs:isDefinedBy cs: ;
    skos:definition "Change To Street Name, Number Last And Primary Postcode"@en ;
    skos:inScheme cs: ;
    skos:prefLabel "Stname-Nolast-Postcode"@en ;
    skos:topConceptOf cs: .

:STN-PPC a skos:Concept ;
    dcterms:identifier "STN-PPC"^^xsd:token ;
    status:status iso19153:original ;
    rdfs:isDefinedBy cs: ;
    skos:definition "Change To Street Name And Primary Postcode"@en ;
    skos:inScheme cs: ;
    skos:prefLabel "Stname-Postcode"@en ;
    skos:topConceptOf cs: .

:STN-STS a skos:Concept ;
    dcterms:identifier "STN-STS"^^xsd:token ;
    status:status iso19153:original ;
    rdfs:isDefinedBy cs: ;
    skos:definition "Change To Street Name And Street Suffix"@en ;
    skos:inScheme cs: ;
    skos:prefLabel "Stname-Stsuffix"@en ;
    skos:topConceptOf cs: .

:STN-STS-LOT a skos:Concept ;
    dcterms:identifier "STN-STS-LOT"^^xsd:token ;
    status:status iso19153:original ;
    rdfs:isDefinedBy cs: ;
    skos:definition "Change To Street Name, Street Suffix And Lot Number"@en ;
    skos:inScheme cs: ;
    skos:prefLabel "Stname-Stsuffix-Lotno"@en ;
    skos:topConceptOf cs: .

:STN-STS-LOT-LVN a skos:Concept ;
    dcterms:identifier "STN-STS-LOT-LVN"^^xsd:token ;
    status:status iso19153:original ;
    rdfs:isDefinedBy cs: ;
    skos:definition "Change To Street Name, Street Suffix, Lot Number And Level Number"@en ;
    skos:inScheme cs: ;
    skos:prefLabel "Stname-Stsuffix-Lotno-Levelno"@en ;
    skos:topConceptOf cs: .

:STN-STS-LOT-LVN-PPC a skos:Concept ;
    dcterms:identifier "STN-STS-LOT-LVN-PPC"^^xsd:token ;
    status:status iso19153:original ;
    rdfs:isDefinedBy cs: ;
    skos:definition "Change To Street Name, Street Suffix, Lot Number, Level Number And Primary Postcode"@en ;
    skos:inScheme cs: ;
    skos:prefLabel "Stname-Stsuffix-Lotno-Levelno-Postcode"@en ;
    skos:topConceptOf cs: .

:STN-STS-LOT-PPC a skos:Concept ;
    dcterms:identifier "STN-STS-LOT-PPC"^^xsd:token ;
    status:status iso19153:original ;
    rdfs:isDefinedBy cs: ;
    skos:definition "Change To Street Name, Street Suffix, Lot Number And Primary Postcode"@en ;
    skos:inScheme cs: ;
    skos:prefLabel "Stname-Stsuffix-Lotno-Postcode"@en ;
    skos:topConceptOf cs: .

:STN-STS-LVN a skos:Concept ;
    dcterms:identifier "STN-STS-LVN"^^xsd:token ;
    status:status iso19153:original ;
    rdfs:isDefinedBy cs: ;
    skos:definition "Change To Street Name, Street Suffix And Level Number"@en ;
    skos:inScheme cs: ;
    skos:prefLabel "Stname-Stsuffix-Levelno"@en ;
    skos:topConceptOf cs: .

:STN-STS-LVN-PPC a skos:Concept ;
    dcterms:identifier "STN-STS-LVN-PPC"^^xsd:token ;
    status:status iso19153:original ;
    rdfs:isDefinedBy cs: ;
    skos:definition "Change To Street Name, Street Suffix, Level Number And Primary Postcode"@en ;
    skos:inScheme cs: ;
    skos:prefLabel "Stname-Stsuffix-Levelno-Postcode"@en ;
    skos:topConceptOf cs: .

:STN-STS-NOF a skos:Concept ;
    dcterms:identifier "STN-STS-NOF"^^xsd:token ;
    status:status iso19153:original ;
    rdfs:isDefinedBy cs: ;
    skos:definition "Change To Street Name, Street Suffix And Number First"@en ;
    skos:inScheme cs: ;
    skos:prefLabel "Stname-Stsuffix-Nofirst"@en ;
    skos:topConceptOf cs: .

:STN-STS-NOF-LOT a skos:Concept ;
    dcterms:identifier "STN-STS-NOF-LOT"^^xsd:token ;
    status:status iso19153:original ;
    rdfs:isDefinedBy cs: ;
    skos:definition "Change To Street Name, Street Suffix, Number First And Lot Number"@en ;
    skos:inScheme cs: ;
    skos:prefLabel "Stname-Stsuffix-Nofirst-Lotno"@en ;
    skos:topConceptOf cs: .

:STN-STS-NOF-LOT-LVN a skos:Concept ;
    dcterms:identifier "STN-STS-NOF-LOT-LVN"^^xsd:token ;
    status:status iso19153:original ;
    rdfs:isDefinedBy cs: ;
    skos:definition "Change To Street Name, Street Suffix, Number First, Lot Number And Level Number"@en ;
    skos:inScheme cs: ;
    skos:prefLabel "Stname-Stsuffix-Nofirst-Lotno-Levelno"@en ;
    skos:topConceptOf cs: .

:STN-STS-NOF-LOT-LVN-PPC a skos:Concept ;
    dcterms:identifier "STN-STS-NOF-LOT-LVN-PPC"^^xsd:token ;
    status:status iso19153:original ;
    rdfs:isDefinedBy cs: ;
    skos:definition "Change To Street Name, Street Suffix, Number First, Lot Number, Level Number And Primary Postcode"@en ;
    skos:inScheme cs: ;
    skos:prefLabel "Stname-Stsuffix-Nofirst-Lotno-Levelno-Postcode"@en ;
    skos:topConceptOf cs: .

:STN-STS-NOF-LOT-PPC a skos:Concept ;
    dcterms:identifier "STN-STS-NOF-LOT-PPC"^^xsd:token ;
    status:status iso19153:original ;
    rdfs:isDefinedBy cs: ;
    skos:definition "Change To Street Name, Street Suffix, Number First, Lot Number And Primary Postcode"@en ;
    skos:inScheme cs: ;
    skos:prefLabel "Stname-Stsuffix-Nofirst-Lotno-Postcode"@en ;
    skos:topConceptOf cs: .

:STN-STS-NOF-LVN a skos:Concept ;
    dcterms:identifier "STN-STS-NOF-LVN"^^xsd:token ;
    status:status iso19153:original ;
    rdfs:isDefinedBy cs: ;
    skos:definition "Change To Street Name, Street Suffix, Number First And Level Number"@en ;
    skos:inScheme cs: ;
    skos:prefLabel "Stname-Stsuffix-Nofirst-Levelno"@en ;
    skos:topConceptOf cs: .

:STN-STS-NOF-LVN-PPC a skos:Concept ;
    dcterms:identifier "STN-STS-NOF-LVN-PPC"^^xsd:token ;
    status:status iso19153:original ;
    rdfs:isDefinedBy cs: ;
    skos:definition "Change To Street Name, Street Suffix, Number First, Level Number And Primary Postcode"@en ;
    skos:inScheme cs: ;
    skos:prefLabel "Stname-Stsuffix-Nofirst-Levelno-Postcode"@en ;
    skos:topConceptOf cs: .

:STN-STS-NOF-NOL a skos:Concept ;
    dcterms:identifier "STN-STS-NOF-NOL"^^xsd:token ;
    status:status iso19153:original ;
    rdfs:isDefinedBy cs: ;
    skos:definition "Change To Street Name, Street Suffix, Number First And Number Last"@en ;
    skos:inScheme cs: ;
    skos:prefLabel "Stname-Stsuffix-Nofirst-Nolast"@en ;
    skos:topConceptOf cs: .

:STN-STS-NOF-NOL-LOT a skos:Concept ;
    dcterms:identifier "STN-STS-NOF-NOL-LOT"^^xsd:token ;
    status:status iso19153:original ;
    rdfs:isDefinedBy cs: ;
    skos:definition "Change To Street Name, Street Suffix, Number First, Number Last And Lot Number"@en ;
    skos:inScheme cs: ;
    skos:prefLabel "Stname-Stsuffix-Nofirst-Nolast-Lotno"@en ;
    skos:topConceptOf cs: .

:STN-STS-NOF-NOL-LOT-LVN a skos:Concept ;
    dcterms:identifier "STN-STS-NOF-NOL-LOT-LVN"^^xsd:token ;
    status:status iso19153:original ;
    rdfs:isDefinedBy cs: ;
    skos:definition "Change To Street Name, Street Suffix, Number First, Number Last, Lot Number And Level Number"@en ;
    skos:inScheme cs: ;
    skos:prefLabel "Stname-Stsuffix-Nofirst-Nolast-Lotno-Levelno"@en ;
    skos:topConceptOf cs: .

:STN-STS-NOF-NOL-LOT-LVN-PPC a skos:Concept ;
    dcterms:identifier "STN-STS-NOF-NOL-LOT-LVN-PPC"^^xsd:token ;
    status:status iso19153:original ;
    rdfs:isDefinedBy cs: ;
    skos:definition "Change To Street Name, Street Suffix, Number First, Number Last, Lot Number, Level Number And Primary Postcode"@en ;
    skos:inScheme cs: ;
    skos:prefLabel "Stname-Stsuffix-Nofirst-Nolast-Lotno-Levelno-Postcode"@en ;
    skos:topConceptOf cs: .

:STN-STS-NOF-NOL-LOT-PPC a skos:Concept ;
    dcterms:identifier "STN-STS-NOF-NOL-LOT-PPC"^^xsd:token ;
    status:status iso19153:original ;
    rdfs:isDefinedBy cs: ;
    skos:definition "Change To Street Name, Street Suffix, Number First, Number Last, Lot Number And Primary Postcode"@en ;
    skos:inScheme cs: ;
    skos:prefLabel "Stname-Stsuffix-Nofirst-Nolast-Lotno-Postcode"@en ;
    skos:topConceptOf cs: .

:STN-STS-NOF-NOL-LVN a skos:Concept ;
    dcterms:identifier "STN-STS-NOF-NOL-LVN"^^xsd:token ;
    status:status iso19153:original ;
    rdfs:isDefinedBy cs: ;
    skos:definition "Change To Street Name, Street Suffix, Number First, Number Last And Level Number"@en ;
    skos:inScheme cs: ;
    skos:prefLabel "Stname-Stsuffix-Nofirst-Nolast-Levelno"@en ;
    skos:topConceptOf cs: .

:STN-STS-NOF-NOL-LVN-PPC a skos:Concept ;
    dcterms:identifier "STN-STS-NOF-NOL-LVN-PPC"^^xsd:token ;
    status:status iso19153:original ;
    rdfs:isDefinedBy cs: ;
    skos:definition "Change To Street Name, Street Suffix, Number First, Number Last, Level Number And Primary Postcode"@en ;
    skos:inScheme cs: ;
    skos:prefLabel "Stname-Stsuffix-Nofirst-Nolast-Levelno-Postcode"@en ;
    skos:topConceptOf cs: .

:STN-STS-NOF-NOL-PPC a skos:Concept ;
    dcterms:identifier "STN-STS-NOF-NOL-PPC"^^xsd:token ;
    status:status iso19153:original ;
    rdfs:isDefinedBy cs: ;
    skos:definition "Change To Street Name, Street Suffix, Number First, Number Last And Primary Postcode"@en ;
    skos:inScheme cs: ;
    skos:prefLabel "Stname-Stsuffix-Nofirst-Nolast-Postcode"@en ;
    skos:topConceptOf cs: .

:STN-STS-NOF-PPC a skos:Concept ;
    dcterms:identifier "STN-STS-NOF-PPC"^^xsd:token ;
    status:status iso19153:original ;
    rdfs:isDefinedBy cs: ;
    skos:definition "Change To Street Name, Street Suffix, Number First And Primary Postcode"@en ;
    skos:inScheme cs: ;
    skos:prefLabel "Stname-Stsuffix-Nofirst-Postcode"@en ;
    skos:topConceptOf cs: .

:STN-STS-NOL a skos:Concept ;
    dcterms:identifier "STN-STS-NOL"^^xsd:token ;
    status:status iso19153:original ;
    rdfs:isDefinedBy cs: ;
    skos:definition "Change To Street Name, Street Suffix And Number Last"@en ;
    skos:inScheme cs: ;
    skos:prefLabel "Stname-Stsuffix-Nolast"@en ;
    skos:topConceptOf cs: .

:STN-STS-NOL-LOT a skos:Concept ;
    dcterms:identifier "STN-STS-NOL-LOT"^^xsd:token ;
    status:status iso19153:original ;
    rdfs:isDefinedBy cs: ;
    skos:definition "Change To Street Name, Street Suffix, Number Last And Lot Number"@en ;
    skos:inScheme cs: ;
    skos:prefLabel "Stname-Stsuffix-Nolast-Lotno"@en ;
    skos:topConceptOf cs: .

:STN-STS-NOL-LOT-LVN a skos:Concept ;
    dcterms:identifier "STN-STS-NOL-LOT-LVN"^^xsd:token ;
    status:status iso19153:original ;
    rdfs:isDefinedBy cs: ;
    skos:definition "Change To Street Name, Street Suffix, Number Last, Lot Number And Level Number"@en ;
    skos:inScheme cs: ;
    skos:prefLabel "Stname-Stsuffix-Nolast-Lotno-Levelno"@en ;
    skos:topConceptOf cs: .

:STN-STS-NOL-LOT-LVN-PPC a skos:Concept ;
    dcterms:identifier "STN-STS-NOL-LOT-LVN-PPC"^^xsd:token ;
    status:status iso19153:original ;
    rdfs:isDefinedBy cs: ;
    skos:definition "Change To Street Name, Street Suffix, Number Last, Lot Number, Level Number And Primary Postcode"@en ;
    skos:inScheme cs: ;
    skos:prefLabel "Stname-Stsuffix-Nolast-Lotno-Levelno-Postcode"@en ;
    skos:topConceptOf cs: .

:STN-STS-NOL-LOT-PPC a skos:Concept ;
    dcterms:identifier "STN-STS-NOL-LOT-PPC"^^xsd:token ;
    status:status iso19153:original ;
    rdfs:isDefinedBy cs: ;
    skos:definition "Change To Street Name, Street Suffix, Number Last, Lot Number And Primary Postcode"@en ;
    skos:inScheme cs: ;
    skos:prefLabel "Stname-Stsuffix-Nolast-Lotno-Postcode"@en ;
    skos:topConceptOf cs: .

:STN-STS-NOL-LVN a skos:Concept ;
    dcterms:identifier "STN-STS-NOL-LVN"^^xsd:token ;
    status:status iso19153:original ;
    rdfs:isDefinedBy cs: ;
    skos:definition "Change To Street Name, Street Suffix, Number Last And Level Number"@en ;
    skos:inScheme cs: ;
    skos:prefLabel "Stname-Stsuffix-Nolast-Levelno"@en ;
    skos:topConceptOf cs: .

:STN-STS-NOL-LVN-PPC a skos:Concept ;
    dcterms:identifier "STN-STS-NOL-LVN-PPC"^^xsd:token ;
    status:status iso19153:original ;
    rdfs:isDefinedBy cs: ;
    skos:definition "Change To Street Name, Street Suffix, Number Last, Level Number And Primary Postcode"@en ;
    skos:inScheme cs: ;
    skos:prefLabel "Stname-Stsuffix-Nolast-Levelno-Postcode"@en ;
    skos:topConceptOf cs: .

:STN-STS-NOL-PPC a skos:Concept ;
    dcterms:identifier "STN-STS-NOL-PPC"^^xsd:token ;
    status:status iso19153:original ;
    rdfs:isDefinedBy cs: ;
    skos:definition "Change To Street Name, Street Suffix, Number Last And Primary Postcode"@en ;
    skos:inScheme cs: ;
    skos:prefLabel "Stname-Stsuffix-Nolast-Postcode"@en ;
    skos:topConceptOf cs: .

:STN-STS-PPC a skos:Concept ;
    dcterms:identifier "STN-STS-PPC"^^xsd:token ;
    status:status iso19153:original ;
    rdfs:isDefinedBy cs: ;
    skos:definition "Change To Street Name, Street Suffix And Primary Postcode"@en ;
    skos:inScheme cs: ;
    skos:prefLabel "Stname-Stsuffix-Postcode"@en ;
    skos:topConceptOf cs: .

:STN-STT a skos:Concept ;
    dcterms:identifier "STN-STT"^^xsd:token ;
    status:status iso19153:original ;
    rdfs:isDefinedBy cs: ;
    skos:definition "Change To Street Name And Street Type"@en ;
    skos:inScheme cs: ;
    skos:prefLabel "Stname-Sttype"@en ;
    skos:topConceptOf cs: .

:STN-STT-LOT a skos:Concept ;
    dcterms:identifier "STN-STT-LOT"^^xsd:token ;
    status:status iso19153:original ;
    rdfs:isDefinedBy cs: ;
    skos:definition "Change To Street Name, Street Type And Lot Number"@en ;
    skos:inScheme cs: ;
    skos:prefLabel "Stname-Sttype-Lotno"@en ;
    skos:topConceptOf cs: .

:STN-STT-LOT-LVN a skos:Concept ;
    dcterms:identifier "STN-STT-LOT-LVN"^^xsd:token ;
    status:status iso19153:original ;
    rdfs:isDefinedBy cs: ;
    skos:definition "Change To Street Name, Street Type, Lot Number And Level Number"@en ;
    skos:inScheme cs: ;
    skos:prefLabel "Stname-Sttype-Lotno-Levelno"@en ;
    skos:topConceptOf cs: .

:STN-STT-LOT-LVN-PPC a skos:Concept ;
    dcterms:identifier "STN-STT-LOT-LVN-PPC"^^xsd:token ;
    status:status iso19153:original ;
    rdfs:isDefinedBy cs: ;
    skos:definition "Change To Street Name, Street Type, Lot Number, Level Number And Primary Postcode"@en ;
    skos:inScheme cs: ;
    skos:prefLabel "Stname-Sttype-Lotno-Levelno-Postcode"@en ;
    skos:topConceptOf cs: .

:STN-STT-LOT-PPC a skos:Concept ;
    dcterms:identifier "STN-STT-LOT-PPC"^^xsd:token ;
    status:status iso19153:original ;
    rdfs:isDefinedBy cs: ;
    skos:definition "Change To Street Name, Street Type, Lot Number And Primary Postcode"@en ;
    skos:inScheme cs: ;
    skos:prefLabel "Stname-Sttype-Lotno-Postcode"@en ;
    skos:topConceptOf cs: .

:STN-STT-LVN a skos:Concept ;
    dcterms:identifier "STN-STT-LVN"^^xsd:token ;
    status:status iso19153:original ;
    rdfs:isDefinedBy cs: ;
    skos:definition "Change To Street Name, Street Type And Level Number"@en ;
    skos:inScheme cs: ;
    skos:prefLabel "Stname-Sttype-Levelno"@en ;
    skos:topConceptOf cs: .

:STN-STT-LVN-PPC a skos:Concept ;
    dcterms:identifier "STN-STT-LVN-PPC"^^xsd:token ;
    status:status iso19153:original ;
    rdfs:isDefinedBy cs: ;
    skos:definition "Change To Street Name, Street Type, Level Number And Primary Postcode"@en ;
    skos:inScheme cs: ;
    skos:prefLabel "Stname-Sttype-Levelno-Postcode"@en ;
    skos:topConceptOf cs: .

:STN-STT-NOF a skos:Concept ;
    dcterms:identifier "STN-STT-NOF"^^xsd:token ;
    status:status iso19153:original ;
    rdfs:isDefinedBy cs: ;
    skos:definition "Change To Street Name, Street Type And Number First"@en ;
    skos:inScheme cs: ;
    skos:prefLabel "Stname-Sttype-Nofirst"@en ;
    skos:topConceptOf cs: .

:STN-STT-NOF-LOT a skos:Concept ;
    dcterms:identifier "STN-STT-NOF-LOT"^^xsd:token ;
    status:status iso19153:original ;
    rdfs:isDefinedBy cs: ;
    skos:definition "Change To Street Name, Street Type, Number First And Lot Number"@en ;
    skos:inScheme cs: ;
    skos:prefLabel "Stname-Sttype-Nofirst-Lotno"@en ;
    skos:topConceptOf cs: .

:STN-STT-NOF-LOT-LVN a skos:Concept ;
    dcterms:identifier "STN-STT-NOF-LOT-LVN"^^xsd:token ;
    status:status iso19153:original ;
    rdfs:isDefinedBy cs: ;
    skos:definition "Change To Street Name, Street Type, Number First, Lot Number And Level Number"@en ;
    skos:inScheme cs: ;
    skos:prefLabel "Stname-Sttype-Nofirst-Lotno-Levelno"@en ;
    skos:topConceptOf cs: .

:STN-STT-NOF-LOT-LVN-PPC a skos:Concept ;
    dcterms:identifier "STN-STT-NOF-LOT-LVN-PPC"^^xsd:token ;
    status:status iso19153:original ;
    rdfs:isDefinedBy cs: ;
    skos:definition "Change To Street Name, Street Type, Number First, Lot Number, Level Number And Primary Postcode"@en ;
    skos:inScheme cs: ;
    skos:prefLabel "Stname-Sttype-Nofirst-Lotno-Levelno-Postcode"@en ;
    skos:topConceptOf cs: .

:STN-STT-NOF-LOT-PPC a skos:Concept ;
    dcterms:identifier "STN-STT-NOF-LOT-PPC"^^xsd:token ;
    status:status iso19153:original ;
    rdfs:isDefinedBy cs: ;
    skos:definition "Change To Street Name, Street Type, Number First, Lot Number And Primary Postcode"@en ;
    skos:inScheme cs: ;
    skos:prefLabel "Stname-Sttype-Nofirst-Lotno-Postcode"@en ;
    skos:topConceptOf cs: .

:STN-STT-NOF-LVN a skos:Concept ;
    dcterms:identifier "STN-STT-NOF-LVN"^^xsd:token ;
    status:status iso19153:original ;
    rdfs:isDefinedBy cs: ;
    skos:definition "Change To Street Name, Street Type, Number First And Level Number"@en ;
    skos:inScheme cs: ;
    skos:prefLabel "Stname-Sttype-Nofirst-Levelno"@en ;
    skos:topConceptOf cs: .

:STN-STT-NOF-LVN-PPC a skos:Concept ;
    dcterms:identifier "STN-STT-NOF-LVN-PPC"^^xsd:token ;
    status:status iso19153:original ;
    rdfs:isDefinedBy cs: ;
    skos:definition "Change To Street Name, Street Type, Number First, Level Number And Primary Postcode"@en ;
    skos:inScheme cs: ;
    skos:prefLabel "Stname-Sttype-Nofirst-Levelno-Postcode"@en ;
    skos:topConceptOf cs: .

:STN-STT-NOF-NOL a skos:Concept ;
    dcterms:identifier "STN-STT-NOF-NOL"^^xsd:token ;
    status:status iso19153:original ;
    rdfs:isDefinedBy cs: ;
    skos:definition "Change To Street Name, Street Type, Number First And Number Last"@en ;
    skos:inScheme cs: ;
    skos:prefLabel "Stname-Sttype-Nofirst-Nolast"@en ;
    skos:topConceptOf cs: .

:STN-STT-NOF-NOL-LOT a skos:Concept ;
    dcterms:identifier "STN-STT-NOF-NOL-LOT"^^xsd:token ;
    status:status iso19153:original ;
    rdfs:isDefinedBy cs: ;
    skos:definition "Change To Street Name, Street Type, Number First, Number Last And Lot Number"@en ;
    skos:inScheme cs: ;
    skos:prefLabel "Stname-Sttype-Nofirst-Nolast-Lotno"@en ;
    skos:topConceptOf cs: .

:STN-STT-NOF-NOL-LOT-LVN a skos:Concept ;
    dcterms:identifier "STN-STT-NOF-NOL-LOT-LVN"^^xsd:token ;
    status:status iso19153:original ;
    rdfs:isDefinedBy cs: ;
    skos:definition "Change To Street Name, Street Type, Number First, Number Last, Lot Number And Level Number"@en ;
    skos:inScheme cs: ;
    skos:prefLabel "Stname-Sttype-Nofirst-Nolast-Lotno-Levelno"@en ;
    skos:topConceptOf cs: .

:STN-STT-NOF-NOL-LOT-LVN-PPC a skos:Concept ;
    dcterms:identifier "STN-STT-NOF-NOL-LOT-LVN-PPC"^^xsd:token ;
    status:status iso19153:original ;
    rdfs:isDefinedBy cs: ;
    skos:definition "Change To Street Name, Street Type, Number First, Number Last, Lot Number, Level Number And Primary Postcode"@en ;
    skos:inScheme cs: ;
    skos:prefLabel "Stname-Sttype-Nofirst-Nolast-Lotno-Levelno-Postcode"@en ;
    skos:topConceptOf cs: .

:STN-STT-NOF-NOL-LOT-PPC a skos:Concept ;
    dcterms:identifier "STN-STT-NOF-NOL-LOT-PPC"^^xsd:token ;
    status:status iso19153:original ;
    rdfs:isDefinedBy cs: ;
    skos:definition "Change To Street Name, Street Type, Number First, Number Last, Lot Number And Primary Postcode"@en ;
    skos:inScheme cs: ;
    skos:prefLabel "Stname-Sttype-Nofirst-Nolast-Lotno-Postcode"@en ;
    skos:topConceptOf cs: .

:STN-STT-NOF-NOL-LVN a skos:Concept ;
    dcterms:identifier "STN-STT-NOF-NOL-LVN"^^xsd:token ;
    status:status iso19153:original ;
    rdfs:isDefinedBy cs: ;
    skos:definition "Change To Street Name, Street Type, Number First, Number Last And Level Number"@en ;
    skos:inScheme cs: ;
    skos:prefLabel "Stname-Sttype-Nofirst-Nolast-Levelno"@en ;
    skos:topConceptOf cs: .

:STN-STT-NOF-NOL-LVN-PPC a skos:Concept ;
    dcterms:identifier "STN-STT-NOF-NOL-LVN-PPC"^^xsd:token ;
    status:status iso19153:original ;
    rdfs:isDefinedBy cs: ;
    skos:definition "Change To Street Name, Street Type, Number First, Number Last, Level Number And Primary Postcode"@en ;
    skos:inScheme cs: ;
    skos:prefLabel "Stname-Sttype-Nofirst-Nolast-Levelno-Postcode"@en ;
    skos:topConceptOf cs: .

:STN-STT-NOF-NOL-PPC a skos:Concept ;
    dcterms:identifier "STN-STT-NOF-NOL-PPC"^^xsd:token ;
    status:status iso19153:original ;
    rdfs:isDefinedBy cs: ;
    skos:definition "Change To Street Name, Street Type, Number First, Number Last And Primary Postcode"@en ;
    skos:inScheme cs: ;
    skos:prefLabel "Stname-Sttype-Nofirst-Nolast-Postcode"@en ;
    skos:topConceptOf cs: .

:STN-STT-NOF-PPC a skos:Concept ;
    dcterms:identifier "STN-STT-NOF-PPC"^^xsd:token ;
    status:status iso19153:original ;
    rdfs:isDefinedBy cs: ;
    skos:definition "Change To Street Name, Street Type, Number First And Primary Postcode"@en ;
    skos:inScheme cs: ;
    skos:prefLabel "Stname-Sttype-Nofirst-Postcode"@en ;
    skos:topConceptOf cs: .

:STN-STT-NOL a skos:Concept ;
    dcterms:identifier "STN-STT-NOL"^^xsd:token ;
    status:status iso19153:original ;
    rdfs:isDefinedBy cs: ;
    skos:definition "Change To Street Name, Street Type And Number Last"@en ;
    skos:inScheme cs: ;
    skos:prefLabel "Stname-Sttype-Nolast"@en ;
    skos:topConceptOf cs: .

:STN-STT-NOL-LOT a skos:Concept ;
    dcterms:identifier "STN-STT-NOL-LOT"^^xsd:token ;
    status:status iso19153:original ;
    rdfs:isDefinedBy cs: ;
    skos:definition "Change To Street Name, Street Type, Number Last And Lot Number"@en ;
    skos:inScheme cs: ;
    skos:prefLabel "Stname-Sttype-Nolast-Lotno"@en ;
    skos:topConceptOf cs: .

:STN-STT-NOL-LOT-LVN a skos:Concept ;
    dcterms:identifier "STN-STT-NOL-LOT-LVN"^^xsd:token ;
    status:status iso19153:original ;
    rdfs:isDefinedBy cs: ;
    skos:definition "Change To Street Name, Street Type, Number Last, Lot Number And Level Number"@en ;
    skos:inScheme cs: ;
    skos:prefLabel "Stname-Sttype-Nolast-Lotno-Levelno"@en ;
    skos:topConceptOf cs: .

:STN-STT-NOL-LOT-LVN-PPC a skos:Concept ;
    dcterms:identifier "STN-STT-NOL-LOT-LVN-PPC"^^xsd:token ;
    status:status iso19153:original ;
    rdfs:isDefinedBy cs: ;
    skos:definition "Change To Street Name, Street Type, Number Last, Lot Number, Level Number And Primary Postcode"@en ;
    skos:inScheme cs: ;
    skos:prefLabel "Stname-Sttype-Nolast-Lotno-Levelno-Postcode"@en ;
    skos:topConceptOf cs: .

:STN-STT-NOL-LOT-PPC a skos:Concept ;
    dcterms:identifier "STN-STT-NOL-LOT-PPC"^^xsd:token ;
    status:status iso19153:original ;
    rdfs:isDefinedBy cs: ;
    skos:definition "Change To Street Name, Street Type, Number Last, Lot Number And Primary Postcode"@en ;
    skos:inScheme cs: ;
    skos:prefLabel "Stname-Sttype-Nolast-Lotno-Postcode"@en ;
    skos:topConceptOf cs: .

:STN-STT-NOL-LVN a skos:Concept ;
    dcterms:identifier "STN-STT-NOL-LVN"^^xsd:token ;
    status:status iso19153:original ;
    rdfs:isDefinedBy cs: ;
    skos:definition "Change To Street Name, Street Type, Number Last And Level Number"@en ;
    skos:inScheme cs: ;
    skos:prefLabel "Stname-Sttype-Nolast-Levelno"@en ;
    skos:topConceptOf cs: .

:STN-STT-NOL-LVN-PPC a skos:Concept ;
    dcterms:identifier "STN-STT-NOL-LVN-PPC"^^xsd:token ;
    status:status iso19153:original ;
    rdfs:isDefinedBy cs: ;
    skos:definition "Change To Street Name, Street Type, Number Last, Level Number And Primary Postcode"@en ;
    skos:inScheme cs: ;
    skos:prefLabel "Stname-Sttype-Nolast-Levelno-Postcode"@en ;
    skos:topConceptOf cs: .

:STN-STT-NOL-PPC a skos:Concept ;
    dcterms:identifier "STN-STT-NOL-PPC"^^xsd:token ;
    status:status iso19153:original ;
    rdfs:isDefinedBy cs: ;
    skos:definition "Change To Street Name, Street Type, Number Last And Primary Postcode"@en ;
    skos:inScheme cs: ;
    skos:prefLabel "Stname-Sttype-Nolast-Postcode"@en ;
    skos:topConceptOf cs: .

:STN-STT-PPC a skos:Concept ;
    dcterms:identifier "STN-STT-PPC"^^xsd:token ;
    status:status iso19153:original ;
    rdfs:isDefinedBy cs: ;
    skos:definition "Change To Street Name, Street Type And Primary Postcode"@en ;
    skos:inScheme cs: ;
    skos:prefLabel "Stname-Sttype-Postcode"@en ;
    skos:topConceptOf cs: .

:STN-STT-STS a skos:Concept ;
    dcterms:identifier "STN-STT-STS"^^xsd:token ;
    status:status iso19153:original ;
    rdfs:isDefinedBy cs: ;
    skos:definition "Change To Street Name, Street Type And Street Suffix"@en ;
    skos:inScheme cs: ;
    skos:prefLabel "Stname-Sttype-Stsuffix"@en ;
    skos:topConceptOf cs: .

:STN-STT-STS-LOT a skos:Concept ;
    dcterms:identifier "STN-STT-STS-LOT"^^xsd:token ;
    status:status iso19153:original ;
    rdfs:isDefinedBy cs: ;
    skos:definition "Change To Street Name, Street Type, Street Suffix And Lot Number"@en ;
    skos:inScheme cs: ;
    skos:prefLabel "Stname-Sttype-Stsuffix-Lotno"@en ;
    skos:topConceptOf cs: .

:STN-STT-STS-LOT-LVN a skos:Concept ;
    dcterms:identifier "STN-STT-STS-LOT-LVN"^^xsd:token ;
    status:status iso19153:original ;
    rdfs:isDefinedBy cs: ;
    skos:definition "Change To Street Name, Street Type, Street Suffix, Lot Number And Level Number"@en ;
    skos:inScheme cs: ;
    skos:prefLabel "Stname-Sttype-Stsuffix-Lotno-Levelno"@en ;
    skos:topConceptOf cs: .

:STN-STT-STS-LOT-LVN-PPC a skos:Concept ;
    dcterms:identifier "STN-STT-STS-LOT-LVN-PPC"^^xsd:token ;
    status:status iso19153:original ;
    rdfs:isDefinedBy cs: ;
    skos:definition "Change To Street Name, Street Type, Street Suffix, Lot Number, Level Number And Primary Postcode"@en ;
    skos:inScheme cs: ;
    skos:prefLabel "Stname-Sttype-Stsuffix-Lotno-Levelno-Postcode"@en ;
    skos:topConceptOf cs: .

:STN-STT-STS-LOT-PPC a skos:Concept ;
    dcterms:identifier "STN-STT-STS-LOT-PPC"^^xsd:token ;
    status:status iso19153:original ;
    rdfs:isDefinedBy cs: ;
    skos:definition "Change To Street Name, Street Type, Street Suffix, Lot Number And Primary Postcode"@en ;
    skos:inScheme cs: ;
    skos:prefLabel "Stname-Sttype-Stsuffix-Lotno-Postcode"@en ;
    skos:topConceptOf cs: .

:STN-STT-STS-LVN a skos:Concept ;
    dcterms:identifier "STN-STT-STS-LVN"^^xsd:token ;
    status:status iso19153:original ;
    rdfs:isDefinedBy cs: ;
    skos:definition "Change To Street Name, Street Type, Street Suffix And Level Number"@en ;
    skos:inScheme cs: ;
    skos:prefLabel "Stname-Sttype-Stsuffix-Levelno"@en ;
    skos:topConceptOf cs: .

:STN-STT-STS-LVN-PPC a skos:Concept ;
    dcterms:identifier "STN-STT-STS-LVN-PPC"^^xsd:token ;
    status:status iso19153:original ;
    rdfs:isDefinedBy cs: ;
    skos:definition "Change To Street Name, Street Type, Street Suffix, Level Number And Primary Postcode"@en ;
    skos:inScheme cs: ;
    skos:prefLabel "Stname-Sttype-Stsuffix-Levelno-Postcode"@en ;
    skos:topConceptOf cs: .

:STN-STT-STS-NOF a skos:Concept ;
    dcterms:identifier "STN-STT-STS-NOF"^^xsd:token ;
    status:status iso19153:original ;
    rdfs:isDefinedBy cs: ;
    skos:definition "Change To Street Name, Street Type, Street Suffix And Number First"@en ;
    skos:inScheme cs: ;
    skos:prefLabel "Stname-Sttype-Stsuffix-Nofirst"@en ;
    skos:topConceptOf cs: .

:STN-STT-STS-NOF-LOT a skos:Concept ;
    dcterms:identifier "STN-STT-STS-NOF-LOT"^^xsd:token ;
    status:status iso19153:original ;
    rdfs:isDefinedBy cs: ;
    skos:definition "Change To Street Name, Street Type, Street Suffix, Number First And Lot Number"@en ;
    skos:inScheme cs: ;
    skos:prefLabel "Stname-Sttype-Stsuffix-Nofirst-Lotno"@en ;
    skos:topConceptOf cs: .

:STN-STT-STS-NOF-LOT-LVN a skos:Concept ;
    dcterms:identifier "STN-STT-STS-NOF-LOT-LVN"^^xsd:token ;
    status:status iso19153:original ;
    rdfs:isDefinedBy cs: ;
    skos:definition "Change To Street Name, Street Type, Street Suffix, Number First, Lot Number And Level Number"@en ;
    skos:inScheme cs: ;
    skos:prefLabel "Stname-Sttype-Stsuffix-Nofirst-Lotno-Levelno"@en ;
    skos:topConceptOf cs: .

:STN-STT-STS-NOF-LOT-LVN-PPC a skos:Concept ;
    dcterms:identifier "STN-STT-STS-NOF-LOT-LVN-PPC"^^xsd:token ;
    status:status iso19153:original ;
    rdfs:isDefinedBy cs: ;
    skos:definition "Change To Street Name, Street Type, Street Suffix, Number First, Lot Number, Level Number And Primary Postcode"@en ;
    skos:inScheme cs: ;
    skos:prefLabel "Stname-Sttype-Stsuffix-Nofirst-Lotno-Levelno-Postcode"@en ;
    skos:topConceptOf cs: .

:STN-STT-STS-NOF-LOT-PPC a skos:Concept ;
    dcterms:identifier "STN-STT-STS-NOF-LOT-PPC"^^xsd:token ;
    status:status iso19153:original ;
    rdfs:isDefinedBy cs: ;
    skos:definition "Change To Street Name, Street Type, Street Suffix, Number First, Lot Number And Primary Postcode"@en ;
    skos:inScheme cs: ;
    skos:prefLabel "Stname-Sttype-Stsuffix-Nofirst-Lotno-Postcode"@en ;
    skos:topConceptOf cs: .

:STN-STT-STS-NOF-LVN a skos:Concept ;
    dcterms:identifier "STN-STT-STS-NOF-LVN"^^xsd:token ;
    status:status iso19153:original ;
    rdfs:isDefinedBy cs: ;
    skos:definition "Change To Street Name, Street Type, Street Suffix, Number First And Level Number"@en ;
    skos:inScheme cs: ;
    skos:prefLabel "Stname-Sttype-Stsuffix-Nofirst-Levelno"@en ;
    skos:topConceptOf cs: .

:STN-STT-STS-NOF-LVN-PPC a skos:Concept ;
    dcterms:identifier "STN-STT-STS-NOF-LVN-PPC"^^xsd:token ;
    status:status iso19153:original ;
    rdfs:isDefinedBy cs: ;
    skos:definition "Change To Street Name, Street Type, Street Suffix, Number First, Level Number And Primary Postcode"@en ;
    skos:inScheme cs: ;
    skos:prefLabel "Stname-Sttype-Stsuffix-Nofirst-Levelno-Postcode"@en ;
    skos:topConceptOf cs: .

:STN-STT-STS-NOF-NOL a skos:Concept ;
    dcterms:identifier "STN-STT-STS-NOF-NOL"^^xsd:token ;
    status:status iso19153:original ;
    rdfs:isDefinedBy cs: ;
    skos:definition "Change To Street Name, Street Type, Street Suffix, Number First And Number Last"@en ;
    skos:inScheme cs: ;
    skos:prefLabel "Stname-Sttype-Stsuffix-Nofirst-Nolast"@en ;
    skos:topConceptOf cs: .

:STN-STT-STS-NOF-NOL-LOT a skos:Concept ;
    dcterms:identifier "STN-STT-STS-NOF-NOL-LOT"^^xsd:token ;
    status:status iso19153:original ;
    rdfs:isDefinedBy cs: ;
    skos:definition "Change To Street Name, Street Type, Street Suffix, Number First, Number Last And Lot Number"@en ;
    skos:inScheme cs: ;
    skos:prefLabel "Stname-Sttype-Stsuffix-Nofirst-Nolast-Lotno"@en ;
    skos:topConceptOf cs: .

:STN-STT-STS-NOF-NOL-LOT-LVN a skos:Concept ;
    dcterms:identifier "STN-STT-STS-NOF-NOL-LOT-LVN"^^xsd:token ;
    status:status iso19153:original ;
    rdfs:isDefinedBy cs: ;
    skos:definition "Change To Street Name, Street Type, Street Suffix, Number First, Number Last, Lot Number And Level Number"@en ;
    skos:inScheme cs: ;
    skos:prefLabel "Stname-Sttype-Stsuffix-Nofirst-Nolast-Lotno-Levelno"@en ;
    skos:topConceptOf cs: .

:STN-STT-STS-NOF-NOL-LOT-LVN-PPC a skos:Concept ;
    dcterms:identifier "STN-STT-STS-NOF-NOL-LOT-LVN-PPC"^^xsd:token ;
    status:status iso19153:original ;
    rdfs:isDefinedBy cs: ;
    skos:definition "Change To Street Name, Street Type, Street Suffix, Number First, Number Last, Lot Number, Level Number And Primary Postcode"@en ;
    skos:inScheme cs: ;
    skos:prefLabel "Stname-Sttype-Stsuffix-Nofirst-Nolast-Lotno-Levelno-Postcode"@en ;
    skos:topConceptOf cs: .

:STN-STT-STS-NOF-NOL-LOT-PPC a skos:Concept ;
    dcterms:identifier "STN-STT-STS-NOF-NOL-LOT-PPC"^^xsd:token ;
    status:status iso19153:original ;
    rdfs:isDefinedBy cs: ;
    skos:definition "Change To Street Name, Street Type, Street Suffix, Number First, Number Last, Lot Number And Primary Postcode"@en ;
    skos:inScheme cs: ;
    skos:prefLabel "Stname-Sttype-Stsuffix-Nofirst-Nolast-Lotno-Postcode"@en ;
    skos:topConceptOf cs: .

:STN-STT-STS-NOF-NOL-LVN a skos:Concept ;
    dcterms:identifier "STN-STT-STS-NOF-NOL-LVN"^^xsd:token ;
    status:status iso19153:original ;
    rdfs:isDefinedBy cs: ;
    skos:definition "Change To Street Name, Street Type, Street Suffix, Number First, Number Last And Level Number"@en ;
    skos:inScheme cs: ;
    skos:prefLabel "Stname-Sttype-Stsuffix-Nofirst-Nolast-Levelno"@en ;
    skos:topConceptOf cs: .

:STN-STT-STS-NOF-NOL-LVN-PPC a skos:Concept ;
    dcterms:identifier "STN-STT-STS-NOF-NOL-LVN-PPC"^^xsd:token ;
    status:status iso19153:original ;
    rdfs:isDefinedBy cs: ;
    skos:definition "Change To Street Name, Street Type, Street Suffix, Number First, Number Last, Level Number And Primary Postcode"@en ;
    skos:inScheme cs: ;
    skos:prefLabel "Stname-Sttype-Stsuffix-Nofirst-Nolast-Levelno-Postcode"@en ;
    skos:topConceptOf cs: .

:STN-STT-STS-NOF-NOL-PPC a skos:Concept ;
    dcterms:identifier "STN-STT-STS-NOF-NOL-PPC"^^xsd:token ;
    status:status iso19153:original ;
    rdfs:isDefinedBy cs: ;
    skos:definition "Change To Street Name, Street Type, Street Suffix, Number First, Number Last And Primary Postcode"@en ;
    skos:inScheme cs: ;
    skos:prefLabel "Stname-Sttype-Stsuffix-Nofirst-Nolast-Postcode"@en ;
    skos:topConceptOf cs: .

:STN-STT-STS-NOF-PPC a skos:Concept ;
    dcterms:identifier "STN-STT-STS-NOF-PPC"^^xsd:token ;
    status:status iso19153:original ;
    rdfs:isDefinedBy cs: ;
    skos:definition "Change To Street Name, Street Type, Street Suffix, Number First And Primary Postcode"@en ;
    skos:inScheme cs: ;
    skos:prefLabel "Stname-Sttype-Stsuffix-Nofirst-Postcode"@en ;
    skos:topConceptOf cs: .

:STN-STT-STS-NOL a skos:Concept ;
    dcterms:identifier "STN-STT-STS-NOL"^^xsd:token ;
    status:status iso19153:original ;
    rdfs:isDefinedBy cs: ;
    skos:definition "Change To Street Name, Street Type, Street Suffix And Number Last"@en ;
    skos:inScheme cs: ;
    skos:prefLabel "Stname-Sttype-Stsuffix-Nolast"@en ;
    skos:topConceptOf cs: .

:STN-STT-STS-NOL-LOT a skos:Concept ;
    dcterms:identifier "STN-STT-STS-NOL-LOT"^^xsd:token ;
    status:status iso19153:original ;
    rdfs:isDefinedBy cs: ;
    skos:definition "Change To Street Name, Street Type, Street Suffix, Number Last And Lot Number"@en ;
    skos:inScheme cs: ;
    skos:prefLabel "Stname-Sttype-Stsuffix-Nolast-Lotno"@en ;
    skos:topConceptOf cs: .

:STN-STT-STS-NOL-LOT-LVN a skos:Concept ;
    dcterms:identifier "STN-STT-STS-NOL-LOT-LVN"^^xsd:token ;
    status:status iso19153:original ;
    rdfs:isDefinedBy cs: ;
    skos:definition "Change To Street Name, Street Type, Street Suffix, Number Last, Lot Number And Level Number"@en ;
    skos:inScheme cs: ;
    skos:prefLabel "Stname-Sttype-Stsuffix-Nolast-Lotno-Levelno"@en ;
    skos:topConceptOf cs: .

:STN-STT-STS-NOL-LOT-LVN-PPC a skos:Concept ;
    dcterms:identifier "STN-STT-STS-NOL-LOT-LVN-PPC"^^xsd:token ;
    status:status iso19153:original ;
    rdfs:isDefinedBy cs: ;
    skos:definition "Change To Street Name, Street Type, Street Suffix, Number Last, Lot Number, Level Number And Primary Postcode"@en ;
    skos:inScheme cs: ;
    skos:prefLabel "Stname-Sttype-Stsuffix-Nolast-Lotno-Levelno-Postcode"@en ;
    skos:topConceptOf cs: .

:STN-STT-STS-NOL-LOT-PPC a skos:Concept ;
    dcterms:identifier "STN-STT-STS-NOL-LOT-PPC"^^xsd:token ;
    status:status iso19153:original ;
    rdfs:isDefinedBy cs: ;
    skos:definition "Change To Street Name, Street Type, Street Suffix, Number Last, Lot Number And Primary Postcode"@en ;
    skos:inScheme cs: ;
    skos:prefLabel "Stname-Sttype-Stsuffix-Nolast-Lotno-Postcode"@en ;
    skos:topConceptOf cs: .

:STN-STT-STS-NOL-LVN a skos:Concept ;
    dcterms:identifier "STN-STT-STS-NOL-LVN"^^xsd:token ;
    status:status iso19153:original ;
    rdfs:isDefinedBy cs: ;
    skos:definition "Change To Street Name, Street Type, Street Suffix, Number Last And Level Number"@en ;
    skos:inScheme cs: ;
    skos:prefLabel "Stname-Sttype-Stsuffix-Nolast-Levelno"@en ;
    skos:topConceptOf cs: .

:STN-STT-STS-NOL-LVN-PPC a skos:Concept ;
    dcterms:identifier "STN-STT-STS-NOL-LVN-PPC"^^xsd:token ;
    status:status iso19153:original ;
    rdfs:isDefinedBy cs: ;
    skos:definition "Change To Street Name, Street Type, Street Suffix, Number Last, Level Number And Primary Postcode"@en ;
    skos:inScheme cs: ;
    skos:prefLabel "Stname-Sttype-Stsuffix-Nolast-Levelno-Postcode"@en ;
    skos:topConceptOf cs: .

:STN-STT-STS-NOL-PPC a skos:Concept ;
    dcterms:identifier "STN-STT-STS-NOL-PPC"^^xsd:token ;
    status:status iso19153:original ;
    rdfs:isDefinedBy cs: ;
    skos:definition "Change To Street Name, Street Type, Street Suffix, Number Last And Primary Postcode"@en ;
    skos:inScheme cs: ;
    skos:prefLabel "Stname-Sttype-Stsuffix-Nolast-Postcode"@en ;
    skos:topConceptOf cs: .

:STN-STT-STS-PPC a skos:Concept ;
    dcterms:identifier "STN-STT-STS-PPC"^^xsd:token ;
    status:status iso19153:original ;
    rdfs:isDefinedBy cs: ;
    skos:definition "Change To Street Name, Street Type, Street Suffix And Primary Postcode"@en ;
    skos:inScheme cs: ;
    skos:prefLabel "Stname-Sttype-Stsuffix-Postcode"@en ;
    skos:topConceptOf cs: .

:STS a skos:Concept ;
    dcterms:identifier "STS"^^xsd:token ;
    status:status iso19153:original ;
    rdfs:isDefinedBy cs: ;
    skos:definition "Change To Street Suffix Only"@en ;
    skos:inScheme cs: ;
    skos:prefLabel "Stsuffix"@en ;
    skos:topConceptOf cs: .

:STS-LOT a skos:Concept ;
    dcterms:identifier "STS-LOT"^^xsd:token ;
    status:status iso19153:original ;
    rdfs:isDefinedBy cs: ;
    skos:definition "Change To Street Suffix And Lot Number"@en ;
    skos:inScheme cs: ;
    skos:prefLabel "Stsuffix-Lotno"@en ;
    skos:topConceptOf cs: .

:STS-LOT-LVN a skos:Concept ;
    dcterms:identifier "STS-LOT-LVN"^^xsd:token ;
    status:status iso19153:original ;
    rdfs:isDefinedBy cs: ;
    skos:definition "Change To Street Suffix, Lot Number And Level Number"@en ;
    skos:inScheme cs: ;
    skos:prefLabel "Stsuffix-Lotno-Levelno"@en ;
    skos:topConceptOf cs: .

:STS-LOT-LVN-PPC a skos:Concept ;
    dcterms:identifier "STS-LOT-LVN-PPC"^^xsd:token ;
    status:status iso19153:original ;
    rdfs:isDefinedBy cs: ;
    skos:definition "Change To Street Suffix, Lot Number, Level Number And Primary Postcode"@en ;
    skos:inScheme cs: ;
    skos:prefLabel "Stsuffix-Lotno-Levelno-Postcode"@en ;
    skos:topConceptOf cs: .

:STS-LOT-PPC a skos:Concept ;
    dcterms:identifier "STS-LOT-PPC"^^xsd:token ;
    status:status iso19153:original ;
    rdfs:isDefinedBy cs: ;
    skos:definition "Change To Street Suffix, Lot Number And Primary Postcode"@en ;
    skos:inScheme cs: ;
    skos:prefLabel "Stsuffix-Lotno-Postcode"@en ;
    skos:topConceptOf cs: .

:STS-LVN a skos:Concept ;
    dcterms:identifier "STS-LVN"^^xsd:token ;
    status:status iso19153:original ;
    rdfs:isDefinedBy cs: ;
    skos:definition "Change To Street Suffix And Level Number"@en ;
    skos:inScheme cs: ;
    skos:prefLabel "Stsuffix-Levelno"@en ;
    skos:topConceptOf cs: .

:STS-LVN-PPC a skos:Concept ;
    dcterms:identifier "STS-LVN-PPC"^^xsd:token ;
    status:status iso19153:original ;
    rdfs:isDefinedBy cs: ;
    skos:definition "Change To Street Suffix, Level Number And Primary Postcode"@en ;
    skos:inScheme cs: ;
    skos:prefLabel "Stsuffix-Levelno-Postcode"@en ;
    skos:topConceptOf cs: .

:STS-NOF a skos:Concept ;
    dcterms:identifier "STS-NOF"^^xsd:token ;
    status:status iso19153:original ;
    rdfs:isDefinedBy cs: ;
    skos:definition "Change To Street Suffix And Number First"@en ;
    skos:inScheme cs: ;
    skos:prefLabel "Stsuffix-Nofirst"@en ;
    skos:topConceptOf cs: .

:STS-NOF-LOT a skos:Concept ;
    dcterms:identifier "STS-NOF-LOT"^^xsd:token ;
    status:status iso19153:original ;
    rdfs:isDefinedBy cs: ;
    skos:definition "Change To Street Suffix, Number First And Lot Number"@en ;
    skos:inScheme cs: ;
    skos:prefLabel "Stsuffix-Nofirst-Lotno"@en ;
    skos:topConceptOf cs: .

:STS-NOF-LOT-LVN a skos:Concept ;
    dcterms:identifier "STS-NOF-LOT-LVN"^^xsd:token ;
    status:status iso19153:original ;
    rdfs:isDefinedBy cs: ;
    skos:definition "Change To Street Suffix, Number First, Lot Number And Level Number"@en ;
    skos:inScheme cs: ;
    skos:prefLabel "Stsuffix-Nofirst-Lotno-Levelno"@en ;
    skos:topConceptOf cs: .

:STS-NOF-LOT-LVN-PPC a skos:Concept ;
    dcterms:identifier "STS-NOF-LOT-LVN-PPC"^^xsd:token ;
    status:status iso19153:original ;
    rdfs:isDefinedBy cs: ;
    skos:definition "Change To Street Suffix, Number First, Lot Number, Level Number And Primary Postcode"@en ;
    skos:inScheme cs: ;
    skos:prefLabel "Stsuffix-Nofirst-Lotno-Levelno-Postcode"@en ;
    skos:topConceptOf cs: .

:STS-NOF-LOT-PPC a skos:Concept ;
    dcterms:identifier "STS-NOF-LOT-PPC"^^xsd:token ;
    status:status iso19153:original ;
    rdfs:isDefinedBy cs: ;
    skos:definition "Change To Street Suffix, Number First, Lot Number And Primary Postcode"@en ;
    skos:inScheme cs: ;
    skos:prefLabel "Stsuffix-Nofirst-Lotno-Postcode"@en ;
    skos:topConceptOf cs: .

:STS-NOF-LVN a skos:Concept ;
    dcterms:identifier "STS-NOF-LVN"^^xsd:token ;
    status:status iso19153:original ;
    rdfs:isDefinedBy cs: ;
    skos:definition "Change To Street Suffix, Number First And Level Number"@en ;
    skos:inScheme cs: ;
    skos:prefLabel "Stsuffix-Nofirst-Levelno"@en ;
    skos:topConceptOf cs: .

:STS-NOF-LVN-PPC a skos:Concept ;
    dcterms:identifier "STS-NOF-LVN-PPC"^^xsd:token ;
    status:status iso19153:original ;
    rdfs:isDefinedBy cs: ;
    skos:definition "Change To Street Suffix, Number First, Level Number And Primary Postcode"@en ;
    skos:inScheme cs: ;
    skos:prefLabel "Stsuffix-Nofirst-Levelno-Postcode"@en ;
    skos:topConceptOf cs: .

:STS-NOF-NOL a skos:Concept ;
    dcterms:identifier "STS-NOF-NOL"^^xsd:token ;
    status:status iso19153:original ;
    rdfs:isDefinedBy cs: ;
    skos:definition "Change To Street Suffix, Number First And Number Last"@en ;
    skos:inScheme cs: ;
    skos:prefLabel "Stsuffix-Nofirst-Nolast"@en ;
    skos:topConceptOf cs: .

:STS-NOF-NOL-LOT a skos:Concept ;
    dcterms:identifier "STS-NOF-NOL-LOT"^^xsd:token ;
    status:status iso19153:original ;
    rdfs:isDefinedBy cs: ;
    skos:definition "Change To Street Suffix, Number First, Number Last And Lot Number"@en ;
    skos:inScheme cs: ;
    skos:prefLabel "Stsuffix-Nofirst-Nolast-Lotno"@en ;
    skos:topConceptOf cs: .

:STS-NOF-NOL-LOT-LVN a skos:Concept ;
    dcterms:identifier "STS-NOF-NOL-LOT-LVN"^^xsd:token ;
    status:status iso19153:original ;
    rdfs:isDefinedBy cs: ;
    skos:definition "Change To Street Suffix, Number First, Number Last, Lot Number And Level Number"@en ;
    skos:inScheme cs: ;
    skos:prefLabel "Stsuffix-Nofirst-Nolast-Lotno-Levelno"@en ;
    skos:topConceptOf cs: .

:STS-NOF-NOL-LOT-LVN-PPC a skos:Concept ;
    dcterms:identifier "STS-NOF-NOL-LOT-LVN-PPC"^^xsd:token ;
    status:status iso19153:original ;
    rdfs:isDefinedBy cs: ;
    skos:definition "Change To Street Suffix, Number First, Number Last, Lot Number, Level Number And Primary Postcode"@en ;
    skos:inScheme cs: ;
    skos:prefLabel "Stsuffix-Nofirst-Nolast-Lotno-Levelno-Postcode"@en ;
    skos:topConceptOf cs: .

:STS-NOF-NOL-LOT-PPC a skos:Concept ;
    dcterms:identifier "STS-NOF-NOL-LOT-PPC"^^xsd:token ;
    status:status iso19153:original ;
    rdfs:isDefinedBy cs: ;
    skos:definition "Change To Street Suffix, Number First, Number Last, Lot Number And Primary Postcode"@en ;
    skos:inScheme cs: ;
    skos:prefLabel "Stsuffix-Nofirst-Nolast-Lotno-Postcode"@en ;
    skos:topConceptOf cs: .

:STS-NOF-NOL-LVN a skos:Concept ;
    dcterms:identifier "STS-NOF-NOL-LVN"^^xsd:token ;
    status:status iso19153:original ;
    rdfs:isDefinedBy cs: ;
    skos:definition "Change To Street Suffix, Number First, Number Last And Level Number"@en ;
    skos:inScheme cs: ;
    skos:prefLabel "Stsuffix-Nofirst-Nolast-Levelno"@en ;
    skos:topConceptOf cs: .

:STS-NOF-NOL-LVN-PPC a skos:Concept ;
    dcterms:identifier "STS-NOF-NOL-LVN-PPC"^^xsd:token ;
    status:status iso19153:original ;
    rdfs:isDefinedBy cs: ;
    skos:definition "Change To Street Suffix, Number First, Number Last, Level Number And Primary Postcode"@en ;
    skos:inScheme cs: ;
    skos:prefLabel "Stsuffix-Nofirst-Nolast-Levelno-Postcode"@en ;
    skos:topConceptOf cs: .

:STS-NOF-NOL-PPC a skos:Concept ;
    dcterms:identifier "STS-NOF-NOL-PPC"^^xsd:token ;
    status:status iso19153:original ;
    rdfs:isDefinedBy cs: ;
    skos:definition "Change To Street Suffix, Number First, Number Last And Primary Postcode"@en ;
    skos:inScheme cs: ;
    skos:prefLabel "Stsuffix-Nofirst-Nolast-Postcode"@en ;
    skos:topConceptOf cs: .

:STS-NOF-PPC a skos:Concept ;
    dcterms:identifier "STS-NOF-PPC"^^xsd:token ;
    status:status iso19153:original ;
    rdfs:isDefinedBy cs: ;
    skos:definition "Change To Street Suffix, Number First And Primary Postcode"@en ;
    skos:inScheme cs: ;
    skos:prefLabel "Stsuffix-Nofirst-Postcode"@en ;
    skos:topConceptOf cs: .

:STS-NOL a skos:Concept ;
    dcterms:identifier "STS-NOL"^^xsd:token ;
    status:status iso19153:original ;
    rdfs:isDefinedBy cs: ;
    skos:definition "Change To Street Suffix And Number Last"@en ;
    skos:inScheme cs: ;
    skos:prefLabel "Stsuffix-Nolast"@en ;
    skos:topConceptOf cs: .

:STS-NOL-LOT a skos:Concept ;
    dcterms:identifier "STS-NOL-LOT"^^xsd:token ;
    status:status iso19153:original ;
    rdfs:isDefinedBy cs: ;
    skos:definition "Change To Street Suffix, Number Last And Lot Number"@en ;
    skos:inScheme cs: ;
    skos:prefLabel "Stsuffix-Nolast-Lotno"@en ;
    skos:topConceptOf cs: .

:STS-NOL-LOT-LVN a skos:Concept ;
    dcterms:identifier "STS-NOL-LOT-LVN"^^xsd:token ;
    status:status iso19153:original ;
    rdfs:isDefinedBy cs: ;
    skos:definition "Change To Street Suffix, Number Last, Lot Number And Level Number"@en ;
    skos:inScheme cs: ;
    skos:prefLabel "Stsuffix-Nolast-Lotno-Levelno"@en ;
    skos:topConceptOf cs: .

:STS-NOL-LOT-LVN-PPC a skos:Concept ;
    dcterms:identifier "STS-NOL-LOT-LVN-PPC"^^xsd:token ;
    status:status iso19153:original ;
    rdfs:isDefinedBy cs: ;
    skos:definition "Change To Street Suffix, Number Last, Lot Number, Level Number And Primary Postcode"@en ;
    skos:inScheme cs: ;
    skos:prefLabel "Stsuffix-Nolast-Lotno-Levelno-Postcode"@en ;
    skos:topConceptOf cs: .

:STS-NOL-LOT-PPC a skos:Concept ;
    dcterms:identifier "STS-NOL-LOT-PPC"^^xsd:token ;
    status:status iso19153:original ;
    rdfs:isDefinedBy cs: ;
    skos:definition "Change To Street Suffix, Number Last, Lot Number And Primary Postcode"@en ;
    skos:inScheme cs: ;
    skos:prefLabel "Stsuffix-Nolast-Lotno-Postcode"@en ;
    skos:topConceptOf cs: .

:STS-NOL-LVN a skos:Concept ;
    dcterms:identifier "STS-NOL-LVN"^^xsd:token ;
    status:status iso19153:original ;
    rdfs:isDefinedBy cs: ;
    skos:definition "Change To Street Suffix, Number Last And Level Number"@en ;
    skos:inScheme cs: ;
    skos:prefLabel "Stsuffix-Nolast-Levelno"@en ;
    skos:topConceptOf cs: .

:STS-NOL-LVN-PPC a skos:Concept ;
    dcterms:identifier "STS-NOL-LVN-PPC"^^xsd:token ;
    status:status iso19153:original ;
    rdfs:isDefinedBy cs: ;
    skos:definition "Change To Street Suffix, Number Last, Level Number And Primary Postcode"@en ;
    skos:inScheme cs: ;
    skos:prefLabel "Stsuffix-Nolast-Levelno-Postcode"@en ;
    skos:topConceptOf cs: .

:STS-NOL-PPC a skos:Concept ;
    dcterms:identifier "STS-NOL-PPC"^^xsd:token ;
    status:status iso19153:original ;
    rdfs:isDefinedBy cs: ;
    skos:definition "Change To Street Suffix, Number Last And Primary Postcode"@en ;
    skos:inScheme cs: ;
    skos:prefLabel "Stsuffix-Nolast-Postcode"@en ;
    skos:topConceptOf cs: .

:STS-PPC a skos:Concept ;
    dcterms:identifier "STS-PPC"^^xsd:token ;
    status:status iso19153:original ;
    rdfs:isDefinedBy cs: ;
    skos:definition "Change To Street Suffix And Primary Postcode"@en ;
    skos:inScheme cs: ;
    skos:prefLabel "Stsuffix-Postcode"@en ;
    skos:topConceptOf cs: .

:STT a skos:Concept ;
    dcterms:identifier "STT"^^xsd:token ;
    status:status iso19153:original ;
    rdfs:isDefinedBy cs: ;
    skos:definition "Change To Street Type Only"@en ;
    skos:inScheme cs: ;
    skos:prefLabel "Sttype"@en ;
    skos:topConceptOf cs: .

:STT-LOT a skos:Concept ;
    dcterms:identifier "STT-LOT"^^xsd:token ;
    status:status iso19153:original ;
    rdfs:isDefinedBy cs: ;
    skos:definition "Change To Street Type And Lot Number"@en ;
    skos:inScheme cs: ;
    skos:prefLabel "Sttype-Lotno"@en ;
    skos:topConceptOf cs: .

:STT-LOT-LVN a skos:Concept ;
    dcterms:identifier "STT-LOT-LVN"^^xsd:token ;
    status:status iso19153:original ;
    rdfs:isDefinedBy cs: ;
    skos:definition "Change To Street Type, Lot Number And Level Number"@en ;
    skos:inScheme cs: ;
    skos:prefLabel "Sttype-Lotno-Levelno"@en ;
    skos:topConceptOf cs: .

:STT-LOT-LVN-PPC a skos:Concept ;
    dcterms:identifier "STT-LOT-LVN-PPC"^^xsd:token ;
    status:status iso19153:original ;
    rdfs:isDefinedBy cs: ;
    skos:definition "Change To Street Type, Lot Number, Level Number And Primary Postcode"@en ;
    skos:inScheme cs: ;
    skos:prefLabel "Sttype-Lotno-Levelno-Postcode"@en ;
    skos:topConceptOf cs: .

:STT-LOT-PPC a skos:Concept ;
    dcterms:identifier "STT-LOT-PPC"^^xsd:token ;
    status:status iso19153:original ;
    rdfs:isDefinedBy cs: ;
    skos:definition "Change To Street Type, Lot Number And Primary Postcode"@en ;
    skos:inScheme cs: ;
    skos:prefLabel "Sttype-Lotno-Postcode"@en ;
    skos:topConceptOf cs: .

:STT-LVN a skos:Concept ;
    dcterms:identifier "STT-LVN"^^xsd:token ;
    status:status iso19153:original ;
    rdfs:isDefinedBy cs: ;
    skos:definition "Change To Street Type And Level Number"@en ;
    skos:inScheme cs: ;
    skos:prefLabel "Sttype-Levelno"@en ;
    skos:topConceptOf cs: .

:STT-LVN-PPC a skos:Concept ;
    dcterms:identifier "STT-LVN-PPC"^^xsd:token ;
    status:status iso19153:original ;
    rdfs:isDefinedBy cs: ;
    skos:definition "Change To Street Type, Level Number And Primary Postcode"@en ;
    skos:inScheme cs: ;
    skos:prefLabel "Sttype-Levelno-Postcode"@en ;
    skos:topConceptOf cs: .

:STT-NOF a skos:Concept ;
    dcterms:identifier "STT-NOF"^^xsd:token ;
    status:status iso19153:original ;
    rdfs:isDefinedBy cs: ;
    skos:definition "Change To Street Type And Number First"@en ;
    skos:inScheme cs: ;
    skos:prefLabel "Sttype-Nofirst"@en ;
    skos:topConceptOf cs: .

:STT-NOF-LOT a skos:Concept ;
    dcterms:identifier "STT-NOF-LOT"^^xsd:token ;
    status:status iso19153:original ;
    rdfs:isDefinedBy cs: ;
    skos:definition "Change To Street Type, Number First And Lot Number"@en ;
    skos:inScheme cs: ;
    skos:prefLabel "Sttype-Nofirst-Lotno"@en ;
    skos:topConceptOf cs: .

:STT-NOF-LOT-LVN a skos:Concept ;
    dcterms:identifier "STT-NOF-LOT-LVN"^^xsd:token ;
    status:status iso19153:original ;
    rdfs:isDefinedBy cs: ;
    skos:definition "Change To Street Type, Number First, Lot Number And Level Number"@en ;
    skos:inScheme cs: ;
    skos:prefLabel "Sttype-Nofirst-Lotno-Levelno"@en ;
    skos:topConceptOf cs: .

:STT-NOF-LOT-LVN-PPC a skos:Concept ;
    dcterms:identifier "STT-NOF-LOT-LVN-PPC"^^xsd:token ;
    status:status iso19153:original ;
    rdfs:isDefinedBy cs: ;
    skos:definition "Change To Street Type, Number First, Lot Number, Level Number And Primary Postcode"@en ;
    skos:inScheme cs: ;
    skos:prefLabel "Sttype-Nofirst-Lotno-Levelno-Postcode"@en ;
    skos:topConceptOf cs: .

:STT-NOF-LOT-PPC a skos:Concept ;
    dcterms:identifier "STT-NOF-LOT-PPC"^^xsd:token ;
    status:status iso19153:original ;
    rdfs:isDefinedBy cs: ;
    skos:definition "Change To Street Type, Number First, Lot Number And Primary Postcode"@en ;
    skos:inScheme cs: ;
    skos:prefLabel "Sttype-Nofirst-Lotno-Postcode"@en ;
    skos:topConceptOf cs: .

:STT-NOF-LVN a skos:Concept ;
    dcterms:identifier "STT-NOF-LVN"^^xsd:token ;
    status:status iso19153:original ;
    rdfs:isDefinedBy cs: ;
    skos:definition "Change To Street Type, Number First And Level Number"@en ;
    skos:inScheme cs: ;
    skos:prefLabel "Sttype-Nofirst-Levelno"@en ;
    skos:topConceptOf cs: .

:STT-NOF-LVN-PPC a skos:Concept ;
    dcterms:identifier "STT-NOF-LVN-PPC"^^xsd:token ;
    status:status iso19153:original ;
    rdfs:isDefinedBy cs: ;
    skos:definition "Change To Street Type, Number First, Level Number And Primary Postcode"@en ;
    skos:inScheme cs: ;
    skos:prefLabel "Sttype-Nofirst-Levelno-Postcode"@en ;
    skos:topConceptOf cs: .

:STT-NOF-NOL a skos:Concept ;
    dcterms:identifier "STT-NOF-NOL"^^xsd:token ;
    status:status iso19153:original ;
    rdfs:isDefinedBy cs: ;
    skos:definition "Change To Street Type, Number First And Number Last"@en ;
    skos:inScheme cs: ;
    skos:prefLabel "Sttype-Nofirst-Nolast"@en ;
    skos:topConceptOf cs: .

:STT-NOF-NOL-LOT a skos:Concept ;
    dcterms:identifier "STT-NOF-NOL-LOT"^^xsd:token ;
    status:status iso19153:original ;
    rdfs:isDefinedBy cs: ;
    skos:definition "Change To Street Type, Number First, Number Last And Lot Number"@en ;
    skos:inScheme cs: ;
    skos:prefLabel "Sttype-Nofirst-Nolast-Lotno"@en ;
    skos:topConceptOf cs: .

:STT-NOF-NOL-LOT-LVN a skos:Concept ;
    dcterms:identifier "STT-NOF-NOL-LOT-LVN"^^xsd:token ;
    status:status iso19153:original ;
    rdfs:isDefinedBy cs: ;
    skos:definition "Change To Street Type, Number First, Number Last, Lot Number And Level Number"@en ;
    skos:inScheme cs: ;
    skos:prefLabel "Sttype-Nofirst-Nolast-Lotno-Levelno"@en ;
    skos:topConceptOf cs: .

:STT-NOF-NOL-LOT-LVN-PPC a skos:Concept ;
    dcterms:identifier "STT-NOF-NOL-LOT-LVN-PPC"^^xsd:token ;
    status:status iso19153:original ;
    rdfs:isDefinedBy cs: ;
    skos:definition "Change To Street Type, Number First, Number Last, Lot Number, Level Number And Primary Postcode"@en ;
    skos:inScheme cs: ;
    skos:prefLabel "Sttype-Nofirst-Nolast-Lotno-Levelno-Postcode"@en ;
    skos:topConceptOf cs: .

:STT-NOF-NOL-LOT-PPC a skos:Concept ;
    dcterms:identifier "STT-NOF-NOL-LOT-PPC"^^xsd:token ;
    status:status iso19153:original ;
    rdfs:isDefinedBy cs: ;
    skos:definition "Change To Street Type, Number First, Number Last, Lot Number And Primary Postcode"@en ;
    skos:inScheme cs: ;
    skos:prefLabel "Sttype-Nofirst-Nolast-Lotno-Postcode"@en ;
    skos:topConceptOf cs: .

:STT-NOF-NOL-LVN a skos:Concept ;
    dcterms:identifier "STT-NOF-NOL-LVN"^^xsd:token ;
    status:status iso19153:original ;
    rdfs:isDefinedBy cs: ;
    skos:definition "Change To Street Type, Number First, Number Last And Level Number"@en ;
    skos:inScheme cs: ;
    skos:prefLabel "Sttype-Nofirst-Nolast-Levelno"@en ;
    skos:topConceptOf cs: .

:STT-NOF-NOL-LVN-PPC a skos:Concept ;
    dcterms:identifier "STT-NOF-NOL-LVN-PPC"^^xsd:token ;
    status:status iso19153:original ;
    rdfs:isDefinedBy cs: ;
    skos:definition "Change To Street Type, Number First, Number Last, Level Number And Primary Postcode"@en ;
    skos:inScheme cs: ;
    skos:prefLabel "Sttype-Nofirst-Nolast-Levelno-Postcode"@en ;
    skos:topConceptOf cs: .

:STT-NOF-NOL-PPC a skos:Concept ;
    dcterms:identifier "STT-NOF-NOL-PPC"^^xsd:token ;
    status:status iso19153:original ;
    rdfs:isDefinedBy cs: ;
    skos:definition "Change To Street Type, Number First, Number Last And Primary Postcode"@en ;
    skos:inScheme cs: ;
    skos:prefLabel "Sttype-Nofirst-Nolast-Postcode"@en ;
    skos:topConceptOf cs: .

:STT-NOF-PPC a skos:Concept ;
    dcterms:identifier "STT-NOF-PPC"^^xsd:token ;
    status:status iso19153:original ;
    rdfs:isDefinedBy cs: ;
    skos:definition "Change To Street Type, Number First And Primary Postcode"@en ;
    skos:inScheme cs: ;
    skos:prefLabel "Sttype-Nofirst-Postcode"@en ;
    skos:topConceptOf cs: .

:STT-NOL a skos:Concept ;
    dcterms:identifier "STT-NOL"^^xsd:token ;
    status:status iso19153:original ;
    rdfs:isDefinedBy cs: ;
    skos:definition "Change To Street Type And Number Last"@en ;
    skos:inScheme cs: ;
    skos:prefLabel "Sttype-Nolast"@en ;
    skos:topConceptOf cs: .

:STT-NOL-LOT a skos:Concept ;
    dcterms:identifier "STT-NOL-LOT"^^xsd:token ;
    status:status iso19153:original ;
    rdfs:isDefinedBy cs: ;
    skos:definition "Change To Street Type, Number Last And Lot Number"@en ;
    skos:inScheme cs: ;
    skos:prefLabel "Sttype-Nolast-Lotno"@en ;
    skos:topConceptOf cs: .

:STT-NOL-LOT-LVN a skos:Concept ;
    dcterms:identifier "STT-NOL-LOT-LVN"^^xsd:token ;
    status:status iso19153:original ;
    rdfs:isDefinedBy cs: ;
    skos:definition "Change To Street Type, Number Last, Lot Number And Level Number"@en ;
    skos:inScheme cs: ;
    skos:prefLabel "Sttype-Nolast-Lotno-Levelno"@en ;
    skos:topConceptOf cs: .

:STT-NOL-LOT-LVN-PPC a skos:Concept ;
    dcterms:identifier "STT-NOL-LOT-LVN-PPC"^^xsd:token ;
    status:status iso19153:original ;
    rdfs:isDefinedBy cs: ;
    skos:definition "Change To Street Type, Number Last, Lot Number, Level Number And Primary Postcode"@en ;
    skos:inScheme cs: ;
    skos:prefLabel "Sttype-Nolast-Lotno-Levelno-Postcode"@en ;
    skos:topConceptOf cs: .

:STT-NOL-LOT-PPC a skos:Concept ;
    dcterms:identifier "STT-NOL-LOT-PPC"^^xsd:token ;
    status:status iso19153:original ;
    rdfs:isDefinedBy cs: ;
    skos:definition "Change To Street Type, Number Last, Lot Number And Primary Postcode"@en ;
    skos:inScheme cs: ;
    skos:prefLabel "Sttype-Nolast-Lotno-Postcode"@en ;
    skos:topConceptOf cs: .

:STT-NOL-LVN a skos:Concept ;
    dcterms:identifier "STT-NOL-LVN"^^xsd:token ;
    status:status iso19153:original ;
    rdfs:isDefinedBy cs: ;
    skos:definition "Change To Street Type, Number Last And Level Number"@en ;
    skos:inScheme cs: ;
    skos:prefLabel "Sttype-Nolast-Levelno"@en ;
    skos:topConceptOf cs: .

:STT-NOL-LVN-PPC a skos:Concept ;
    dcterms:identifier "STT-NOL-LVN-PPC"^^xsd:token ;
    status:status iso19153:original ;
    rdfs:isDefinedBy cs: ;
    skos:definition "Change To Street Type, Number Last, Level Number And Primary Postcode"@en ;
    skos:inScheme cs: ;
    skos:prefLabel "Sttype-Nolast-Levelno-Postcode"@en ;
    skos:topConceptOf cs: .

:STT-NOL-PPC a skos:Concept ;
    dcterms:identifier "STT-NOL-PPC"^^xsd:token ;
    status:status iso19153:original ;
    rdfs:isDefinedBy cs: ;
    skos:definition "Change To Street Type, Number Last And Primary Postcode"@en ;
    skos:inScheme cs: ;
    skos:prefLabel "Sttype-Nolast-Postcode"@en ;
    skos:topConceptOf cs: .

:STT-PPC a skos:Concept ;
    dcterms:identifier "STT-PPC"^^xsd:token ;
    status:status iso19153:original ;
    rdfs:isDefinedBy cs: ;
    skos:definition "Change To Street Type And Primary Postcode"@en ;
    skos:inScheme cs: ;
    skos:prefLabel "Sttype-Postcode"@en ;
    skos:topConceptOf cs: .

:STT-STS a skos:Concept ;
    dcterms:identifier "STT-STS"^^xsd:token ;
    status:status iso19153:original ;
    rdfs:isDefinedBy cs: ;
    skos:definition "Change To Street Type And Street Suffix"@en ;
    skos:inScheme cs: ;
    skos:prefLabel "Sttype-Stsuffix"@en ;
    skos:topConceptOf cs: .

:STT-STS-LOT a skos:Concept ;
    dcterms:identifier "STT-STS-LOT"^^xsd:token ;
    status:status iso19153:original ;
    rdfs:isDefinedBy cs: ;
    skos:definition "Change To Street Type, Street Suffix And Lot Number"@en ;
    skos:inScheme cs: ;
    skos:prefLabel "Sttype-Stsuffix-Lotno"@en ;
    skos:topConceptOf cs: .

:STT-STS-LOT-LVN a skos:Concept ;
    dcterms:identifier "STT-STS-LOT-LVN"^^xsd:token ;
    status:status iso19153:original ;
    rdfs:isDefinedBy cs: ;
    skos:definition "Change To Street Type, Street Suffix, Lot Number And Level Number"@en ;
    skos:inScheme cs: ;
    skos:prefLabel "Sttype-Stsuffix-Lotno-Levelno"@en ;
    skos:topConceptOf cs: .

:STT-STS-LOT-LVN-PPC a skos:Concept ;
    dcterms:identifier "STT-STS-LOT-LVN-PPC"^^xsd:token ;
    status:status iso19153:original ;
    rdfs:isDefinedBy cs: ;
    skos:definition "Change To Street Type, Street Suffix, Lot Number, Level Number And Primary Postcode"@en ;
    skos:inScheme cs: ;
    skos:prefLabel "Sttype-Stsuffix-Lotno-Levelno-Postcode"@en ;
    skos:topConceptOf cs: .

:STT-STS-LOT-PPC a skos:Concept ;
    dcterms:identifier "STT-STS-LOT-PPC"^^xsd:token ;
    status:status iso19153:original ;
    rdfs:isDefinedBy cs: ;
    skos:definition "Change To Street Type, Street Suffix, Lot Number And Primary Postcode"@en ;
    skos:inScheme cs: ;
    skos:prefLabel "Sttype-Stsuffix-Lotno-Postcode"@en ;
    skos:topConceptOf cs: .

:STT-STS-LVN a skos:Concept ;
    dcterms:identifier "STT-STS-LVN"^^xsd:token ;
    status:status iso19153:original ;
    rdfs:isDefinedBy cs: ;
    skos:definition "Change To Street Type, Street Suffix And Level Number"@en ;
    skos:inScheme cs: ;
    skos:prefLabel "Sttype-Stsuffix-Levelno"@en ;
    skos:topConceptOf cs: .

:STT-STS-LVN-PPC a skos:Concept ;
    dcterms:identifier "STT-STS-LVN-PPC"^^xsd:token ;
    status:status iso19153:original ;
    rdfs:isDefinedBy cs: ;
    skos:definition "Change To Street Type, Street Suffix, Level Number And Primary Postcode"@en ;
    skos:inScheme cs: ;
    skos:prefLabel "Sttype-Stsuffix-Levelno-Postcode"@en ;
    skos:topConceptOf cs: .

:STT-STS-NOF a skos:Concept ;
    dcterms:identifier "STT-STS-NOF"^^xsd:token ;
    status:status iso19153:original ;
    rdfs:isDefinedBy cs: ;
    skos:definition "Change To Street Type, Street Suffix And Number First"@en ;
    skos:inScheme cs: ;
    skos:prefLabel "Sttype-Stsuffix-Nofirst"@en ;
    skos:topConceptOf cs: .

:STT-STS-NOF-LOT a skos:Concept ;
    dcterms:identifier "STT-STS-NOF-LOT"^^xsd:token ;
    status:status iso19153:original ;
    rdfs:isDefinedBy cs: ;
    skos:definition "Change To Street Type, Street Suffix, Number First And Lot Number"@en ;
    skos:inScheme cs: ;
    skos:prefLabel "Sttype-Stsuffix-Nofirst-Lotno"@en ;
    skos:topConceptOf cs: .

:STT-STS-NOF-LOT-LVN a skos:Concept ;
    dcterms:identifier "STT-STS-NOF-LOT-LVN"^^xsd:token ;
    status:status iso19153:original ;
    rdfs:isDefinedBy cs: ;
    skos:definition "Change To Street Type, Street Suffix, Number First, Lot Number And Level Number"@en ;
    skos:inScheme cs: ;
    skos:prefLabel "Sttype-Stsuffix-Nofirst-Lotno-Levelno"@en ;
    skos:topConceptOf cs: .

:STT-STS-NOF-LOT-LVN-PPC a skos:Concept ;
    dcterms:identifier "STT-STS-NOF-LOT-LVN-PPC"^^xsd:token ;
    status:status iso19153:original ;
    rdfs:isDefinedBy cs: ;
    skos:definition "Change To Street Type, Street Suffix, Number First, Lot Number, Level Number And Primary Postcode"@en ;
    skos:inScheme cs: ;
    skos:prefLabel "Sttype-Stsuffix-Nofirst-Lotno-Levelno-Postcode"@en ;
    skos:topConceptOf cs: .

:STT-STS-NOF-LOT-PPC a skos:Concept ;
    dcterms:identifier "STT-STS-NOF-LOT-PPC"^^xsd:token ;
    status:status iso19153:original ;
    rdfs:isDefinedBy cs: ;
    skos:definition "Change To Street Type, Street Suffix, Number First, Lot Number And Primary Postcode"@en ;
    skos:inScheme cs: ;
    skos:prefLabel "Sttype-Stsuffix-Nofirst-Lotno-Postcode"@en ;
    skos:topConceptOf cs: .

:STT-STS-NOF-LVN a skos:Concept ;
    dcterms:identifier "STT-STS-NOF-LVN"^^xsd:token ;
    status:status iso19153:original ;
    rdfs:isDefinedBy cs: ;
    skos:definition "Change To Street Type, Street Suffix, Number First And Level Number"@en ;
    skos:inScheme cs: ;
    skos:prefLabel "Sttype-Stsuffix-Nofirst-Levelno"@en ;
    skos:topConceptOf cs: .

:STT-STS-NOF-LVN-PPC a skos:Concept ;
    dcterms:identifier "STT-STS-NOF-LVN-PPC"^^xsd:token ;
    status:status iso19153:original ;
    rdfs:isDefinedBy cs: ;
    skos:definition "Change To Street Type, Street Suffix, Number First, Level Number And Primary Postcode"@en ;
    skos:inScheme cs: ;
    skos:prefLabel "Sttype-Stsuffix-Nofirst-Levelno-Postcode"@en ;
    skos:topConceptOf cs: .

:STT-STS-NOF-NOL a skos:Concept ;
    dcterms:identifier "STT-STS-NOF-NOL"^^xsd:token ;
    status:status iso19153:original ;
    rdfs:isDefinedBy cs: ;
    skos:definition "Change To Street Type, Street Suffix, Number First And Number Last"@en ;
    skos:inScheme cs: ;
    skos:prefLabel "Sttype-Stsuffix-Nofirst-Nolast"@en ;
    skos:topConceptOf cs: .

:STT-STS-NOF-NOL-LOT a skos:Concept ;
    dcterms:identifier "STT-STS-NOF-NOL-LOT"^^xsd:token ;
    status:status iso19153:original ;
    rdfs:isDefinedBy cs: ;
    skos:definition "Change To Street Type, Street Suffix, Number First, Number Last And Lot Number"@en ;
    skos:inScheme cs: ;
    skos:prefLabel "Sttype-Stsuffix-Nofirst-Nolast-Lotno"@en ;
    skos:topConceptOf cs: .

:STT-STS-NOF-NOL-LOT-LVN a skos:Concept ;
    dcterms:identifier "STT-STS-NOF-NOL-LOT-LVN"^^xsd:token ;
    status:status iso19153:original ;
    rdfs:isDefinedBy cs: ;
    skos:definition "Change To Street Type, Street Suffix, Number First, Number Last, Lot Number And Level Number"@en ;
    skos:inScheme cs: ;
    skos:prefLabel "Sttype-Stsuffix-Nofirst-Nolast-Lotno-Levelno"@en ;
    skos:topConceptOf cs: .

:STT-STS-NOF-NOL-LOT-LVN-PPC a skos:Concept ;
    dcterms:identifier "STT-STS-NOF-NOL-LOT-LVN-PPC"^^xsd:token ;
    status:status iso19153:original ;
    rdfs:isDefinedBy cs: ;
    skos:definition "Change To Street Type, Street Suffix, Number First, Number Last, Lot Number, Level Number And Primary Postcode"@en ;
    skos:inScheme cs: ;
    skos:prefLabel "Sttype-Stsuffix-Nofirst-Nolast-Lotno-Levelno-Postcode"@en ;
    skos:topConceptOf cs: .

:STT-STS-NOF-NOL-LOT-PPC a skos:Concept ;
    dcterms:identifier "STT-STS-NOF-NOL-LOT-PPC"^^xsd:token ;
    status:status iso19153:original ;
    rdfs:isDefinedBy cs: ;
    skos:definition "Change To Street Type, Street Suffix, Number First, Number Last, Lot Number And Primary Postcode"@en ;
    skos:inScheme cs: ;
    skos:prefLabel "Sttype-Stsuffix-Nofirst-Nolast-Lotno-Postcode"@en ;
    skos:topConceptOf cs: .

:STT-STS-NOF-NOL-LVN a skos:Concept ;
    dcterms:identifier "STT-STS-NOF-NOL-LVN"^^xsd:token ;
    status:status iso19153:original ;
    rdfs:isDefinedBy cs: ;
    skos:definition "Change To Street Type, Street Suffix, Number First, Number Last And Level Number"@en ;
    skos:inScheme cs: ;
    skos:prefLabel "Sttype-Stsuffix-Nofirst-Nolast-Levelno"@en ;
    skos:topConceptOf cs: .

:STT-STS-NOF-NOL-LVN-PPC a skos:Concept ;
    dcterms:identifier "STT-STS-NOF-NOL-LVN-PPC"^^xsd:token ;
    status:status iso19153:original ;
    rdfs:isDefinedBy cs: ;
    skos:definition "Change To Street Type, Street Suffix, Number First, Number Last, Level Number And Primary Postcode"@en ;
    skos:inScheme cs: ;
    skos:prefLabel "Sttype-Stsuffix-Nofirst-Nolast-Levelno-Postcode"@en ;
    skos:topConceptOf cs: .

:STT-STS-NOF-NOL-PPC a skos:Concept ;
    dcterms:identifier "STT-STS-NOF-NOL-PPC"^^xsd:token ;
    status:status iso19153:original ;
    rdfs:isDefinedBy cs: ;
    skos:definition "Change To Street Type, Street Suffix, Number First, Number Last And Primary Postcode"@en ;
    skos:inScheme cs: ;
    skos:prefLabel "Sttype-Stsuffix-Nofirst-Nolast-Postcode"@en ;
    skos:topConceptOf cs: .

:STT-STS-NOF-PPC a skos:Concept ;
    dcterms:identifier "STT-STS-NOF-PPC"^^xsd:token ;
    status:status iso19153:original ;
    rdfs:isDefinedBy cs: ;
    skos:definition "Change To Street Type, Street Suffix, Number First And Primary Postcode"@en ;
    skos:inScheme cs: ;
    skos:prefLabel "Sttype-Stsuffix-Nofirst-Postcode"@en ;
    skos:topConceptOf cs: .

:STT-STS-NOL a skos:Concept ;
    dcterms:identifier "STT-STS-NOL"^^xsd:token ;
    status:status iso19153:original ;
    rdfs:isDefinedBy cs: ;
    skos:definition "Change To Street Type, Street Suffix And Number Last"@en ;
    skos:inScheme cs: ;
    skos:prefLabel "Sttype-Stsuffix-Nolast"@en ;
    skos:topConceptOf cs: .

:STT-STS-NOL-LOT a skos:Concept ;
    dcterms:identifier "STT-STS-NOL-LOT"^^xsd:token ;
    status:status iso19153:original ;
    rdfs:isDefinedBy cs: ;
    skos:definition "Change To Street Type, Street Suffix, Number Last And Lot Number"@en ;
    skos:inScheme cs: ;
    skos:prefLabel "Sttype-Stsuffix-Nolast-Lotno"@en ;
    skos:topConceptOf cs: .

:STT-STS-NOL-LOT-LVN a skos:Concept ;
    dcterms:identifier "STT-STS-NOL-LOT-LVN"^^xsd:token ;
    status:status iso19153:original ;
    rdfs:isDefinedBy cs: ;
    skos:definition "Change To Street Type, Street Suffix, Number Last, Lot Number And Level Number"@en ;
    skos:inScheme cs: ;
    skos:prefLabel "Sttype-Stsuffix-Nolast-Lotno-Levelno"@en ;
    skos:topConceptOf cs: .

:STT-STS-NOL-LOT-LVN-PPC a skos:Concept ;
    dcterms:identifier "STT-STS-NOL-LOT-LVN-PPC"^^xsd:token ;
    status:status iso19153:original ;
    rdfs:isDefinedBy cs: ;
    skos:definition "Change To Street Type, Street Suffix, Number Last, Lot Number, Level Number And Primary Postcode"@en ;
    skos:inScheme cs: ;
    skos:prefLabel "Sttype-Stsuffix-Nolast-Lotno-Levelno-Postcode"@en ;
    skos:topConceptOf cs: .

:STT-STS-NOL-LOT-PPC a skos:Concept ;
    dcterms:identifier "STT-STS-NOL-LOT-PPC"^^xsd:token ;
    status:status iso19153:original ;
    rdfs:isDefinedBy cs: ;
    skos:definition "Change To Street Type, Street Suffix, Number Last, Lot Number And Primary Postcode"@en ;
    skos:inScheme cs: ;
    skos:prefLabel "Sttype-Stsuffix-Nolast-Lotno-Postcode"@en ;
    skos:topConceptOf cs: .

:STT-STS-NOL-LVN a skos:Concept ;
    dcterms:identifier "STT-STS-NOL-LVN"^^xsd:token ;
    status:status iso19153:original ;
    rdfs:isDefinedBy cs: ;
    skos:definition "Change To Street Type, Street Suffix, Number Last And Level Number"@en ;
    skos:inScheme cs: ;
    skos:prefLabel "Sttype-Stsuffix-Nolast-Levelno"@en ;
    skos:topConceptOf cs: .

:STT-STS-NOL-LVN-PPC a skos:Concept ;
    dcterms:identifier "STT-STS-NOL-LVN-PPC"^^xsd:token ;
    status:status iso19153:original ;
    rdfs:isDefinedBy cs: ;
    skos:definition "Change To Street Type, Street Suffix, Number Last, Level Number And Primary Postcode"@en ;
    skos:inScheme cs: ;
    skos:prefLabel "Sttype-Stsuffix-Nolast-Levelno-Postcode"@en ;
    skos:topConceptOf cs: .

:STT-STS-NOL-PPC a skos:Concept ;
    dcterms:identifier "STT-STS-NOL-PPC"^^xsd:token ;
    status:status iso19153:original ;
    rdfs:isDefinedBy cs: ;
    skos:definition "Change To Street Type, Street Suffix, Number Last And Primary Postcode"@en ;
    skos:inScheme cs: ;
    skos:prefLabel "Sttype-Stsuffix-Nolast-Postcode"@en ;
    skos:topConceptOf cs: .

:STT-STS-PPC a skos:Concept ;
    dcterms:identifier "STT-STS-PPC"^^xsd:token ;
    status:status iso19153:original ;
    rdfs:isDefinedBy cs: ;
    skos:definition "Change To Street Type, Street Suffix And Primary Postcode"@en ;
    skos:inScheme cs: ;
    skos:prefLabel "Sttype-Stsuffix-Postcode"@en ;
    skos:topConceptOf cs: .

cs: a skos:ConceptScheme ;
    dcterms:created "2018-02-10"^^xsd:date ;
    dcterms:identifier "addressChangeType"^^xsd:token ;
    dcterms:modified "2022-05-30"^^xsd:date ;
    dcterms:provenance "Automatically created from the G-NAF codelists"@en ;
    skos:definition "Description of address change type code"@en ;
    skos:hasTopConcept :LOC,
        :LOC-LOT,
        :LOC-LOT-LVN,
        :LOC-LOT-LVN-PPC,
        :LOC-LOT-PPC,
        :LOC-LVN,
        :LOC-LVN-PPC,
        :LOC-NOF,
        :LOC-NOF-LOT,
        :LOC-NOF-LOT-LVN,
        :LOC-NOF-LOT-LVN-PPC,
        :LOC-NOF-LOT-PPC,
        :LOC-NOF-LVN,
        :LOC-NOF-LVN-PPC,
        :LOC-NOF-NOL,
        :LOC-NOF-NOL-LOT,
        :LOC-NOF-NOL-LOT-LVN,
        :LOC-NOF-NOL-LOT-LVN-PPC,
        :LOC-NOF-NOL-LOT-PPC,
        :LOC-NOF-NOL-LVN,
        :LOC-NOF-NOL-LVN-PPC,
        :LOC-NOF-NOL-PPC,
        :LOC-NOF-PPC,
        :LOC-NOL,
        :LOC-NOL-LOT,
        :LOC-NOL-LOT-LVN,
        :LOC-NOL-LOT-LVN-PPC,
        :LOC-NOL-LOT-PPC,
        :LOC-NOL-LVN,
        :LOC-NOL-LVN-PPC,
        :LOC-NOL-PPC,
        :LOC-PPC,
        :LOC-STN,
        :LOC-STN-LOT,
        :LOC-STN-LOT-LVN,
        :LOC-STN-LOT-LVN-PPC,
        :LOC-STN-LOT-PPC,
        :LOC-STN-LVN,
        :LOC-STN-LVN-PPC,
        :LOC-STN-NOF,
        :LOC-STN-NOF-LOT,
        :LOC-STN-NOF-LOT-LVN,
        :LOC-STN-NOF-LOT-LVN-PPC,
        :LOC-STN-NOF-LOT-PPC,
        :LOC-STN-NOF-LVN,
        :LOC-STN-NOF-LVN-PPC,
        :LOC-STN-NOF-NOL,
        :LOC-STN-NOF-NOL-LOT,
        :LOC-STN-NOF-NOL-LOT-LVN,
        :LOC-STN-NOF-NOL-LOT-LVN-PPC,
        :LOC-STN-NOF-NOL-LOT-PPC,
        :LOC-STN-NOF-NOL-LVN,
        :LOC-STN-NOF-NOL-LVN-PPC,
        :LOC-STN-NOF-NOL-PPC,
        :LOC-STN-NOF-PPC,
        :LOC-STN-NOL,
        :LOC-STN-NOL-LOT,
        :LOC-STN-NOL-LOT-LVN,
        :LOC-STN-NOL-LOT-LVN-PPC,
        :LOC-STN-NOL-LOT-PPC,
        :LOC-STN-NOL-LVN,
        :LOC-STN-NOL-LVN-PPC,
        :LOC-STN-NOL-PPC,
        :LOC-STN-PPC,
        :LOC-STN-STS,
        :LOC-STN-STS-LOT,
        :LOC-STN-STS-LOT-LVN,
        :LOC-STN-STS-LOT-LVN-PPC,
        :LOC-STN-STS-LOT-PPC,
        :LOC-STN-STS-LVN,
        :LOC-STN-STS-LVN-PPC,
        :LOC-STN-STS-NOF,
        :LOC-STN-STS-NOF-LOT,
        :LOC-STN-STS-NOF-LOT-LVN,
        :LOC-STN-STS-NOF-LOT-LVN-PPC,
        :LOC-STN-STS-NOF-LOT-PPC,
        :LOC-STN-STS-NOF-LVN,
        :LOC-STN-STS-NOF-LVN-PPC,
        :LOC-STN-STS-NOF-NOL,
        :LOC-STN-STS-NOF-NOL-LOT,
        :LOC-STN-STS-NOF-NOL-LOT-LVN,
        :LOC-STN-STS-NOF-NOL-LOT-LVN-PPC,
        :LOC-STN-STS-NOF-NOL-LOT-PPC,
        :LOC-STN-STS-NOF-NOL-LVN,
        :LOC-STN-STS-NOF-NOL-LVN-PPC,
        :LOC-STN-STS-NOF-NOL-PPC,
        :LOC-STN-STS-NOF-PPC,
        :LOC-STN-STS-NOL,
        :LOC-STN-STS-NOL-LOT,
        :LOC-STN-STS-NOL-LOT-LVN,
        :LOC-STN-STS-NOL-LOT-LVN-PPC,
        :LOC-STN-STS-NOL-LOT-PPC,
        :LOC-STN-STS-NOL-LVN,
        :LOC-STN-STS-NOL-LVN-PPC,
        :LOC-STN-STS-NOL-PPC,
        :LOC-STN-STS-PPC,
        :LOC-STN-STT,
        :LOC-STN-STT-LOT,
        :LOC-STN-STT-LOT-LVN,
        :LOC-STN-STT-LOT-LVN-PPC,
        :LOC-STN-STT-LOT-PPC,
        :LOC-STN-STT-LVN,
        :LOC-STN-STT-LVN-PPC,
        :LOC-STN-STT-NOF,
        :LOC-STN-STT-NOF-LOT,
        :LOC-STN-STT-NOF-LOT-LVN,
        :LOC-STN-STT-NOF-LOT-LVN-PPC,
        :LOC-STN-STT-NOF-LOT-PPC,
        :LOC-STN-STT-NOF-LVN,
        :LOC-STN-STT-NOF-LVN-PPC,
        :LOC-STN-STT-NOF-NOL,
        :LOC-STN-STT-NOF-NOL-LOT,
        :LOC-STN-STT-NOF-NOL-LOT-LVN,
        :LOC-STN-STT-NOF-NOL-LOT-LVN-PPC,
        :LOC-STN-STT-NOF-NOL-LOT-PPC,
        :LOC-STN-STT-NOF-NOL-LVN,
        :LOC-STN-STT-NOF-NOL-LVN-PPC,
        :LOC-STN-STT-NOF-NOL-PPC,
        :LOC-STN-STT-NOF-PPC,
        :LOC-STN-STT-NOL,
        :LOC-STN-STT-NOL-LOT,
        :LOC-STN-STT-NOL-LOT-LVN,
        :LOC-STN-STT-NOL-LOT-LVN-PPC,
        :LOC-STN-STT-NOL-LOT-PPC,
        :LOC-STN-STT-NOL-LVN,
        :LOC-STN-STT-NOL-LVN-PPC,
        :LOC-STN-STT-NOL-PPC,
        :LOC-STN-STT-PPC,
        :LOC-STN-STT-STS,
        :LOC-STN-STT-STS-LOT,
        :LOC-STN-STT-STS-LOT-LVN,
        :LOC-STN-STT-STS-LOT-LVN-PPC,
        :LOC-STN-STT-STS-LOT-PPC,
        :LOC-STN-STT-STS-LVN,
        :LOC-STN-STT-STS-LVN-PPC,
        :LOC-STN-STT-STS-NOF,
        :LOC-STN-STT-STS-NOF-LOT,
        :LOC-STN-STT-STS-NOF-LOT-LVN,
        :LOC-STN-STT-STS-NOF-LOT-LVN-PPC,
        :LOC-STN-STT-STS-NOF-LOT-PPC,
        :LOC-STN-STT-STS-NOF-LVN,
        :LOC-STN-STT-STS-NOF-LVN-PPC,
        :LOC-STN-STT-STS-NOF-NOL,
        :LOC-STN-STT-STS-NOF-NOL-LOT,
        :LOC-STN-STT-STS-NOF-NOL-LOT-LVN,
        :LOC-STN-STT-STS-NOF-NOL-LOT-LVN-PPC,
        :LOC-STN-STT-STS-NOF-NOL-LOT-PPC,
        :LOC-STN-STT-STS-NOF-NOL-LVN,
        :LOC-STN-STT-STS-NOF-NOL-LVN-PPC,
        :LOC-STN-STT-STS-NOF-NOL-PPC,
        :LOC-STN-STT-STS-NOF-PPC,
        :LOC-STN-STT-STS-NOL,
        :LOC-STN-STT-STS-NOL-LOT,
        :LOC-STN-STT-STS-NOL-LOT-LVN,
        :LOC-STN-STT-STS-NOL-LOT-LVN-PPC,
        :LOC-STN-STT-STS-NOL-LOT-PPC,
        :LOC-STN-STT-STS-NOL-LVN,
        :LOC-STN-STT-STS-NOL-LVN-PPC,
        :LOC-STN-STT-STS-NOL-PPC,
        :LOC-STN-STT-STS-PPC,
        :LOC-STS,
        :LOC-STS-LOT,
        :LOC-STS-LOT-LVN,
        :LOC-STS-LOT-LVN-PPC,
        :LOC-STS-LOT-PPC,
        :LOC-STS-LVN,
        :LOC-STS-LVN-PPC,
        :LOC-STS-NOF,
        :LOC-STS-NOF-LOT,
        :LOC-STS-NOF-LOT-LVN,
        :LOC-STS-NOF-LOT-LVN-PPC,
        :LOC-STS-NOF-LOT-PPC,
        :LOC-STS-NOF-LVN,
        :LOC-STS-NOF-LVN-PPC,
        :LOC-STS-NOF-NOL,
        :LOC-STS-NOF-NOL-LOT,
        :LOC-STS-NOF-NOL-LOT-LVN,
        :LOC-STS-NOF-NOL-LOT-LVN-PPC,
        :LOC-STS-NOF-NOL-LOT-PPC,
        :LOC-STS-NOF-NOL-LVN,
        :LOC-STS-NOF-NOL-LVN-PPC,
        :LOC-STS-NOF-NOL-PPC,
        :LOC-STS-NOF-PPC,
        :LOC-STS-NOL,
        :LOC-STS-NOL-LOT,
        :LOC-STS-NOL-LOT-LVN,
        :LOC-STS-NOL-LOT-LVN-PPC,
        :LOC-STS-NOL-LOT-PPC,
        :LOC-STS-NOL-LVN,
        :LOC-STS-NOL-LVN-PPC,
        :LOC-STS-NOL-PPC,
        :LOC-STS-PPC,
        :LOC-STT,
        :LOC-STT-LOT,
        :LOC-STT-LOT-LVN,
        :LOC-STT-LOT-LVN-PPC,
        :LOC-STT-LOT-PPC,
        :LOC-STT-LVN,
        :LOC-STT-LVN-PPC,
        :LOC-STT-NOF,
        :LOC-STT-NOF-LOT,
        :LOC-STT-NOF-LOT-LVN,
        :LOC-STT-NOF-LOT-LVN-PPC,
        :LOC-STT-NOF-LOT-PPC,
        :LOC-STT-NOF-LVN,
        :LOC-STT-NOF-LVN-PPC,
        :LOC-STT-NOF-NOL,
        :LOC-STT-NOF-NOL-LOT,
        :LOC-STT-NOF-NOL-LOT-LVN,
        :LOC-STT-NOF-NOL-LOT-LVN-PPC,
        :LOC-STT-NOF-NOL-LOT-PPC,
        :LOC-STT-NOF-NOL-LVN,
        :LOC-STT-NOF-NOL-LVN-PPC,
        :LOC-STT-NOF-NOL-PPC,
        :LOC-STT-NOF-PPC,
        :LOC-STT-NOL,
        :LOC-STT-NOL-LOT,
        :LOC-STT-NOL-LOT-LVN,
        :LOC-STT-NOL-LOT-LVN-PPC,
        :LOC-STT-NOL-LOT-PPC,
        :LOC-STT-NOL-LVN,
        :LOC-STT-NOL-LVN-PPC,
        :LOC-STT-NOL-PPC,
        :LOC-STT-PPC,
        :LOC-STT-STS,
        :LOC-STT-STS-LOT,
        :LOC-STT-STS-LOT-LVN,
        :LOC-STT-STS-LOT-LVN-PPC,
        :LOC-STT-STS-LOT-PPC,
        :LOC-STT-STS-LVN,
        :LOC-STT-STS-LVN-PPC,
        :LOC-STT-STS-NOF,
        :LOC-STT-STS-NOF-LOT,
        :LOC-STT-STS-NOF-LOT-LVN,
        :LOC-STT-STS-NOF-LOT-LVN-PPC,
        :LOC-STT-STS-NOF-LOT-PPC,
        :LOC-STT-STS-NOF-LVN,
        :LOC-STT-STS-NOF-LVN-PPC,
        :LOC-STT-STS-NOF-NOL,
        :LOC-STT-STS-NOF-NOL-LOT,
        :LOC-STT-STS-NOF-NOL-LOT-LVN,
        :LOC-STT-STS-NOF-NOL-LOT-LVN-PPC,
        :LOC-STT-STS-NOF-NOL-LOT-PPC,
        :LOC-STT-STS-NOF-NOL-LVN,
        :LOC-STT-STS-NOF-NOL-LVN-PPC,
        :LOC-STT-STS-NOF-NOL-PPC,
        :LOC-STT-STS-NOF-PPC,
        :LOC-STT-STS-NOL,
        :LOC-STT-STS-NOL-LOT,
        :LOC-STT-STS-NOL-LOT-LVN,
        :LOC-STT-STS-NOL-LOT-LVN-PPC,
        :LOC-STT-STS-NOL-LOT-PPC,
        :LOC-STT-STS-NOL-LVN,
        :LOC-STT-STS-NOL-LVN-PPC,
        :LOC-STT-STS-NOL-PPC,
        :LOC-STT-STS-PPC,
        :LOT,
        :LOT-LVN,
        :LOT-LVN-PPC,
        :LOT-PPC,
        :LVN,
        :LVN-PPC,
        :NOF,
        :NOF-LOT,
        :NOF-LOT-LVN,
        :NOF-LOT-LVN-PPC,
        :NOF-LOT-PPC,
        :NOF-LVN,
        :NOF-LVN-PPC,
        :NOF-NOL,
        :NOF-NOL-LOT,
        :NOF-NOL-LOT-LVN,
        :NOF-NOL-LOT-LVN-PPC,
        :NOF-NOL-LOT-PPC,
        :NOF-NOL-LVN,
        :NOF-NOL-LVN-PPC,
        :NOF-NOL-PPC,
        :NOF-PPC,
        :NOL,
        :NOL-LOT,
        :NOL-LOT-LVN,
        :NOL-LOT-LVN-PPC,
        :NOL-LOT-PPC,
        :NOL-LVN,
        :NOL-LVN-PPC,
        :NOL-PPC,
        :PPC,
        :STN,
        :STN-LOT,
        :STN-LOT-LVN,
        :STN-LOT-LVN-PPC,
        :STN-LOT-PPC,
        :STN-LVN,
        :STN-LVN-PPC,
        :STN-NOF,
        :STN-NOF-LOT,
        :STN-NOF-LOT-LVN,
        :STN-NOF-LOT-LVN-PPC,
        :STN-NOF-LOT-PPC,
        :STN-NOF-LVN,
        :STN-NOF-LVN-PPC,
        :STN-NOF-NOL,
        :STN-NOF-NOL-LOT,
        :STN-NOF-NOL-LOT-LVN,
        :STN-NOF-NOL-LOT-LVN-PPC,
        :STN-NOF-NOL-LOT-PPC,
        :STN-NOF-NOL-LVN,
        :STN-NOF-NOL-LVN-PPC,
        :STN-NOF-NOL-PPC,
        :STN-NOF-PPC,
        :STN-NOL,
        :STN-NOL-LOT,
        :STN-NOL-LOT-LVN,
        :STN-NOL-LOT-LVN-PPC,
        :STN-NOL-LOT-PPC,
        :STN-NOL-LVN,
        :STN-NOL-LVN-PPC,
        :STN-NOL-PPC,
        :STN-PPC,
        :STN-STS,
        :STN-STS-LOT,
        :STN-STS-LOT-LVN,
        :STN-STS-LOT-LVN-PPC,
        :STN-STS-LOT-PPC,
        :STN-STS-LVN,
        :STN-STS-LVN-PPC,
        :STN-STS-NOF,
        :STN-STS-NOF-LOT,
        :STN-STS-NOF-LOT-LVN,
        :STN-STS-NOF-LOT-LVN-PPC,
        :STN-STS-NOF-LOT-PPC,
        :STN-STS-NOF-LVN,
        :STN-STS-NOF-LVN-PPC,
        :STN-STS-NOF-NOL,
        :STN-STS-NOF-NOL-LOT,
        :STN-STS-NOF-NOL-LOT-LVN,
        :STN-STS-NOF-NOL-LOT-LVN-PPC,
        :STN-STS-NOF-NOL-LOT-PPC,
        :STN-STS-NOF-NOL-LVN,
        :STN-STS-NOF-NOL-LVN-PPC,
        :STN-STS-NOF-NOL-PPC,
        :STN-STS-NOF-PPC,
        :STN-STS-NOL,
        :STN-STS-NOL-LOT,
        :STN-STS-NOL-LOT-LVN,
        :STN-STS-NOL-LOT-LVN-PPC,
        :STN-STS-NOL-LOT-PPC,
        :STN-STS-NOL-LVN,
        :STN-STS-NOL-LVN-PPC,
        :STN-STS-NOL-PPC,
        :STN-STS-PPC,
        :STN-STT,
        :STN-STT-LOT,
        :STN-STT-LOT-LVN,
        :STN-STT-LOT-LVN-PPC,
        :STN-STT-LOT-PPC,
        :STN-STT-LVN,
        :STN-STT-LVN-PPC,
        :STN-STT-NOF,
        :STN-STT-NOF-LOT,
        :STN-STT-NOF-LOT-LVN,
        :STN-STT-NOF-LOT-LVN-PPC,
        :STN-STT-NOF-LOT-PPC,
        :STN-STT-NOF-LVN,
        :STN-STT-NOF-LVN-PPC,
        :STN-STT-NOF-NOL,
        :STN-STT-NOF-NOL-LOT,
        :STN-STT-NOF-NOL-LOT-LVN,
        :STN-STT-NOF-NOL-LOT-LVN-PPC,
        :STN-STT-NOF-NOL-LOT-PPC,
        :STN-STT-NOF-NOL-LVN,
        :STN-STT-NOF-NOL-LVN-PPC,
        :STN-STT-NOF-NOL-PPC,
        :STN-STT-NOF-PPC,
        :STN-STT-NOL,
        :STN-STT-NOL-LOT,
        :STN-STT-NOL-LOT-LVN,
        :STN-STT-NOL-LOT-LVN-PPC,
        :STN-STT-NOL-LOT-PPC,
        :STN-STT-NOL-LVN,
        :STN-STT-NOL-LVN-PPC,
        :STN-STT-NOL-PPC,
        :STN-STT-PPC,
        :STN-STT-STS,
        :STN-STT-STS-LOT,
        :STN-STT-STS-LOT-LVN,
        :STN-STT-STS-LOT-LVN-PPC,
        :STN-STT-STS-LOT-PPC,
        :STN-STT-STS-LVN,
        :STN-STT-STS-LVN-PPC,
        :STN-STT-STS-NOF,
        :STN-STT-STS-NOF-LOT,
        :STN-STT-STS-NOF-LOT-LVN,
        :STN-STT-STS-NOF-LOT-LVN-PPC,
        :STN-STT-STS-NOF-LOT-PPC,
        :STN-STT-STS-NOF-LVN,
        :STN-STT-STS-NOF-LVN-PPC,
        :STN-STT-STS-NOF-NOL,
        :STN-STT-STS-NOF-NOL-LOT,
        :STN-STT-STS-NOF-NOL-LOT-LVN,
        :STN-STT-STS-NOF-NOL-LOT-LVN-PPC,
        :STN-STT-STS-NOF-NOL-LOT-PPC,
        :STN-STT-STS-NOF-NOL-LVN,
        :STN-STT-STS-NOF-NOL-LVN-PPC,
        :STN-STT-STS-NOF-NOL-PPC,
        :STN-STT-STS-NOF-PPC,
        :STN-STT-STS-NOL,
        :STN-STT-STS-NOL-LOT,
        :STN-STT-STS-NOL-LOT-LVN,
        :STN-STT-STS-NOL-LOT-LVN-PPC,
        :STN-STT-STS-NOL-LOT-PPC,
        :STN-STT-STS-NOL-LVN,
        :STN-STT-STS-NOL-LVN-PPC,
        :STN-STT-STS-NOL-PPC,
        :STN-STT-STS-PPC,
        :STS,
        :STS-LOT,
        :STS-LOT-LVN,
        :STS-LOT-LVN-PPC,
        :STS-LOT-PPC,
        :STS-LVN,
        :STS-LVN-PPC,
        :STS-NOF,
        :STS-NOF-LOT,
        :STS-NOF-LOT-LVN,
        :STS-NOF-LOT-LVN-PPC,
        :STS-NOF-LOT-PPC,
        :STS-NOF-LVN,
        :STS-NOF-LVN-PPC,
        :STS-NOF-NOL,
        :STS-NOF-NOL-LOT,
        :STS-NOF-NOL-LOT-LVN,
        :STS-NOF-NOL-LOT-LVN-PPC,
        :STS-NOF-NOL-LOT-PPC,
        :STS-NOF-NOL-LVN,
        :STS-NOF-NOL-LVN-PPC,
        :STS-NOF-NOL-PPC,
        :STS-NOF-PPC,
        :STS-NOL,
        :STS-NOL-LOT,
        :STS-NOL-LOT-LVN,
        :STS-NOL-LOT-LVN-PPC,
        :STS-NOL-LOT-PPC,
        :STS-NOL-LVN,
        :STS-NOL-LVN-PPC,
        :STS-NOL-PPC,
        :STS-PPC,
        :STT,
        :STT-LOT,
        :STT-LOT-LVN,
        :STT-LOT-LVN-PPC,
        :STT-LOT-PPC,
        :STT-LVN,
        :STT-LVN-PPC,
        :STT-NOF,
        :STT-NOF-LOT,
        :STT-NOF-LOT-LVN,
        :STT-NOF-LOT-LVN-PPC,
        :STT-NOF-LOT-PPC,
        :STT-NOF-LVN,
        :STT-NOF-LVN-PPC,
        :STT-NOF-NOL,
        :STT-NOF-NOL-LOT,
        :STT-NOF-NOL-LOT-LVN,
        :STT-NOF-NOL-LOT-LVN-PPC,
        :STT-NOF-NOL-LOT-PPC,
        :STT-NOF-NOL-LVN,
        :STT-NOF-NOL-LVN-PPC,
        :STT-NOF-NOL-PPC,
        :STT-NOF-PPC,
        :STT-NOL,
        :STT-NOL-LOT,
        :STT-NOL-LOT-LVN,
        :STT-NOL-LOT-LVN-PPC,
        :STT-NOL-LOT-PPC,
        :STT-NOL-LVN,
        :STT-NOL-LVN-PPC,
        :STT-NOL-PPC,
        :STT-PPC,
        :STT-STS,
        :STT-STS-LOT,
        :STT-STS-LOT-LVN,
        :STT-STS-LOT-LVN-PPC,
        :STT-STS-LOT-PPC,
        :STT-STS-LVN,
        :STT-STS-LVN-PPC,
        :STT-STS-NOF,
        :STT-STS-NOF-LOT,
        :STT-STS-NOF-LOT-LVN,
        :STT-STS-NOF-LOT-LVN-PPC,
        :STT-STS-NOF-LOT-PPC,
        :STT-STS-NOF-LVN,
        :STT-STS-NOF-LVN-PPC,
        :STT-STS-NOF-NOL,
        :STT-STS-NOF-NOL-LOT,
        :STT-STS-NOF-NOL-LOT-LVN,
        :STT-STS-NOF-NOL-LOT-LVN-PPC,
        :STT-STS-NOF-NOL-LOT-PPC,
        :STT-STS-NOF-NOL-LVN,
        :STT-STS-NOF-NOL-LVN-PPC,
        :STT-STS-NOF-NOL-PPC,
        :STT-STS-NOF-PPC,
        :STT-STS-NOL,
        :STT-STS-NOL-LOT,
        :STT-STS-NOL-LOT-LVN,
        :STT-STS-NOL-LOT-LVN-PPC,
        :STT-STS-NOL-LOT-PPC,
        :STT-STS-NOL-LVN,
        :STT-STS-NOL-LVN-PPC,
        :STT-STS-NOL-PPC,
        :STT-STS-PPC ;
    skos:prefLabel "Address Change Type"@en ;
    sdo:creator <https://linked.data.gov.au/org/ga> ;
    sdo:publisher <https://linked.data.gov.au/org/icsm> .

