             @prefix bhd: <http://linked.data.gov.au/def/borehole-design/> .
@prefix dc: <http://purl.org/dc/elements/1.1/> .
@prefix dcterms: <http://purl.org/dc/terms/> .
@prefix owl: <http://www.w3.org/2002/07/owl#> .
@prefix rdfs: <http://www.w3.org/2000/01/rdf-schema#> .
@prefix sdo: <https://schema.org/> .
@prefix skos: <http://www.w3.org/2004/02/skos/core#> .
@prefix xsd: <http://www.w3.org/2001/XMLSchema#> .

<http://linked.data.gov.au/def/borehole-design> a owl:Ontology , skos:ConceptScheme ;
    dcterms:created "2019-10-03T16:24:51"^^xsd:dateTime ;
    dcterms:creator <http://linked.data.gov.au/org/gsq> ;
    dcterms:modified "2019-10-03T16:32:36"^^xsd:dateTime ;
    dcterms:publisher <http://linked.data.gov.au/org/gsq> ;
    dcterms:provenance "Developed by the Geological Survey of Queensland." ;
    skos:definition "A description of the intended configuration and trajectory of a borehole."@en ;
    skos:hasTopConcept bhd:deviated,
        bhd:inclinedup,
        bhd:inclineddown,
        bhd:lateral,
        bhd:vertical ;
    skos:prefLabel "Borehole Design"@en .

<http://linked.data.gov.au/org/gsq> a sdo:Organization ;
    sdo:name "Geological Survey of Queensland" ;
    sdo:url "https://www.business.qld.gov.au/industries/mining-energy-water/resources/geoscience-information/gsq"^^xsd:anyURI .

bhd:deviated a skos:Concept ;
    rdfs:isDefinedBy <http://linked.data.gov.au/def/borehole-design> ;
    skos:altLabel "Directional"@en ;
    skos:definition "A borehole drilled with geosteering equipment with the intent of controlling inclination and/or azimuth on a specified trajectory to intersect a target or targets."@en ;
    skos:inScheme <http://linked.data.gov.au/def/borehole-design> ;
    skos:prefLabel "Deviated"@en ;
    skos:topConceptOf <http://linked.data.gov.au/def/borehole-design> .

bhd:inclinedup a skos:Concept ;
    rdfs:isDefinedBy <http://linked.data.gov.au/def/borehole-design> ;
    skos:definition "A borehole drilled without geosteering equipment at a non-vertical angle above horizontal."@en ;
    skos:inScheme <http://linked.data.gov.au/def/borehole-design> ;
    skos:prefLabel "Inclined Up"@en ;
    skos:topConceptOf <http://linked.data.gov.au/def/borehole-design> .

bhd:inclineddown a skos:Concept ;
    rdfs:isDefinedBy <http://linked.data.gov.au/def/borehole-design> ;
    skos:altLabel "Inclined"@en ;
    skos:definition "A borehole drilled without geosteering equipment at a non-vertical angle at or below horizontal."@en ;
    skos:inScheme <http://linked.data.gov.au/def/borehole-design> ;
    skos:prefLabel "Inclined Down"@en ;
    skos:topConceptOf <http://linked.data.gov.au/def/borehole-design> .

bhd:lateral a skos:Concept ;
    rdfs:isDefinedBy <http://linked.data.gov.au/def/borehole-design> ;
    skos:altLabel "Horizontal"@en ;
    skos:definition "A borehole drilled with geosteering equipment with the intent of controlling the trajectory to drill laterally within a targeted stratigraphic interval or intervals."@en ;
    skos:inScheme <http://linked.data.gov.au/def/borehole-design> ;
    skos:prefLabel "Lateral"@en ;
    skos:topConceptOf <http://linked.data.gov.au/def/borehole-design> .

bhd:vertical a skos:Concept ;
    rdfs:isDefinedBy <http://linked.data.gov.au/def/borehole-design> ;
    skos:definition "A borehole drilled in a vertical downward direction with the intent of maintaining a vertical trajectory."@en ;
    skos:inScheme <http://linked.data.gov.au/def/borehole-design> ;
    skos:prefLabel "Vertical"@en ;
    skos:topConceptOf <http://linked.data.gov.au/def/borehole-design> .
