# baseURI: https://linked.data.gov.au/def/fsdf/ground-relations
# prefix: ground

@prefix cs: <https://linked.data.gov.au/def/fsdf/ground-relations> .
@prefix dcterms: <http://purl.org/dc/terms/> .
@prefix fsdf: <https://linked.data.gov.au/def/fsdf/> .
@prefix ground: <https://linked.data.gov.au/def/fsdf/ground-relations/> .
@prefix owl: <http://www.w3.org/2002/07/owl#> .
@prefix rdf: <http://www.w3.org/1999/02/22-rdf-syntax-ns#> .
@prefix rdfs: <http://www.w3.org/2000/01/rdf-schema#> .
@prefix skos: <http://www.w3.org/2004/02/skos/core#> .
@prefix xsd: <http://www.w3.org/2001/XMLSchema#> .


cs: 
    a owl:Ontology , skos:ConceptScheme ;
    skos:prefLabel "FSDF Ground Relations" ;
    dcterms:creator <https://linked.data.gov.au/org/ga> ;
    dcterms:publisher <https://linked.data.gov.au/org/icsm> ;
    dcterms:license <http://purl.org/NET/rdflicense/cc-by4.0> ;
    dcterms:created "2021-06-08"^^xsd:date ;
    dcterms:modified "2021-06-08"^^xsd:date ;
    dcterms:provenance "Created for the Loc-I DR Project"@en ;
    skos:definition "This vocabulary lists relations of geospatial Feature to the earth's surface"@en ;
    owl:versionInfo "1.0"^^xsd:string ;
    skos:hasTopConcept
    	ground:aboveGround ,
        ground:belowGround ,
        ground:atGround ,
        ground:unknown ;
.

ground:aboveGround
    a skos:Concept , fsdf:GroundRelation ;
    skos:prefLabel "Above Ground"@en ;
    skos:definition "The Feature is entirely above - on or over - the earth's surface"@en ;
    rdfs:isDefinedBy cs: ;
    skos:inScheme cs: ;
    skos:topConceptOf cs: ;
.

ground:belowGround
    a skos:Concept , fsdf:GroundRelation ;
    skos:prefLabel "Below Ground"@en ;
    skos:definition "The Feature is entirely below - or under - the earth's surface"@en ;
    rdfs:isDefinedBy cs: ;
    skos:inScheme cs: ;
    skos:topConceptOf cs: ;
.

ground:aboveAndBelowGround
    a skos:Concept , fsdf:GroundRelation ;
    skos:broader ground:aboveGround , ground:belowGround ;
    skos:prefLabel "Above and Below Ground"@en ;
    skos:definition "The Feature is both above - on or over - and below - under - the earth's surface"@en ;
    rdfs:isDefinedBy cs: ;
    skos:inScheme cs: ;
    skos:topConceptOf cs: ;
.

ground:atGround
    a skos:Concept , fsdf:GroundRelation ;
    skos:prefLabel "At Ground"@en ;
    skos:definition "The Feature in the place of the earth's surface"@en ;
    rdfs:isDefinedBy cs: ;
    skos:inScheme cs: ;
    skos:topConceptOf cs: ;
.

ground:unknown
    a skos:Concept , fsdf:GroundRelation ;
    skos:prefLabel "Unknown"@en ;
    skos:definition "The Feature's relation to the 'earth's surface is not known"@en ;
    rdfs:isDefinedBy cs: ;
    skos:inScheme cs: ;
    skos:topConceptOf cs: ;
.
